<?xml version="1.0"?>


<!DOCTYPE rdf:RDF [
    <!ENTITY owl "http://www.w3.org/2002/07/owl#" >
    <!ENTITY swrl "http://www.w3.org/2003/11/swrl#" >
    <!ENTITY swrlb "http://www.w3.org/2003/11/swrlb#" >
    <!ENTITY xsd "http://www.w3.org/2001/XMLSchema#" >
    <!ENTITY rdfs "http://www.w3.org/2000/01/rdf-schema#" >
    <!ENTITY rdf "http://www.w3.org/1999/02/22-rdf-syntax-ns#" >
    <!ENTITY protege "http://protege.stanford.edu/plugins/owl/protege#" >
    <!ENTITY xsp "http://www.owl-ontologies.com/2005/08/07/xsp.owl#" >
    <!ENTITY kern "http://europe.bourges.univ-orleans.fr/sites/default/files/download/Ontology/kernel.owl#" >
]>


<rdf:RDF xmlns="http://europe.bourges.univ-orleans.fr/sites/default/files/download/Ontology/Core/kernel.owl#"
     xml:base="http://europe.bourges.univ-orleans.fr/sites/default/files/download/Ontology/Core/kernel.owl"
     xmlns:xsp="http://www.owl-ontologies.com/2005/08/07/xsp.owl#"
     xmlns:kern="http://europe.bourges.univ-orleans.fr/sites/default/files/download/Ontology/kernel.owl#"
     xmlns:rdf="http://www.w3.org/1999/02/22-rdf-syntax-ns#"
     xmlns:owl="http://www.w3.org/2002/07/owl#"
     xmlns:swrlb="http://www.w3.org/2003/11/swrlb#"
     xmlns:protege="http://protege.stanford.edu/plugins/owl/protege#"
     xmlns:swrl="http://www.w3.org/2003/11/swrl#"
     xmlns:xsd="http://www.w3.org/2001/XMLSchema#"
     xmlns:rdfs="http://www.w3.org/2000/01/rdf-schema#">
    <owl:Ontology rdf:about="http://europe.bourges.univ-orleans.fr/sites/default/files/download/Ontology/Core/kernel.owl">
        <otherURI rdf:datatype="&xsd;anyURI">https://github.com/RobotML/RobotML/wiki/Ontology-evolution</otherURI>
        <TODO xml:lang="en">1. Definitions linked to event, evolution machine, ... have to be aligned as close as possible to DEVS theory.
2. Rules definition must be completed</TODO>
        <rdfs:comment xml:lang="en">The goal of the ontology is to help and support:
- the creation of specialised languages for robotics
- the creation of a standardised protocol dedicated to robots cooperation
- the creation of a standardised way to understand what is a simulation

It is organised in three logical parts. First part provides concepts to manipulate &quot;systems&quot;, static as well as dynamic through:
- Static representation
-&gt; System
-&gt; Architecture
-&gt; Component
-&gt; Interaction

- Dynamic representation
-&gt; Evolution model
-&gt; State
-&gt; derived in InteractionState and ComponentState

Second part is the representation of the physical world, of the universe of the problem. It includes:
- Environment
- PhysicalObject
- Hardware and Hardware{Aggregate|Component}
- PhysicalInteraction
- Referential

Third part is the representation of the software &quot;world&quot;. All that concerns information and how it is mapped onto the hardware:
- Software and Software{Aggregate|Component}
- SoftwareConnector
- Computer
- SoftwareToHardwareInteraction and HardwareToSoftwareInteraction (These two are very important as they allow the software to live in the hardware)</rdfs:comment>
        <rdfs:comment xml:lang="en">This work is based upon a previous one funded by the French Research agency ANR (Agence Nationale de la Recherche) through thePROTEUS project (see http://www.anr-project.fr). It is the property of its authors and is governed by the CECILL B V1 licence (see http://www.cecill.info for information and the associated Licence_CeCILL-B_V1-en.txt or Licence_CeCILL-B_V1-fr.txt files).</rdfs:comment>
        <rdfs:comment xml:lang="en">comments associated to rules
1. it needs a human to build a hardware
2. there is nothing else than an agent that can geenrate actions
3. if a system aggregates other systems then its isAtomic property is false
4. ...
x. if there is a software defined then there must be a hardware on which it executes</rdfs:comment>
        <author xml:lang="en">modified Bruno Patin - 03/10/2013
- addition of rule stating that an action is only done by an agent
modified Bruno Patin - 09/10/2013
- addition of a rule stating that hardware is built by human only
modified Bruno Patin - 13/10/2013
- addition of a comment in order to explain rules goals
modified Bruno Patin - 20/07/2014
- in order to know more easily what has been done from version to version a wiki page has been created on the RobotML github project (see https://github.com/RobotML/RobotML/wiki/Ontology-evolution)</author>
    </owl:Ontology>
    


    <!-- 
    ///////////////////////////////////////////////////////////////////////////////////////
    //
    // Annotation properties
    //
    ///////////////////////////////////////////////////////////////////////////////////////
     -->

    


    <!-- http://europe.bourges.univ-orleans.fr/sites/default/files/download/Ontology/Core/kernel.owl#TODO -->

    <owl:AnnotationProperty rdf:about="http://europe.bourges.univ-orleans.fr/sites/default/files/download/Ontology/Core/kernel.owl#TODO">
        <rdfs:comment xml:lang="en">this annotation allows its user to tag questions or requests for actions to be done / discussed with respect to the ontology.</rdfs:comment>
    </owl:AnnotationProperty>
    


    <!-- http://europe.bourges.univ-orleans.fr/sites/default/files/download/Ontology/Core/kernel.owl#author -->

    <owl:AnnotationProperty rdf:about="http://europe.bourges.univ-orleans.fr/sites/default/files/download/Ontology/Core/kernel.owl#author">
        <rdfs:comment xml:lang="en">creation Bruno Patin - 28/09/2013
- annotation created to track changes</rdfs:comment>
    </owl:AnnotationProperty>
    


    <!-- http://europe.bourges.univ-orleans.fr/sites/default/files/download/Ontology/Core/kernel.owl#openCycURI -->

    <owl:AnnotationProperty rdf:about="http://europe.bourges.univ-orleans.fr/sites/default/files/download/Ontology/Core/kernel.owl#openCycURI"/>
    


    <!-- http://europe.bourges.univ-orleans.fr/sites/default/files/download/Ontology/Core/kernel.owl#otherURI -->

    <owl:AnnotationProperty rdf:about="http://europe.bourges.univ-orleans.fr/sites/default/files/download/Ontology/Core/kernel.owl#otherURI"/>
    


    <!-- http://europe.bourges.univ-orleans.fr/sites/default/files/download/Ontology/Core/kernel.owl#wikipediaURI -->

    <owl:AnnotationProperty rdf:about="http://europe.bourges.univ-orleans.fr/sites/default/files/download/Ontology/Core/kernel.owl#wikipediaURI"/>
    


    <!-- http://europe.bourges.univ-orleans.fr/sites/default/files/download/Ontology/Core/kernel.owl#wiktionaryURI -->

    <owl:AnnotationProperty rdf:about="http://europe.bourges.univ-orleans.fr/sites/default/files/download/Ontology/Core/kernel.owl#wiktionaryURI"/>
    


    <!-- 
    ///////////////////////////////////////////////////////////////////////////////////////
    //
    // Object Properties
    //
    ///////////////////////////////////////////////////////////////////////////////////////
     -->

    


    <!-- http://europe.bourges.univ-orleans.fr/sites/default/files/download/Ontology/Core/environment.owl#isAssociatedToPO -->

    <owl:ObjectProperty rdf:about="http://europe.bourges.univ-orleans.fr/sites/default/files/download/Ontology/Core/environment.owl#isAssociatedToPO">
        <rdfs:domain rdf:resource="http://europe.bourges.univ-orleans.fr/sites/default/files/download/Ontology/Core/kernel.owl#Frame"/>
        <rdfs:range rdf:resource="http://europe.bourges.univ-orleans.fr/sites/default/files/download/Ontology/Core/kernel.owl#PhysicalObject"/>
    </owl:ObjectProperty>
    


    <!-- http://europe.bourges.univ-orleans.fr/sites/default/files/download/Ontology/Core/kernel.owl#OccursAfterEvent -->

    <owl:ObjectProperty rdf:about="http://europe.bourges.univ-orleans.fr/sites/default/files/download/Ontology/Core/kernel.owl#OccursAfterEvent">
        <rdfs:comment xml:lang="en">A time event occurs after another event.</rdfs:comment>
        <rdfs:range rdf:resource="http://europe.bourges.univ-orleans.fr/sites/default/files/download/Ontology/Core/kernel.owl#Event"/>
        <rdfs:domain rdf:resource="http://europe.bourges.univ-orleans.fr/sites/default/files/download/Ontology/Core/kernel.owl#TimeEvent"/>
    </owl:ObjectProperty>
    


    <!-- http://europe.bourges.univ-orleans.fr/sites/default/files/download/Ontology/Core/kernel.owl#aggregates -->

    <owl:ObjectProperty rdf:about="http://europe.bourges.univ-orleans.fr/sites/default/files/download/Ontology/Core/kernel.owl#aggregates">
        <openCycURI rdf:datatype="&xsd;anyURI">this property relates to the systemComponents OpenCyc property.
http://sw.opencyc.org/concept/Mx4rqWixJi_fQdiDAuNReZaKSg</openCycURI>
        <rdfs:comment xml:lang="en">aggregation is used in order to explains the system composition property. At this step, the &quot;min 2 system&quot; attribute of CompositeSystem leads to indecidability of ontology if putting in effect the ransitivity characteristic. 

a head is composed of 2 eyes is composed of eye 1 and eye 2. No transititvity means no verification of existence of software andf haredware at the lowest level.

This has to be tackled with in the meta-model itself.</rdfs:comment>
        <author xml:lang="en">creation PROTEUS consortium - 
modified Bruno Patin - 30/09/2013
- comment modified</author>
        <rdfs:domain rdf:resource="http://europe.bourges.univ-orleans.fr/sites/default/files/download/Ontology/Core/kernel.owl#CompositeSystem"/>
        <rdfs:range rdf:resource="http://europe.bourges.univ-orleans.fr/sites/default/files/download/Ontology/Core/kernel.owl#System"/>
    </owl:ObjectProperty>
    


    <!-- http://europe.bourges.univ-orleans.fr/sites/default/files/download/Ontology/Core/kernel.owl#animates -->

    <owl:ObjectProperty rdf:about="http://europe.bourges.univ-orleans.fr/sites/default/files/download/Ontology/Core/kernel.owl#animates">
        <wiktionaryURI xml:lang="en">See the first verb definition
http://en.wiktionary.org/wiki/animate</wiktionaryURI>
        <rdfs:comment xml:lang="en">animation is a property describing dynamicity of objects. In the scope of this ontology, Evolution IS the mechanism providing change to systems. Time is how man measures course of change but it has not to be confused.</rdfs:comment>
        <author xml:lang="en">creation PROTEUS consortium - 
modified Bruno Patin - 10/09/2013
- comment modified</author>
        <rdfs:domain rdf:resource="http://europe.bourges.univ-orleans.fr/sites/default/files/download/Ontology/Core/kernel.owl#Evolution"/>
        <rdfs:range rdf:resource="http://europe.bourges.univ-orleans.fr/sites/default/files/download/Ontology/Core/kernel.owl#System"/>
        <owl:inverseOf rdf:resource="http://europe.bourges.univ-orleans.fr/sites/default/files/download/Ontology/Core/kernel.owl#isAnimatedByEvolution"/>
    </owl:ObjectProperty>
    


    <!-- http://europe.bourges.univ-orleans.fr/sites/default/files/download/Ontology/Core/kernel.owl#belongsTo -->

    <owl:ObjectProperty rdf:about="http://europe.bourges.univ-orleans.fr/sites/default/files/download/Ontology/Core/kernel.owl#belongsTo">
        <rdfs:comment xml:lang="en">This property is specific to the time concept. It expresses the fact that the time concept means nothing outside the physical world and must be associated to at least one referential system.</rdfs:comment>
        <author xml:lang="en">creation PROTEUS consortium - 
modified Bruno Patin - 10/09/2013
- TODO annotation added
modified Bruno Parin - 20/06/2014
- TODO annotation deleted. There is no question that a time is linked to a frame in the existing mist updtaed theory we can use (General relativity) thus this concern is to disappear.</author>
        <rdfs:range rdf:resource="http://europe.bourges.univ-orleans.fr/sites/default/files/download/Ontology/Core/kernel.owl#Frame"/>
        <rdfs:domain rdf:resource="http://europe.bourges.univ-orleans.fr/sites/default/files/download/Ontology/Core/kernel.owl#Time"/>
        <owl:inverseOf rdf:resource="http://europe.bourges.univ-orleans.fr/sites/default/files/download/Ontology/Core/kernel.owl#definesSpaceTime"/>
    </owl:ObjectProperty>
    


    <!-- http://europe.bourges.univ-orleans.fr/sites/default/files/download/Ontology/Core/kernel.owl#carries -->

    <owl:ObjectProperty rdf:about="http://europe.bourges.univ-orleans.fr/sites/default/files/download/Ontology/Core/kernel.owl#carries">
        <rdfs:comment xml:lang="en">A connector carries interactions.</rdfs:comment>
        <rdfs:domain rdf:resource="http://europe.bourges.univ-orleans.fr/sites/default/files/download/Ontology/Core/kernel.owl#Connector"/>
        <rdfs:range rdf:resource="http://europe.bourges.univ-orleans.fr/sites/default/files/download/Ontology/Core/kernel.owl#Interaction"/>
    </owl:ObjectProperty>
    


    <!-- http://europe.bourges.univ-orleans.fr/sites/default/files/download/Ontology/Core/kernel.owl#constrains -->

    <owl:ObjectProperty rdf:about="http://europe.bourges.univ-orleans.fr/sites/default/files/download/Ontology/Core/kernel.owl#constrains">
        <rdfs:comment xml:lang="en">A protocol constrains the way information is exchanged between systems</rdfs:comment>
        <rdfs:range rdf:resource="http://europe.bourges.univ-orleans.fr/sites/default/files/download/Ontology/Core/kernel.owl#Information"/>
        <rdfs:domain rdf:resource="http://europe.bourges.univ-orleans.fr/sites/default/files/download/Ontology/Core/kernel.owl#Protocol"/>
    </owl:ObjectProperty>
    


    <!-- http://europe.bourges.univ-orleans.fr/sites/default/files/download/Ontology/Core/kernel.owl#constrainsFrame -->

    <owl:ObjectProperty rdf:about="http://europe.bourges.univ-orleans.fr/sites/default/files/download/Ontology/Core/kernel.owl#constrainsFrame">
        <rdfs:comment>this relation expresses the fact that there could exists contraints between frames of two physical objects for instance when two physical objects are in relation through joint. In order to implement the constraint, it is necessary to consider the parameterisation of the PhysicalInteraction in itself (or more its specialisations).</rdfs:comment>
        <author xml:lang="en">creation PROTEUS consortium - 
modified Bruno Patin - 10/09/2013
modified Bruno Patin - 21/06/2014
- annotation TODO added
- annotation TODO completed
modified Bruno Patin - 02/07/2014
- annotation TODO deleted</author>
        <rdfs:domain rdf:resource="http://europe.bourges.univ-orleans.fr/sites/default/files/download/Ontology/Core/kernel.owl#Frame"/>
        <rdfs:range rdf:resource="http://europe.bourges.univ-orleans.fr/sites/default/files/download/Ontology/Core/kernel.owl#Frame"/>
    </owl:ObjectProperty>
    


    <!-- http://europe.bourges.univ-orleans.fr/sites/default/files/download/Ontology/Core/kernel.owl#currentlyPerforms -->

    <owl:ObjectProperty rdf:about="http://europe.bourges.univ-orleans.fr/sites/default/files/download/Ontology/Core/kernel.owl#currentlyPerforms">
        <rdfs:seeAlso rdf:datatype="&xsd;string">ORO: currentlyPerforms</rdfs:seeAlso>
        <rdfs:isDefinedBy rdf:datatype="&xsd;anyURI">http://kb.openrobots.org#currentlyPerforms</rdfs:isDefinedBy>
        <rdfs:comment xml:lang="en">an Agent performs actions and thus is always currently performing some action even if it is nothing</rdfs:comment>
        <rdfs:range rdf:resource="http://europe.bourges.univ-orleans.fr/sites/default/files/download/Ontology/Core/kernel.owl#Action"/>
        <rdfs:domain rdf:resource="http://europe.bourges.univ-orleans.fr/sites/default/files/download/Ontology/Core/kernel.owl#Agent"/>
        <owl:inverseOf rdf:resource="http://europe.bourges.univ-orleans.fr/sites/default/files/download/Ontology/Core/kernel.owl#isPerformedBy"/>
    </owl:ObjectProperty>
    


    <!-- http://europe.bourges.univ-orleans.fr/sites/default/files/download/Ontology/Core/kernel.owl#definesAFrame -->

    <owl:ObjectProperty rdf:about="http://europe.bourges.univ-orleans.fr/sites/default/files/download/Ontology/Core/kernel.owl#definesAFrame">
        <rdf:type rdf:resource="&owl;FunctionalProperty"/>
        <rdfs:comment xml:lang="en">this property expresses the fact that every physical object is associated to a frame providing it its existence in space and time.</rdfs:comment>
        <owl:inverseOf rdf:resource="http://europe.bourges.univ-orleans.fr/sites/default/files/download/Ontology/Core/environment.owl#isAssociatedToPO"/>
        <rdfs:range rdf:resource="http://europe.bourges.univ-orleans.fr/sites/default/files/download/Ontology/Core/kernel.owl#Frame"/>
        <rdfs:domain rdf:resource="http://europe.bourges.univ-orleans.fr/sites/default/files/download/Ontology/Core/kernel.owl#PhysicalObject"/>
    </owl:ObjectProperty>
    


    <!-- http://europe.bourges.univ-orleans.fr/sites/default/files/download/Ontology/Core/kernel.owl#definesSpaceTime -->

    <owl:ObjectProperty rdf:about="http://europe.bourges.univ-orleans.fr/sites/default/files/download/Ontology/Core/kernel.owl#definesSpaceTime">
        <rdfs:comment xml:lang="en">A frame is associated to a local time.</rdfs:comment>
        <rdfs:domain rdf:resource="http://europe.bourges.univ-orleans.fr/sites/default/files/download/Ontology/Core/kernel.owl#Frame"/>
        <rdfs:range rdf:resource="http://europe.bourges.univ-orleans.fr/sites/default/files/download/Ontology/Core/kernel.owl#Time"/>
    </owl:ObjectProperty>
    


    <!-- http://europe.bourges.univ-orleans.fr/sites/default/files/download/Ontology/Core/kernel.owl#describe -->

    <owl:ObjectProperty rdf:about="http://europe.bourges.univ-orleans.fr/sites/default/files/download/Ontology/Core/kernel.owl#describe">
        <wiktionaryURI rdf:datatype="&xsd;anyURI">http://en.wiktionary.org/wiki/describe</wiktionaryURI>
        <openCycURI rdf:datatype="&xsd;anyURI">http://sw.opencyc.org/concept/Mx4rfQCRhMFcEdmAAAACs6hRjg</openCycURI>
        <rdfs:comment xml:lang="en">The &quot;describe&quot; property is the capability for any piece of information to provide an insight on universe / world and its content. It means everything including information (quotation or comment). This description is always done by an agent either writing something or speaking.</rdfs:comment>
        <author xml:lang="en">creation Bruno Patin - 08/09/2013
modified Bruno Patin - 10/09/2013
- addition of OpenCyc link
- modification of comment</author>
        <rdfs:domain rdf:resource="http://europe.bourges.univ-orleans.fr/sites/default/files/download/Ontology/Core/kernel.owl#Information"/>
        <rdfs:range rdf:resource="&owl;Thing"/>
    </owl:ObjectProperty>
    


    <!-- http://europe.bourges.univ-orleans.fr/sites/default/files/download/Ontology/Core/kernel.owl#emits -->

    <owl:ObjectProperty rdf:about="http://europe.bourges.univ-orleans.fr/sites/default/files/download/Ontology/Core/kernel.owl#emits">
        <rdfs:comment xml:lang="en">Ports emit interactions</rdfs:comment>
        <rdfs:range rdf:resource="http://europe.bourges.univ-orleans.fr/sites/default/files/download/Ontology/Core/kernel.owl#Interaction"/>
        <rdfs:domain rdf:resource="http://europe.bourges.univ-orleans.fr/sites/default/files/download/Ontology/Core/kernel.owl#Port"/>
    </owl:ObjectProperty>
    


    <!-- http://europe.bourges.univ-orleans.fr/sites/default/files/download/Ontology/Core/kernel.owl#endsOn -->

    <owl:ObjectProperty rdf:about="http://europe.bourges.univ-orleans.fr/sites/default/files/download/Ontology/Core/kernel.owl#endsOn">
        <rdfs:comment xml:lang="en">A finite state machine has an end state</rdfs:comment>
        <rdfs:range rdf:resource="http://europe.bourges.univ-orleans.fr/sites/default/files/download/Ontology/Core/kernel.owl#AutomataEndState"/>
        <rdfs:domain rdf:resource="http://europe.bourges.univ-orleans.fr/sites/default/files/download/Ontology/Core/kernel.owl#StateMachine"/>
    </owl:ObjectProperty>
    


    <!-- http://europe.bourges.univ-orleans.fr/sites/default/files/download/Ontology/Core/kernel.owl#entail -->

    <owl:ObjectProperty rdf:about="http://europe.bourges.univ-orleans.fr/sites/default/files/download/Ontology/Core/kernel.owl#entail">
        <rdfs:comment xml:lang="en">A transition is triggered by an event after evaluation to truth-value of the established condition.</rdfs:comment>
        <rdfs:domain rdf:resource="http://europe.bourges.univ-orleans.fr/sites/default/files/download/Ontology/Core/kernel.owl#Event"/>
        <rdfs:range rdf:resource="http://europe.bourges.univ-orleans.fr/sites/default/files/download/Ontology/Core/kernel.owl#Transition"/>
    </owl:ObjectProperty>
    


    <!-- http://europe.bourges.univ-orleans.fr/sites/default/files/download/Ontology/Core/kernel.owl#evolvesSpatiallyWithRespectTo -->

    <owl:ObjectProperty rdf:about="http://europe.bourges.univ-orleans.fr/sites/default/files/download/Ontology/Core/kernel.owl#evolvesSpatiallyWithRespectTo">
        <rdfs:comment xml:lang="en">This property expresses the spatial relationships that can exist between physical objects whatever they are (fluidic as well as solid). In order to be of use it is necessary to be able to identify something AS a physical object. It introduces also the fact that there is ALWAYS at least one surface object to associate to this one physical object (property linked to physical objects).</rdfs:comment>
        <author xml:lang="en">creation Bruno Patin - 20/07/2014
modified Bruno Patin- 04/08/2014
- comment is refined</author>
        <rdfs:domain rdf:resource="http://europe.bourges.univ-orleans.fr/sites/default/files/download/Ontology/Core/kernel.owl#PhysicalObject"/>
        <rdfs:range rdf:resource="http://europe.bourges.univ-orleans.fr/sites/default/files/download/Ontology/Core/kernel.owl#PhysicalObject"/>
    </owl:ObjectProperty>
    


    <!-- http://europe.bourges.univ-orleans.fr/sites/default/files/download/Ontology/Core/kernel.owl#executesOn -->

    <owl:ObjectProperty rdf:about="http://europe.bourges.univ-orleans.fr/sites/default/files/download/Ontology/Core/kernel.owl#executesOn">
        <rdfs:comment xml:lang="en">This expresses the fact that there is no software running without a hardware that includes computation capability and supporting it.</rdfs:comment>
        <author xml:lang="en">creation PROTEUS consortium - 
modified Bruno Patin - 10/09/2013
- comment modified</author>
        <rdfs:range rdf:resource="http://europe.bourges.univ-orleans.fr/sites/default/files/download/Ontology/Core/kernel.owl#Hardware"/>
        <rdfs:domain rdf:resource="http://europe.bourges.univ-orleans.fr/sites/default/files/download/Ontology/Core/kernel.owl#Software"/>
    </owl:ObjectProperty>
    


    <!-- http://europe.bourges.univ-orleans.fr/sites/default/files/download/Ontology/Core/kernel.owl#from -->

    <owl:ObjectProperty rdf:about="http://europe.bourges.univ-orleans.fr/sites/default/files/download/Ontology/Core/kernel.owl#from">
        <rdfs:comment xml:lang="en">A transition is defined by a start state and an end state</rdfs:comment>
        <rdfs:range rdf:resource="http://europe.bourges.univ-orleans.fr/sites/default/files/download/Ontology/Core/kernel.owl#AutomataState"/>
        <rdfs:domain rdf:resource="http://europe.bourges.univ-orleans.fr/sites/default/files/download/Ontology/Core/kernel.owl#Transition"/>
    </owl:ObjectProperty>
    


    <!-- http://europe.bourges.univ-orleans.fr/sites/default/files/download/Ontology/Core/kernel.owl#givesNextState -->

    <owl:ObjectProperty rdf:about="http://europe.bourges.univ-orleans.fr/sites/default/files/download/Ontology/Core/kernel.owl#givesNextState">
        <rdfs:comment xml:lang="en">The evolution model is able to provide the next state of a component using its previous known states and a time on which to evaluate the new state.</rdfs:comment>
        <rdfs:domain rdf:resource="http://europe.bourges.univ-orleans.fr/sites/default/files/download/Ontology/Core/kernel.owl#Evolution"/>
        <rdfs:range rdf:resource="http://europe.bourges.univ-orleans.fr/sites/default/files/download/Ontology/Core/kernel.owl#State"/>
    </owl:ObjectProperty>
    


    <!-- http://europe.bourges.univ-orleans.fr/sites/default/files/download/Ontology/Core/kernel.owl#has -->

    <owl:ObjectProperty rdf:about="http://europe.bourges.univ-orleans.fr/sites/default/files/download/Ontology/Core/kernel.owl#has">
        <rdfs:comment xml:lang="en">Things have things.</rdfs:comment>
        <owl:inverseOf rdf:resource="http://europe.bourges.univ-orleans.fr/sites/default/files/download/Ontology/Core/kernel.owl#isPropertyOf"/>
    </owl:ObjectProperty>
    


    <!-- http://europe.bourges.univ-orleans.fr/sites/default/files/download/Ontology/Core/kernel.owl#hasAction -->

    <owl:ObjectProperty rdf:about="http://europe.bourges.univ-orleans.fr/sites/default/files/download/Ontology/Core/kernel.owl#hasAction">
        <rdfs:comment xml:lang="en">An Activity is constituted by a set of Actions.</rdfs:comment>
        <rdfs:range rdf:resource="http://europe.bourges.univ-orleans.fr/sites/default/files/download/Ontology/Core/kernel.owl#Action"/>
        <rdfs:domain rdf:resource="http://europe.bourges.univ-orleans.fr/sites/default/files/download/Ontology/Core/kernel.owl#Activity"/>
        <rdfs:subPropertyOf rdf:resource="http://europe.bourges.univ-orleans.fr/sites/default/files/download/Ontology/Core/kernel.owl#has"/>
    </owl:ObjectProperty>
    


    <!-- http://europe.bourges.univ-orleans.fr/sites/default/files/download/Ontology/Core/kernel.owl#hasActivity -->

    <owl:ObjectProperty rdf:about="http://europe.bourges.univ-orleans.fr/sites/default/files/download/Ontology/Core/kernel.owl#hasActivity">
        <rdfs:comment xml:lang="en">An agent is linked to the Activity made by the actions performed by this agent.</rdfs:comment>
        <rdfs:range rdf:resource="http://europe.bourges.univ-orleans.fr/sites/default/files/download/Ontology/Core/kernel.owl#Activity"/>
        <rdfs:domain rdf:resource="http://europe.bourges.univ-orleans.fr/sites/default/files/download/Ontology/Core/kernel.owl#Agent"/>
        <rdfs:subPropertyOf rdf:resource="http://europe.bourges.univ-orleans.fr/sites/default/files/download/Ontology/Core/kernel.owl#has"/>
    </owl:ObjectProperty>
    


    <!-- http://europe.bourges.univ-orleans.fr/sites/default/files/download/Ontology/Core/kernel.owl#hasDownstreamPort -->

    <owl:ObjectProperty rdf:about="http://europe.bourges.univ-orleans.fr/sites/default/files/download/Ontology/Core/kernel.owl#hasDownstreamPort">
        <rdf:type rdf:resource="&owl;FunctionalProperty"/>
        <rdfs:comment xml:lang="en">A connector has a unique downstream port.</rdfs:comment>
        <rdfs:domain rdf:resource="http://europe.bourges.univ-orleans.fr/sites/default/files/download/Ontology/Core/kernel.owl#Connector"/>
        <rdfs:range rdf:resource="http://europe.bourges.univ-orleans.fr/sites/default/files/download/Ontology/Core/kernel.owl#Port"/>
        <rdfs:subPropertyOf rdf:resource="http://europe.bourges.univ-orleans.fr/sites/default/files/download/Ontology/Core/kernel.owl#has"/>
    </owl:ObjectProperty>
    


    <!-- http://europe.bourges.univ-orleans.fr/sites/default/files/download/Ontology/Core/kernel.owl#hasPort -->

    <owl:ObjectProperty rdf:about="http://europe.bourges.univ-orleans.fr/sites/default/files/download/Ontology/Core/kernel.owl#hasPort">
        <rdf:type rdf:resource="&owl;InverseFunctionalProperty"/>
        <rdfs:comment xml:lang="en">Property to qualify the fact that systems have ports.</rdfs:comment>
        <rdfs:range rdf:resource="http://europe.bourges.univ-orleans.fr/sites/default/files/download/Ontology/Core/kernel.owl#Port"/>
        <rdfs:domain rdf:resource="http://europe.bourges.univ-orleans.fr/sites/default/files/download/Ontology/Core/kernel.owl#System"/>
        <rdfs:subPropertyOf rdf:resource="http://europe.bourges.univ-orleans.fr/sites/default/files/download/Ontology/Core/kernel.owl#has"/>
    </owl:ObjectProperty>
    


    <!-- http://europe.bourges.univ-orleans.fr/sites/default/files/download/Ontology/Core/kernel.owl#hasPortValue -->

    <owl:ObjectProperty rdf:about="http://europe.bourges.univ-orleans.fr/sites/default/files/download/Ontology/Core/kernel.owl#hasPortValue">
        <rdfs:comment xml:lang="en">Each port of a system has some information to receive or to send through interactions from or to other systems. System being the &quot;reality&quot;, these information are abstraction.</rdfs:comment>
        <author xml:lang="en">creation PROTEUS consortium - 
modified Bruno Patin - 10/09/2013
- change of range (from data to information)
- comment completed to take above modification into account</author>
        <rdfs:range rdf:resource="http://europe.bourges.univ-orleans.fr/sites/default/files/download/Ontology/Core/kernel.owl#Abstraction"/>
        <rdfs:domain rdf:resource="http://europe.bourges.univ-orleans.fr/sites/default/files/download/Ontology/Core/kernel.owl#Port"/>
        <rdfs:subPropertyOf rdf:resource="http://europe.bourges.univ-orleans.fr/sites/default/files/download/Ontology/Core/kernel.owl#has"/>
    </owl:ObjectProperty>
    


    <!-- http://europe.bourges.univ-orleans.fr/sites/default/files/download/Ontology/Core/kernel.owl#hasProbe -->

    <owl:ObjectProperty rdf:about="http://europe.bourges.univ-orleans.fr/sites/default/files/download/Ontology/Core/kernel.owl#hasProbe">
        <rdfs:comment xml:lang="en">Systems can have probes to allow evolution model to survey the systems&apos; states.</rdfs:comment>
        <rdfs:range rdf:resource="http://europe.bourges.univ-orleans.fr/sites/default/files/download/Ontology/Core/kernel.owl#Probe"/>
        <rdfs:domain rdf:resource="http://europe.bourges.univ-orleans.fr/sites/default/files/download/Ontology/Core/kernel.owl#System"/>
        <rdfs:subPropertyOf rdf:resource="http://europe.bourges.univ-orleans.fr/sites/default/files/download/Ontology/Core/kernel.owl#has"/>
        <owl:inverseOf rdf:resource="http://europe.bourges.univ-orleans.fr/sites/default/files/download/Ontology/Core/kernel.owl#isProbeOf"/>
    </owl:ObjectProperty>
    


    <!-- http://europe.bourges.univ-orleans.fr/sites/default/files/download/Ontology/Core/kernel.owl#hasProtocol -->

    <owl:ObjectProperty rdf:about="http://europe.bourges.univ-orleans.fr/sites/default/files/download/Ontology/Core/kernel.owl#hasProtocol">
        <rdfs:comment xml:lang="en">An interaction can implement a protocol</rdfs:comment>
        <rdfs:range rdf:resource="http://europe.bourges.univ-orleans.fr/sites/default/files/download/Ontology/Core/kernel.owl#Protocol"/>
        <rdfs:subPropertyOf rdf:resource="http://europe.bourges.univ-orleans.fr/sites/default/files/download/Ontology/Core/kernel.owl#has"/>
        <rdfs:domain>
            <owl:Class>
                <owl:unionOf rdf:parseType="Collection">
                    <rdf:Description rdf:about="http://europe.bourges.univ-orleans.fr/sites/default/files/download/Ontology/Core/kernel.owl#Interaction"/>
                    <rdf:Description rdf:about="http://europe.bourges.univ-orleans.fr/sites/default/files/download/Ontology/Core/kernel.owl#Port"/>
                </owl:unionOf>
            </owl:Class>
        </rdfs:domain>
    </owl:ObjectProperty>
    


    <!-- http://europe.bourges.univ-orleans.fr/sites/default/files/download/Ontology/Core/kernel.owl#hasState -->

    <owl:ObjectProperty rdf:about="http://europe.bourges.univ-orleans.fr/sites/default/files/download/Ontology/Core/kernel.owl#hasState">
        <rdfs:comment xml:lang="en">each class associated through this link to state is able to have a set of state. It does not mean evolution because this is implemented through the evolution model that will allow an ordering of the set.</rdfs:comment>
        <rdfs:range rdf:resource="http://europe.bourges.univ-orleans.fr/sites/default/files/download/Ontology/Core/kernel.owl#State"/>
        <rdfs:subPropertyOf rdf:resource="http://europe.bourges.univ-orleans.fr/sites/default/files/download/Ontology/Core/kernel.owl#has"/>
        <rdfs:domain>
            <owl:Class>
                <owl:unionOf rdf:parseType="Collection">
                    <rdf:Description rdf:about="http://europe.bourges.univ-orleans.fr/sites/default/files/download/Ontology/Core/kernel.owl#Interaction"/>
                    <rdf:Description rdf:about="http://europe.bourges.univ-orleans.fr/sites/default/files/download/Ontology/Core/kernel.owl#System"/>
                </owl:unionOf>
            </owl:Class>
        </rdfs:domain>
    </owl:ObjectProperty>
    


    <!-- http://europe.bourges.univ-orleans.fr/sites/default/files/download/Ontology/Core/kernel.owl#hasStateVariables -->

    <owl:ObjectProperty rdf:about="http://europe.bourges.univ-orleans.fr/sites/default/files/download/Ontology/Core/kernel.owl#hasStateVariables">
        <rdfs:comment xml:lang="en">States have several state variables.
As State is an abstract concept describing object as they are thus the variables defining this state are of Abstraction types.</rdfs:comment>
        <author xml:lang="en">creation PROTEUS consortium - 
modified Bruno Patin - 10/09/2013
- Range modified due to added comment</author>
        <rdfs:range rdf:resource="http://europe.bourges.univ-orleans.fr/sites/default/files/download/Ontology/Core/kernel.owl#Abstraction"/>
        <rdfs:domain rdf:resource="http://europe.bourges.univ-orleans.fr/sites/default/files/download/Ontology/Core/kernel.owl#State"/>
        <rdfs:subPropertyOf rdf:resource="http://europe.bourges.univ-orleans.fr/sites/default/files/download/Ontology/Core/kernel.owl#has"/>
    </owl:ObjectProperty>
    


    <!-- http://europe.bourges.univ-orleans.fr/sites/default/files/download/Ontology/Core/kernel.owl#hasUpstreamPort -->

    <owl:ObjectProperty rdf:about="http://europe.bourges.univ-orleans.fr/sites/default/files/download/Ontology/Core/kernel.owl#hasUpstreamPort">
        <rdf:type rdf:resource="&owl;FunctionalProperty"/>
        <rdfs:comment xml:lang="en">A connector has a unique upstream port.</rdfs:comment>
        <rdfs:domain rdf:resource="http://europe.bourges.univ-orleans.fr/sites/default/files/download/Ontology/Core/kernel.owl#Connector"/>
        <rdfs:range rdf:resource="http://europe.bourges.univ-orleans.fr/sites/default/files/download/Ontology/Core/kernel.owl#Port"/>
        <rdfs:subPropertyOf rdf:resource="http://europe.bourges.univ-orleans.fr/sites/default/files/download/Ontology/Core/kernel.owl#has"/>
    </owl:ObjectProperty>
    


    <!-- http://europe.bourges.univ-orleans.fr/sites/default/files/download/Ontology/Core/kernel.owl#impacts -->

    <owl:ObjectProperty rdf:about="http://europe.bourges.univ-orleans.fr/sites/default/files/download/Ontology/Core/kernel.owl#impacts">
        <author xml:lang="en">creation PROTEUS consortium - 
modified Bruno Patin - 05/10/2013
- impacts is now the inverse of triggers</author>
        <rdfs:comment xml:lang="en">it is the interaction through its evolution that will impact the system by changing / modifying its state.</rdfs:comment>
        <rdfs:domain rdf:resource="http://europe.bourges.univ-orleans.fr/sites/default/files/download/Ontology/Core/kernel.owl#Interaction"/>
        <rdfs:range rdf:resource="http://europe.bourges.univ-orleans.fr/sites/default/files/download/Ontology/Core/kernel.owl#System"/>
    </owl:ObjectProperty>
    


    <!-- http://europe.bourges.univ-orleans.fr/sites/default/files/download/Ontology/Core/kernel.owl#impactsEvolution -->

    <owl:ObjectProperty rdf:about="http://europe.bourges.univ-orleans.fr/sites/default/files/download/Ontology/Core/kernel.owl#impactsEvolution">
        <rdf:type rdf:resource="&owl;FunctionalProperty"/>
        <rdfs:comment xml:lang="en">For instance, the evolution of a stone is not the same in the air and in the water</rdfs:comment>
        <author xml:lang="en">creation PROTEUS Consortium - 
modified Bruno Patin - 14/09/2014
- modification of name due to the fact that Environment does not impact EVolution, it defines it.</author>
        <rdfs:domain rdf:resource="http://europe.bourges.univ-orleans.fr/sites/default/files/download/Ontology/Core/kernel.owl#Environment"/>
        <rdfs:range rdf:resource="http://europe.bourges.univ-orleans.fr/sites/default/files/download/Ontology/Core/kernel.owl#PhysicalObject"/>
    </owl:ObjectProperty>
    


    <!-- http://europe.bourges.univ-orleans.fr/sites/default/files/download/Ontology/Core/kernel.owl#implements -->

    <owl:ObjectProperty rdf:about="http://europe.bourges.univ-orleans.fr/sites/default/files/download/Ontology/Core/kernel.owl#implements">
        <rdfs:comment xml:lang="en">Every data corresponds to an abstraction</rdfs:comment>
        <rdfs:range rdf:resource="http://europe.bourges.univ-orleans.fr/sites/default/files/download/Ontology/Core/kernel.owl#Abstraction"/>
        <rdfs:domain rdf:resource="http://europe.bourges.univ-orleans.fr/sites/default/files/download/Ontology/Core/kernel.owl#Data"/>
    </owl:ObjectProperty>
    


    <!-- http://europe.bourges.univ-orleans.fr/sites/default/files/download/Ontology/Core/kernel.owl#isAFunctionOfTime -->

    <owl:ObjectProperty rdf:about="http://europe.bourges.univ-orleans.fr/sites/default/files/download/Ontology/Core/kernel.owl#isAFunctionOfTime">
        <rdfs:comment xml:lang="en">ad hoc link that needs to be reworked as the evolution concept is an abstract view on the way architectures can evolve and time is a property of a physical object that is no more an abstraction.</rdfs:comment>
        <rdfs:domain rdf:resource="http://europe.bourges.univ-orleans.fr/sites/default/files/download/Ontology/Core/kernel.owl#Evolution"/>
        <rdfs:range rdf:resource="http://europe.bourges.univ-orleans.fr/sites/default/files/download/Ontology/Core/kernel.owl#Time"/>
    </owl:ObjectProperty>
    


    <!-- http://europe.bourges.univ-orleans.fr/sites/default/files/download/Ontology/Core/kernel.owl#isAnimatedByEvolution -->

    <owl:ObjectProperty rdf:about="http://europe.bourges.univ-orleans.fr/sites/default/files/download/Ontology/Core/kernel.owl#isAnimatedByEvolution">
        <rdfs:comment xml:lang="en">abstract property of systems to live.</rdfs:comment>
        <rdfs:range rdf:resource="http://europe.bourges.univ-orleans.fr/sites/default/files/download/Ontology/Core/kernel.owl#Evolution"/>
        <rdfs:domain rdf:resource="http://europe.bourges.univ-orleans.fr/sites/default/files/download/Ontology/Core/kernel.owl#System"/>
    </owl:ObjectProperty>
    


    <!-- http://europe.bourges.univ-orleans.fr/sites/default/files/download/Ontology/Core/kernel.owl#isCarriedBy -->

    <owl:ObjectProperty rdf:about="http://europe.bourges.univ-orleans.fr/sites/default/files/download/Ontology/Core/kernel.owl#isCarriedBy">
        <rdfs:comment xml:lang="en">An interaction is carried by connectors.</rdfs:comment>
        <rdfs:range rdf:resource="http://europe.bourges.univ-orleans.fr/sites/default/files/download/Ontology/Core/kernel.owl#Connector"/>
        <rdfs:domain rdf:resource="http://europe.bourges.univ-orleans.fr/sites/default/files/download/Ontology/Core/kernel.owl#Interaction"/>
        <owl:inverseOf rdf:resource="http://europe.bourges.univ-orleans.fr/sites/default/files/download/Ontology/Core/kernel.owl#carries"/>
    </owl:ObjectProperty>
    


    <!-- http://europe.bourges.univ-orleans.fr/sites/default/files/download/Ontology/Core/kernel.owl#isCodedIn -->

    <owl:ObjectProperty rdf:about="http://europe.bourges.univ-orleans.fr/sites/default/files/download/Ontology/Core/kernel.owl#isCodedIn">
        <rdfs:comment xml:lang="en">An abstraction is translated to be interpretable by a machine trough the Data concept.</rdfs:comment>
        <rdfs:domain rdf:resource="http://europe.bourges.univ-orleans.fr/sites/default/files/download/Ontology/Core/kernel.owl#Abstraction"/>
        <rdfs:range rdf:resource="http://europe.bourges.univ-orleans.fr/sites/default/files/download/Ontology/Core/kernel.owl#Data"/>
        <owl:inverseOf rdf:resource="http://europe.bourges.univ-orleans.fr/sites/default/files/download/Ontology/Core/kernel.owl#implements"/>
    </owl:ObjectProperty>
    


    <!-- http://europe.bourges.univ-orleans.fr/sites/default/files/download/Ontology/Core/kernel.owl#isDefinedBy -->

    <owl:ObjectProperty rdf:about="http://europe.bourges.univ-orleans.fr/sites/default/files/download/Ontology/Core/kernel.owl#isDefinedBy">
        <rdfs:comment xml:lang="en">A finite state machine is defined by a set of states, a set of transitions and events.</rdfs:comment>
        <rdfs:domain rdf:resource="http://europe.bourges.univ-orleans.fr/sites/default/files/download/Ontology/Core/kernel.owl#StateMachine"/>
        <rdfs:range>
            <owl:Class>
                <owl:unionOf rdf:parseType="Collection">
                    <rdf:Description rdf:about="http://europe.bourges.univ-orleans.fr/sites/default/files/download/Ontology/Core/kernel.owl#AutomataState"/>
                    <rdf:Description rdf:about="http://europe.bourges.univ-orleans.fr/sites/default/files/download/Ontology/Core/kernel.owl#Event"/>
                    <rdf:Description rdf:about="http://europe.bourges.univ-orleans.fr/sites/default/files/download/Ontology/Core/kernel.owl#Transition"/>
                </owl:unionOf>
            </owl:Class>
        </rdfs:range>
    </owl:ObjectProperty>
    


    <!-- http://europe.bourges.univ-orleans.fr/sites/default/files/download/Ontology/Core/kernel.owl#isDefinedIn -->

    <owl:ObjectProperty rdf:about="http://europe.bourges.univ-orleans.fr/sites/default/files/download/Ontology/Core/kernel.owl#isDefinedIn">
        <owl:versionInfo rdf:datatype="&xsd;string">It is not functional.</owl:versionInfo>
        <rdfs:comment xml:lang="en">This link means that you can relate any referential to any oher one. It is not functional because a referential may be defined in several referentials.</rdfs:comment>
        <rdfs:range rdf:resource="http://europe.bourges.univ-orleans.fr/sites/default/files/download/Ontology/Core/kernel.owl#Frame"/>
        <rdfs:domain rdf:resource="http://europe.bourges.univ-orleans.fr/sites/default/files/download/Ontology/Core/kernel.owl#Frame"/>
    </owl:ObjectProperty>
    


    <!-- http://europe.bourges.univ-orleans.fr/sites/default/files/download/Ontology/Core/kernel.owl#isDownstreamPortOf -->

    <owl:ObjectProperty rdf:about="http://europe.bourges.univ-orleans.fr/sites/default/files/download/Ontology/Core/kernel.owl#isDownstreamPortOf">
        <rdf:type rdf:resource="&owl;InverseFunctionalProperty"/>
        <rdfs:comment xml:lang="en">A port has incoming connectors.</rdfs:comment>
        <rdfs:range rdf:resource="http://europe.bourges.univ-orleans.fr/sites/default/files/download/Ontology/Core/kernel.owl#Connector"/>
        <rdfs:domain rdf:resource="http://europe.bourges.univ-orleans.fr/sites/default/files/download/Ontology/Core/kernel.owl#Port"/>
        <owl:inverseOf rdf:resource="http://europe.bourges.univ-orleans.fr/sites/default/files/download/Ontology/Core/kernel.owl#hasDownstreamPort"/>
        <rdfs:subPropertyOf rdf:resource="http://europe.bourges.univ-orleans.fr/sites/default/files/download/Ontology/Core/kernel.owl#isPropertyOf"/>
    </owl:ObjectProperty>
    


    <!-- http://europe.bourges.univ-orleans.fr/sites/default/files/download/Ontology/Core/kernel.owl#isEmittedOn -->

    <owl:ObjectProperty rdf:about="http://europe.bourges.univ-orleans.fr/sites/default/files/download/Ontology/Core/kernel.owl#isEmittedOn">
        <rdfs:comment xml:lang="en">An interaction is emitted by a system through a port</rdfs:comment>
        <rdfs:domain rdf:resource="http://europe.bourges.univ-orleans.fr/sites/default/files/download/Ontology/Core/kernel.owl#Interaction"/>
        <rdfs:range rdf:resource="http://europe.bourges.univ-orleans.fr/sites/default/files/download/Ontology/Core/kernel.owl#Port"/>
        <owl:inverseOf rdf:resource="http://europe.bourges.univ-orleans.fr/sites/default/files/download/Ontology/Core/kernel.owl#emits"/>
    </owl:ObjectProperty>
    


    <!-- http://europe.bourges.univ-orleans.fr/sites/default/files/download/Ontology/Core/kernel.owl#isModelledBy -->

    <owl:ObjectProperty rdf:about="http://europe.bourges.univ-orleans.fr/sites/default/files/download/Ontology/Core/kernel.owl#isModelledBy">
        <rdfs:comment xml:lang="en">This property expresses the fact that there exists at least one system to model the system considered</rdfs:comment>
        <rdfs:domain rdf:resource="http://europe.bourges.univ-orleans.fr/sites/default/files/download/Ontology/Core/kernel.owl#System"/>
        <rdfs:range rdf:resource="http://europe.bourges.univ-orleans.fr/sites/default/files/download/Ontology/Core/kernel.owl#System"/>
    </owl:ObjectProperty>
    


    <!-- http://europe.bourges.univ-orleans.fr/sites/default/files/download/Ontology/Core/kernel.owl#isPerformedBy -->

    <owl:ObjectProperty rdf:about="http://europe.bourges.univ-orleans.fr/sites/default/files/download/Ontology/Core/kernel.owl#isPerformedBy">
        <rdfs:comment xml:lang="en">An action is necessarily carried out by an agent.</rdfs:comment>
        <rdfs:domain rdf:resource="http://europe.bourges.univ-orleans.fr/sites/default/files/download/Ontology/Core/kernel.owl#Action"/>
        <rdfs:range rdf:resource="http://europe.bourges.univ-orleans.fr/sites/default/files/download/Ontology/Core/kernel.owl#Agent"/>
    </owl:ObjectProperty>
    


    <!-- http://europe.bourges.univ-orleans.fr/sites/default/files/download/Ontology/Core/kernel.owl#isPortOf -->

    <owl:ObjectProperty rdf:about="http://europe.bourges.univ-orleans.fr/sites/default/files/download/Ontology/Core/kernel.owl#isPortOf">
        <rdf:type rdf:resource="&owl;FunctionalProperty"/>
        <rdfs:comment xml:lang="en">Property to qualify the fact that a port belongs to one and only one system.</rdfs:comment>
        <rdfs:domain rdf:resource="http://europe.bourges.univ-orleans.fr/sites/default/files/download/Ontology/Core/kernel.owl#Port"/>
        <rdfs:range rdf:resource="http://europe.bourges.univ-orleans.fr/sites/default/files/download/Ontology/Core/kernel.owl#System"/>
        <owl:inverseOf rdf:resource="http://europe.bourges.univ-orleans.fr/sites/default/files/download/Ontology/Core/kernel.owl#hasPort"/>
        <rdfs:subPropertyOf rdf:resource="http://europe.bourges.univ-orleans.fr/sites/default/files/download/Ontology/Core/kernel.owl#isPropertyOf"/>
    </owl:ObjectProperty>
    


    <!-- http://europe.bourges.univ-orleans.fr/sites/default/files/download/Ontology/Core/kernel.owl#isPositionedIn -->

    <owl:ObjectProperty rdf:about="http://europe.bourges.univ-orleans.fr/sites/default/files/download/Ontology/Core/kernel.owl#isPositionedIn">
        <owl:versionInfo xml:lang="en">The fact that the referential defined by the object can not be the referential it is positioned in is expressed by a SWRL rule in proteus.owl.</owl:versionInfo>
        <rdfs:comment xml:lang="en">any physical object can be positioned at the very least in the environment referential. There is no meaning to position the object in its proper referential.</rdfs:comment>
        <rdfs:range rdf:resource="http://europe.bourges.univ-orleans.fr/sites/default/files/download/Ontology/Core/kernel.owl#Frame"/>
        <rdfs:domain rdf:resource="http://europe.bourges.univ-orleans.fr/sites/default/files/download/Ontology/Core/kernel.owl#PhysicalObject"/>
    </owl:ObjectProperty>
    


    <!-- http://europe.bourges.univ-orleans.fr/sites/default/files/download/Ontology/Core/kernel.owl#isProbeOf -->

    <owl:ObjectProperty rdf:about="http://europe.bourges.univ-orleans.fr/sites/default/files/download/Ontology/Core/kernel.owl#isProbeOf">
        <rdfs:comment xml:lang="en">This allow to know to which system is associated a probe</rdfs:comment>
        <rdfs:domain rdf:resource="http://europe.bourges.univ-orleans.fr/sites/default/files/download/Ontology/Core/kernel.owl#Probe"/>
        <rdfs:range rdf:resource="http://europe.bourges.univ-orleans.fr/sites/default/files/download/Ontology/Core/kernel.owl#System"/>
        <rdfs:subPropertyOf rdf:resource="http://europe.bourges.univ-orleans.fr/sites/default/files/download/Ontology/Core/kernel.owl#isPropertyOf"/>
    </owl:ObjectProperty>
    


    <!-- http://europe.bourges.univ-orleans.fr/sites/default/files/download/Ontology/Core/kernel.owl#isProducedBy -->

    <owl:ObjectProperty rdf:about="http://europe.bourges.univ-orleans.fr/sites/default/files/download/Ontology/Core/kernel.owl#isProducedBy">
        <rdfs:comment xml:lang="en">an event is produced by a particular state of a system.</rdfs:comment>
        <author xml:lang="en">creation PROTEUS consortium - 
modified Bruno Patin - 05/10/2013
- name has been changed from is TriggeredBy to is ProducedBy (trigger is associated to interaction and not event)</author>
        <rdfs:domain rdf:resource="http://europe.bourges.univ-orleans.fr/sites/default/files/download/Ontology/Core/kernel.owl#Event"/>
        <rdfs:range rdf:resource="http://europe.bourges.univ-orleans.fr/sites/default/files/download/Ontology/Core/kernel.owl#State"/>
    </owl:ObjectProperty>
    


    <!-- http://europe.bourges.univ-orleans.fr/sites/default/files/download/Ontology/Core/kernel.owl#isPropertyOf -->

    <owl:ObjectProperty rdf:about="http://europe.bourges.univ-orleans.fr/sites/default/files/download/Ontology/Core/kernel.owl#isPropertyOf">
        <rdfs:comment xml:lang="en">Things are properties of things.</rdfs:comment>
    </owl:ObjectProperty>
    


    <!-- http://europe.bourges.univ-orleans.fr/sites/default/files/download/Ontology/Core/kernel.owl#isReceivedOn -->

    <owl:ObjectProperty rdf:about="http://europe.bourges.univ-orleans.fr/sites/default/files/download/Ontology/Core/kernel.owl#isReceivedOn">
        <rdfs:comment xml:lang="en">An interaction is received by a system through a port</rdfs:comment>
        <rdfs:domain rdf:resource="http://europe.bourges.univ-orleans.fr/sites/default/files/download/Ontology/Core/kernel.owl#Interaction"/>
        <rdfs:range rdf:resource="http://europe.bourges.univ-orleans.fr/sites/default/files/download/Ontology/Core/kernel.owl#Port"/>
    </owl:ObjectProperty>
    


    <!-- http://europe.bourges.univ-orleans.fr/sites/default/files/download/Ontology/Core/kernel.owl#isTheSupport -->

    <owl:ObjectProperty rdf:about="http://europe.bourges.univ-orleans.fr/sites/default/files/download/Ontology/Core/kernel.owl#isTheSupport">
        <rdfs:comment xml:lang="en">Ports support the emission/reception of interactions</rdfs:comment>
        <rdfs:range rdf:resource="http://europe.bourges.univ-orleans.fr/sites/default/files/download/Ontology/Core/kernel.owl#Interaction"/>
        <rdfs:domain rdf:resource="http://europe.bourges.univ-orleans.fr/sites/default/files/download/Ontology/Core/kernel.owl#Port"/>
    </owl:ObjectProperty>
    


    <!-- http://europe.bourges.univ-orleans.fr/sites/default/files/download/Ontology/Core/kernel.owl#isTriggeredBy -->

    <owl:ObjectProperty rdf:about="http://europe.bourges.univ-orleans.fr/sites/default/files/download/Ontology/Core/kernel.owl#isTriggeredBy">
        <rdfs:comment xml:lang="en">Not to be deleted as the inverse of tirggers property IS NOT impacts</rdfs:comment>
        <rdfs:domain rdf:resource="http://europe.bourges.univ-orleans.fr/sites/default/files/download/Ontology/Core/kernel.owl#Interaction"/>
        <rdfs:range rdf:resource="http://europe.bourges.univ-orleans.fr/sites/default/files/download/Ontology/Core/kernel.owl#System"/>
        <owl:inverseOf rdf:resource="http://europe.bourges.univ-orleans.fr/sites/default/files/download/Ontology/Core/kernel.owl#triggers"/>
    </owl:ObjectProperty>
    


    <!-- http://europe.bourges.univ-orleans.fr/sites/default/files/download/Ontology/Core/kernel.owl#isUpstreamPortOf -->

    <owl:ObjectProperty rdf:about="http://europe.bourges.univ-orleans.fr/sites/default/files/download/Ontology/Core/kernel.owl#isUpstreamPortOf">
        <rdf:type rdf:resource="&owl;InverseFunctionalProperty"/>
        <rdfs:comment xml:lang="en">A port has exiting connectors.</rdfs:comment>
        <rdfs:range rdf:resource="http://europe.bourges.univ-orleans.fr/sites/default/files/download/Ontology/Core/kernel.owl#Connector"/>
        <rdfs:domain rdf:resource="http://europe.bourges.univ-orleans.fr/sites/default/files/download/Ontology/Core/kernel.owl#Port"/>
        <owl:inverseOf rdf:resource="http://europe.bourges.univ-orleans.fr/sites/default/files/download/Ontology/Core/kernel.owl#hasUpstreamPort"/>
        <rdfs:subPropertyOf rdf:resource="http://europe.bourges.univ-orleans.fr/sites/default/files/download/Ontology/Core/kernel.owl#isPropertyOf"/>
    </owl:ObjectProperty>
    


    <!-- http://europe.bourges.univ-orleans.fr/sites/default/files/download/Ontology/Core/kernel.owl#isUsedBy -->

    <owl:ObjectProperty rdf:about="http://europe.bourges.univ-orleans.fr/sites/default/files/download/Ontology/Core/kernel.owl#isUsedBy">
        <rdfs:comment xml:lang="en">Information can be used by System. This property IS NOT a isPropertyOf sub property because an information that is used can be discarded after being used and the isPropertyOf property tags a static property of the concept that cannot exist or is different w/o the property described.</rdfs:comment>
        <author xml:lang="en">created PROTEUS Consortium - 
modified Bruno Patin - 25/07/2014
- TODO deleted
- comment updated</author>
        <rdfs:domain rdf:resource="http://europe.bourges.univ-orleans.fr/sites/default/files/download/Ontology/Core/kernel.owl#Information"/>
        <rdfs:range rdf:resource="http://europe.bourges.univ-orleans.fr/sites/default/files/download/Ontology/Core/kernel.owl#System"/>
        <owl:inverseOf rdf:resource="http://europe.bourges.univ-orleans.fr/sites/default/files/download/Ontology/Core/kernel.owl#uses"/>
        <rdfs:subPropertyOf rdf:resource="&owl;topObjectProperty"/>
    </owl:ObjectProperty>
    


    <!-- http://europe.bourges.univ-orleans.fr/sites/default/files/download/Ontology/Core/kernel.owl#keepsTrackOfTime -->

    <owl:ObjectProperty rdf:about="http://europe.bourges.univ-orleans.fr/sites/default/files/download/Ontology/Core/kernel.owl#keepsTrackOfTime">
        <rdf:type rdf:resource="&owl;FunctionalProperty"/>
        <owl:versionInfo rdf:datatype="&xsd;string">We do not organize the property under things like roboticians properties. Only one kind of viewpoint is modelled.</owl:versionInfo>
        <rdfs:comment xml:lang="en">This property expresses the fact that every hardware do need some way to provide a clock to its included software in order for it to live. This clock relies on the time of the physical object it lives in.</rdfs:comment>
        <rdfs:domain rdf:resource="http://europe.bourges.univ-orleans.fr/sites/default/files/download/Ontology/Core/kernel.owl#Clock"/>
        <rdfs:range rdf:resource="http://europe.bourges.univ-orleans.fr/sites/default/files/download/Ontology/Core/kernel.owl#Time"/>
    </owl:ObjectProperty>
    


    <!-- http://europe.bourges.univ-orleans.fr/sites/default/files/download/Ontology/Core/kernel.owl#managesFileSystem -->

    <owl:ObjectProperty rdf:about="http://europe.bourges.univ-orleans.fr/sites/default/files/download/Ontology/Core/kernel.owl#managesFileSystem">
        <rdfs:comment xml:lang="en">An operating system manages (update, write, read, ...) the file system and the information stored within.</rdfs:comment>
        <rdfs:range rdf:resource="http://europe.bourges.univ-orleans.fr/sites/default/files/download/Ontology/Core/kernel.owl#FileSystem"/>
        <rdfs:domain rdf:resource="http://europe.bourges.univ-orleans.fr/sites/default/files/download/Ontology/Core/kernel.owl#OperatingSystem"/>
    </owl:ObjectProperty>
    


    <!-- http://europe.bourges.univ-orleans.fr/sites/default/files/download/Ontology/Core/kernel.owl#models -->

    <owl:ObjectProperty rdf:about="http://europe.bourges.univ-orleans.fr/sites/default/files/download/Ontology/Core/kernel.owl#models">
        <rdfs:comment xml:lang="en">This property expresses the fact that a system can model another one as well as an evolution model. It is what we do when, considering reality or a first layer of reality, we model it. What is said here is that reality IS a system and that each time we want to represent it we use a system description to do just that.</rdfs:comment>
        <rdfs:domain rdf:resource="http://europe.bourges.univ-orleans.fr/sites/default/files/download/Ontology/Core/kernel.owl#System"/>
        <owl:inverseOf rdf:resource="http://europe.bourges.univ-orleans.fr/sites/default/files/download/Ontology/Core/kernel.owl#isModelledBy"/>
        <rdfs:range>
            <owl:Class>
                <owl:unionOf rdf:parseType="Collection">
                    <rdf:Description rdf:about="http://europe.bourges.univ-orleans.fr/sites/default/files/download/Ontology/Core/kernel.owl#Evolution"/>
                    <rdf:Description rdf:about="http://europe.bourges.univ-orleans.fr/sites/default/files/download/Ontology/Core/kernel.owl#System"/>
                </owl:unionOf>
            </owl:Class>
        </rdfs:range>
    </owl:ObjectProperty>
    


    <!-- http://europe.bourges.univ-orleans.fr/sites/default/files/download/Ontology/Core/kernel.owl#observes -->

    <owl:ObjectProperty rdf:about="http://europe.bourges.univ-orleans.fr/sites/default/files/download/Ontology/Core/kernel.owl#observes">
        <rdfs:comment xml:lang="en">this property expresses the capability to extract information from a state.</rdfs:comment>
        <rdfs:domain rdf:resource="http://europe.bourges.univ-orleans.fr/sites/default/files/download/Ontology/Core/kernel.owl#Probe"/>
        <rdfs:range rdf:resource="http://europe.bourges.univ-orleans.fr/sites/default/files/download/Ontology/Core/kernel.owl#State"/>
    </owl:ObjectProperty>
    


    <!-- http://europe.bourges.univ-orleans.fr/sites/default/files/download/Ontology/Core/kernel.owl#produces -->

    <owl:ObjectProperty rdf:about="http://europe.bourges.univ-orleans.fr/sites/default/files/download/Ontology/Core/kernel.owl#produces">
        <rdfs:comment xml:lang="en">probes produce information thanks to observation of States</rdfs:comment>
        <rdfs:range rdf:resource="http://europe.bourges.univ-orleans.fr/sites/default/files/download/Ontology/Core/kernel.owl#Information"/>
        <rdfs:domain rdf:resource="http://europe.bourges.univ-orleans.fr/sites/default/files/download/Ontology/Core/kernel.owl#Probe"/>
    </owl:ObjectProperty>
    


    <!-- http://europe.bourges.univ-orleans.fr/sites/default/files/download/Ontology/Core/kernel.owl#receives -->

    <owl:ObjectProperty rdf:about="http://europe.bourges.univ-orleans.fr/sites/default/files/download/Ontology/Core/kernel.owl#receives">
        <rdfs:comment xml:lang="en">Ports receive interactions</rdfs:comment>
        <rdfs:range rdf:resource="http://europe.bourges.univ-orleans.fr/sites/default/files/download/Ontology/Core/kernel.owl#Interaction"/>
        <rdfs:domain rdf:resource="http://europe.bourges.univ-orleans.fr/sites/default/files/download/Ontology/Core/kernel.owl#Port"/>
        <owl:inverseOf rdf:resource="http://europe.bourges.univ-orleans.fr/sites/default/files/download/Ontology/Core/kernel.owl#isReceivedOn"/>
    </owl:ObjectProperty>
    


    <!-- http://europe.bourges.univ-orleans.fr/sites/default/files/download/Ontology/Core/kernel.owl#startsFrom -->

    <owl:ObjectProperty rdf:about="http://europe.bourges.univ-orleans.fr/sites/default/files/download/Ontology/Core/kernel.owl#startsFrom">
        <rdfs:comment xml:lang="en">A finite state machine has an initial state</rdfs:comment>
        <rdfs:range rdf:resource="http://europe.bourges.univ-orleans.fr/sites/default/files/download/Ontology/Core/kernel.owl#AutomataInitialState"/>
        <rdfs:domain rdf:resource="http://europe.bourges.univ-orleans.fr/sites/default/files/download/Ontology/Core/kernel.owl#StateMachine"/>
    </owl:ObjectProperty>
    


    <!-- http://europe.bourges.univ-orleans.fr/sites/default/files/download/Ontology/Core/kernel.owl#systemSource -->

    <owl:ObjectProperty rdf:about="http://europe.bourges.univ-orleans.fr/sites/default/files/download/Ontology/Core/kernel.owl#systemSource">
        <rdfs:comment xml:lang="en">This property allows the interaction to know which system triggered the interaction.</rdfs:comment>
        <rdfs:domain rdf:resource="http://europe.bourges.univ-orleans.fr/sites/default/files/download/Ontology/Core/kernel.owl#Interaction"/>
        <rdfs:range rdf:resource="http://europe.bourges.univ-orleans.fr/sites/default/files/download/Ontology/Core/kernel.owl#System"/>
    </owl:ObjectProperty>
    


    <!-- http://europe.bourges.univ-orleans.fr/sites/default/files/download/Ontology/Core/kernel.owl#takesAsInput -->

    <owl:ObjectProperty rdf:about="http://europe.bourges.univ-orleans.fr/sites/default/files/download/Ontology/Core/kernel.owl#takesAsInput">
        <rdfs:comment xml:lang="en">An evolution model has several inputs to process and evaluate which would be the corresponding evolution and destination state in a potential transition.

We can list the general inputs:
* InputState
* InputPort Value

Note that time dependency (InputTime) is taken into account through a specific relation: isAFunctionOfTime</rdfs:comment>
        <rdfs:domain rdf:resource="http://europe.bourges.univ-orleans.fr/sites/default/files/download/Ontology/Core/kernel.owl#Evolution"/>
        <rdfs:range>
            <owl:Class>
                <owl:unionOf rdf:parseType="Collection">
                    <rdf:Description rdf:about="http://europe.bourges.univ-orleans.fr/sites/default/files/download/Ontology/Core/kernel.owl#Port"/>
                    <rdf:Description rdf:about="http://europe.bourges.univ-orleans.fr/sites/default/files/download/Ontology/Core/kernel.owl#State"/>
                </owl:unionOf>
            </owl:Class>
        </rdfs:range>
    </owl:ObjectProperty>
    


    <!-- http://europe.bourges.univ-orleans.fr/sites/default/files/download/Ontology/Core/kernel.owl#to -->

    <owl:ObjectProperty rdf:about="http://europe.bourges.univ-orleans.fr/sites/default/files/download/Ontology/Core/kernel.owl#to">
        <rdfs:comment xml:lang="en">A transition is defined by a start state and an end state</rdfs:comment>
        <rdfs:range rdf:resource="http://europe.bourges.univ-orleans.fr/sites/default/files/download/Ontology/Core/kernel.owl#AutomataState"/>
        <rdfs:domain rdf:resource="http://europe.bourges.univ-orleans.fr/sites/default/files/download/Ontology/Core/kernel.owl#Transition"/>
    </owl:ObjectProperty>
    


    <!-- http://europe.bourges.univ-orleans.fr/sites/default/files/download/Ontology/Core/kernel.owl#transmitInformation -->

    <owl:ObjectProperty rdf:about="http://europe.bourges.univ-orleans.fr/sites/default/files/download/Ontology/Core/kernel.owl#transmitInformation">
        <rdfs:comment xml:lang="en">An interaction allows transitting information.</rdfs:comment>
        <rdfs:range rdf:resource="http://europe.bourges.univ-orleans.fr/sites/default/files/download/Ontology/Core/kernel.owl#Information"/>
        <rdfs:domain rdf:resource="http://europe.bourges.univ-orleans.fr/sites/default/files/download/Ontology/Core/kernel.owl#Interaction"/>
    </owl:ObjectProperty>
    


    <!-- http://europe.bourges.univ-orleans.fr/sites/default/files/download/Ontology/Core/kernel.owl#triggers -->

    <owl:ObjectProperty rdf:about="http://europe.bourges.univ-orleans.fr/sites/default/files/download/Ontology/Core/kernel.owl#triggers">
        <author xml:lang="en">creation PROTEUS consortium - 
modified Bruno Patin - 05/10/2013
- triggers is now the inverse of impacts</author>
        <rdfs:comment xml:lang="en">it is the property that will allow the interaction  through its evolution model to change the interaction state.</rdfs:comment>
        <TODO xml:lang="en">the only dynamicity of the interaction is its triggering by the system. To animate an interaction has no meaning. Evolution animates system that triggers interaction.</TODO>
        <rdfs:range rdf:resource="http://europe.bourges.univ-orleans.fr/sites/default/files/download/Ontology/Core/kernel.owl#Interaction"/>
        <rdfs:domain rdf:resource="http://europe.bourges.univ-orleans.fr/sites/default/files/download/Ontology/Core/kernel.owl#System"/>
    </owl:ObjectProperty>
    


    <!-- http://europe.bourges.univ-orleans.fr/sites/default/files/download/Ontology/Core/kernel.owl#uses -->

    <owl:ObjectProperty rdf:about="http://europe.bourges.univ-orleans.fr/sites/default/files/download/Ontology/Core/kernel.owl#uses">
        <rdfs:comment xml:lang="en">Systems needs information internally in order to work properly. At the most generic level, we do not need to know anything with respect to these internal information but in some cases this becomes an important point.</rdfs:comment>
        <rdfs:range rdf:resource="http://europe.bourges.univ-orleans.fr/sites/default/files/download/Ontology/Core/kernel.owl#Information"/>
        <rdfs:domain rdf:resource="http://europe.bourges.univ-orleans.fr/sites/default/files/download/Ontology/Core/kernel.owl#System"/>
        <rdfs:subPropertyOf rdf:resource="&owl;topObjectProperty"/>
    </owl:ObjectProperty>
    


    <!-- http://europe.bourges.univ-orleans.fr/sites/default/files/download/Ontology/Core/kernel.owl#wraps -->

    <owl:ObjectProperty rdf:about="http://europe.bourges.univ-orleans.fr/sites/default/files/download/Ontology/Core/kernel.owl#wraps">
        <rdfs:comment xml:lang="en">This means that the wrapper translates the dataflow from / to the two linked software.</rdfs:comment>
        <author xml:lang="en">creation PROTEUS Consortium
modified Bruno Patin - 09/10/2013
- due to reorganisation of software concept, wrapper wraps software and no more only Applications</author>
        <rdfs:range rdf:resource="http://europe.bourges.univ-orleans.fr/sites/default/files/download/Ontology/Core/kernel.owl#Software"/>
        <rdfs:domain rdf:resource="http://europe.bourges.univ-orleans.fr/sites/default/files/download/Ontology/Core/kernel.owl#Wrapper"/>
    </owl:ObjectProperty>
    


    <!-- 
    ///////////////////////////////////////////////////////////////////////////////////////
    //
    // Data properties
    //
    ///////////////////////////////////////////////////////////////////////////////////////
     -->

    


    <!-- http://europe.bourges.univ-orleans.fr/sites/default/files/download/Ontology/Core/kernel.owl#isAtomic -->

    <owl:DatatypeProperty rdf:about="http://europe.bourges.univ-orleans.fr/sites/default/files/download/Ontology/Core/kernel.owl#isAtomic">
        <rdfs:comment xml:lang="en">A system is either atomic or composed. An atomic system do not aggregates other systems.</rdfs:comment>
        <rdfs:domain rdf:resource="http://europe.bourges.univ-orleans.fr/sites/default/files/download/Ontology/Core/kernel.owl#System"/>
        <rdfs:range>
            <rdfs:Datatype>
                <owl:oneOf>
                    <rdf:Description>
                        <rdf:type rdf:resource="&rdf;List"/>
                        <rdf:first rdf:datatype="&xsd;boolean">false</rdf:first>
                        <rdf:rest>
                            <rdf:Description>
                                <rdf:type rdf:resource="&rdf;List"/>
                                <rdf:first rdf:datatype="&xsd;boolean">true</rdf:first>
                                <rdf:rest rdf:resource="&rdf;nil"/>
                            </rdf:Description>
                        </rdf:rest>
                    </rdf:Description>
                </owl:oneOf>
            </rdfs:Datatype>
        </rdfs:range>
    </owl:DatatypeProperty>
    


    <!-- http://europe.bourges.univ-orleans.fr/sites/default/files/download/Ontology/Core/kernel.owl#isIn_Out -->

    <owl:DatatypeProperty rdf:about="http://europe.bourges.univ-orleans.fr/sites/default/files/download/Ontology/Core/kernel.owl#isIn_Out">
        <rdfs:comment xml:lang="en">indicates the port type in terms of &quot;in&quot; or &quot;out&quot; or  &quot;in and out&quot; (in-out value) port.</rdfs:comment>
        <rdfs:domain rdf:resource="http://europe.bourges.univ-orleans.fr/sites/default/files/download/Ontology/Core/kernel.owl#Port"/>
        <rdfs:range>
            <rdfs:Datatype>
                <owl:oneOf>
                    <rdf:Description>
                        <rdf:type rdf:resource="&rdf;List"/>
                        <rdf:first rdf:datatype="&xsd;string">in</rdf:first>
                        <rdf:rest>
                            <rdf:Description>
                                <rdf:type rdf:resource="&rdf;List"/>
                                <rdf:first rdf:datatype="&xsd;string">out</rdf:first>
                                <rdf:rest rdf:resource="&rdf;nil"/>
                            </rdf:Description>
                        </rdf:rest>
                    </rdf:Description>
                </owl:oneOf>
            </rdfs:Datatype>
        </rdfs:range>
    </owl:DatatypeProperty>
    


    <!-- http://europe.bourges.univ-orleans.fr/sites/default/files/download/Ontology/Core/kernel.owl#occursAfterDuration -->

    <owl:DatatypeProperty rdf:about="http://europe.bourges.univ-orleans.fr/sites/default/files/download/Ontology/Core/kernel.owl#occursAfterDuration">
        <rdf:type rdf:resource="&owl;FunctionalProperty"/>
        <rdfs:comment xml:lang="en">A time event occurs after a duration.</rdfs:comment>
        <rdfs:domain rdf:resource="http://europe.bourges.univ-orleans.fr/sites/default/files/download/Ontology/Core/kernel.owl#TimeEvent"/>
        <rdfs:range rdf:resource="&xsd;dateTime"/>
    </owl:DatatypeProperty>
    


    <!-- http://europe.bourges.univ-orleans.fr/sites/default/files/download/Ontology/Core/kernel.owl#valued -->

    <owl:DatatypeProperty rdf:about="http://europe.bourges.univ-orleans.fr/sites/default/files/download/Ontology/Core/kernel.owl#valued">
        <rdfs:comment rdf:datatype="&xsd;string">Protégé primitive value for Primitive data</rdfs:comment>
        <rdfs:subPropertyOf rdf:resource="&owl;topDataProperty"/>
    </owl:DatatypeProperty>
    


    <!-- 
    ///////////////////////////////////////////////////////////////////////////////////////
    //
    // Classes
    //
    ///////////////////////////////////////////////////////////////////////////////////////
     -->

    


    <!-- http://europe.bourges.univ-orleans.fr/sites/default/files/download/Ontology/Core/kernel.owl#Abstraction -->

    <owl:Class rdf:about="http://europe.bourges.univ-orleans.fr/sites/default/files/download/Ontology/Core/kernel.owl#Abstraction">
        <rdfs:subClassOf rdf:resource="http://europe.bourges.univ-orleans.fr/sites/default/files/download/Ontology/Core/kernel.owl#Information"/>
        <owl:disjointWith rdf:resource="http://europe.bourges.univ-orleans.fr/sites/default/files/download/Ontology/Core/kernel.owl#Data"/>
        <openCycURI rdf:datatype="&xsd;anyURI">http://sw.opencyc.org/concept/Mx4r0EwZ9r8aEdmAAAACs6hRjg</openCycURI>
        <rdfs:comment xml:lang="en">Abstraction is an information that is disembodied. It means that there are no representation or, more to the point, that there is no interest to consider the concerned representation. The representation we are discussing is in the Data concept through the &quot;implements&quot; property.

The OpenCyc and wikipedia concepts referenced are more generic as an abstraction is the set of common characteristics a set of things shares. There is no object that is The abstraction.

The Abstraction concept here mentionned is closer to the ideas world of Plato.</rdfs:comment>
    </owl:Class>
    


    <!-- http://europe.bourges.univ-orleans.fr/sites/default/files/download/Ontology/Core/kernel.owl#Action -->

    <owl:Class rdf:about="http://europe.bourges.univ-orleans.fr/sites/default/files/download/Ontology/Core/kernel.owl#Action">
        <owl:equivalentClass>
            <owl:Class>
                <owl:unionOf rdf:parseType="Collection">
                    <rdf:Description rdf:about="http://europe.bourges.univ-orleans.fr/sites/default/files/download/Ontology/Core/kernel.owl#DriverToHardwareInteraction"/>
                    <rdf:Description rdf:about="http://europe.bourges.univ-orleans.fr/sites/default/files/download/Ontology/Core/kernel.owl#PhysicalInteraction"/>
                </owl:unionOf>
            </owl:Class>
        </owl:equivalentClass>
        <rdfs:subClassOf rdf:resource="http://europe.bourges.univ-orleans.fr/sites/default/files/download/Ontology/Core/kernel.owl#Interaction"/>
        <owl:disjointWith rdf:resource="http://europe.bourges.univ-orleans.fr/sites/default/files/download/Ontology/Core/kernel.owl#HardwareToDriverInteraction"/>
        <openCycURI rdf:datatype="&xsd;anyURI">http://sw.opencyc.org/concept/Mx4rvVieP5wpEbGdrcN5Y29ycA</openCycURI>
        <rdfs:comment xml:lang="en">An action is a specific kind of interaction. Actions are performed by agents that are either robots or humans. For robots, actions are performed on external world (driver to hardware interaction) or on internal components (driver to software  interaction). For humans, actions are only physical interaction because the ontology does not describe psychology. 

Notice that it exists driver to hardware interactions and software to software interactions that are not actions but only dataflow.

Action in the Ontology is equivalent to the OpenCyc PurposefulAction.</rdfs:comment>
        <author xml:lang="en">creation PROTEUS consortium - 
modified Bruno Patin - 03/10/2013
- rule added to express the fact that only human and robot (Agent) can interact using actions
- equivalence established between action and (Physical or DriverToHardware)Interaction</author>
    </owl:Class>
    


    <!-- http://europe.bourges.univ-orleans.fr/sites/default/files/download/Ontology/Core/kernel.owl#Activity -->

    <owl:Class rdf:about="http://europe.bourges.univ-orleans.fr/sites/default/files/download/Ontology/Core/kernel.owl#Activity">
        <owl:disjointWith rdf:resource="http://europe.bourges.univ-orleans.fr/sites/default/files/download/Ontology/Core/kernel.owl#Connector"/>
        <owl:disjointWith rdf:resource="http://europe.bourges.univ-orleans.fr/sites/default/files/download/Ontology/Core/kernel.owl#Event"/>
        <owl:disjointWith rdf:resource="http://europe.bourges.univ-orleans.fr/sites/default/files/download/Ontology/Core/kernel.owl#Evolution"/>
        <owl:disjointWith rdf:resource="http://europe.bourges.univ-orleans.fr/sites/default/files/download/Ontology/Core/kernel.owl#Frame"/>
        <owl:disjointWith rdf:resource="http://europe.bourges.univ-orleans.fr/sites/default/files/download/Ontology/Core/kernel.owl#Information"/>
        <owl:disjointWith rdf:resource="http://europe.bourges.univ-orleans.fr/sites/default/files/download/Ontology/Core/kernel.owl#Interaction"/>
        <owl:disjointWith rdf:resource="http://europe.bourges.univ-orleans.fr/sites/default/files/download/Ontology/Core/kernel.owl#Port"/>
        <owl:disjointWith rdf:resource="http://europe.bourges.univ-orleans.fr/sites/default/files/download/Ontology/Core/kernel.owl#Probe"/>
        <owl:disjointWith rdf:resource="http://europe.bourges.univ-orleans.fr/sites/default/files/download/Ontology/Core/kernel.owl#Protocol"/>
        <owl:disjointWith rdf:resource="http://europe.bourges.univ-orleans.fr/sites/default/files/download/Ontology/Core/kernel.owl#System"/>
        <owl:disjointWith rdf:resource="http://europe.bourges.univ-orleans.fr/sites/default/files/download/Ontology/Core/kernel.owl#Time"/>
        <owl:disjointWith rdf:resource="http://europe.bourges.univ-orleans.fr/sites/default/files/download/Ontology/Core/kernel.owl#Transition"/>
        <wikipediaURI rdf:datatype="&xsd;anyURI">http://en.wikipedia.org/wiki/Action_%28philosophy%29</wikipediaURI>
        <rdfs:comment xml:lang="en">An Activity is a set of Actions performed by an Agent. In the wikipedia definition activity is seen as action (theory of action).</rdfs:comment>
        <TODO xml:lang="en">What is the value of adding the activity concept in the kernel as it is linked to noting at all. The fact it composes actions is only syntaxic sugar and not something linked to the root concepts. Activity should be either moved or deleted.</TODO>
    </owl:Class>
    


    <!-- http://europe.bourges.univ-orleans.fr/sites/default/files/download/Ontology/Core/kernel.owl#Agent -->

    <owl:Class rdf:about="http://europe.bourges.univ-orleans.fr/sites/default/files/download/Ontology/Core/kernel.owl#Agent">
        <rdfs:subClassOf rdf:resource="http://europe.bourges.univ-orleans.fr/sites/default/files/download/Ontology/Core/kernel.owl#PhysicalObject"/>
        <rdfs:subClassOf>
            <owl:Restriction>
                <owl:onProperty rdf:resource="http://europe.bourges.univ-orleans.fr/sites/default/files/download/Ontology/Core/kernel.owl#triggers"/>
                <owl:someValuesFrom rdf:resource="http://europe.bourges.univ-orleans.fr/sites/default/files/download/Ontology/Core/kernel.owl#Action"/>
            </owl:Restriction>
        </rdfs:subClassOf>
        <rdfs:subClassOf>
            <owl:Restriction>
                <owl:onProperty rdf:resource="http://europe.bourges.univ-orleans.fr/sites/default/files/download/Ontology/Core/kernel.owl#currentlyPerforms"/>
                <owl:onClass rdf:resource="http://europe.bourges.univ-orleans.fr/sites/default/files/download/Ontology/Core/kernel.owl#Action"/>
                <owl:minQualifiedCardinality rdf:datatype="&xsd;nonNegativeInteger">0</owl:minQualifiedCardinality>
            </owl:Restriction>
        </rdfs:subClassOf>
        <owl:disjointWith rdf:resource="http://europe.bourges.univ-orleans.fr/sites/default/files/download/Ontology/Core/kernel.owl#Environment"/>
        <owl:disjointWith rdf:resource="http://europe.bourges.univ-orleans.fr/sites/default/files/download/Ontology/Core/kernel.owl#Hardware"/>
        <otherURI rdf:datatype="&xsd;anyURI">http://www.inf.ufrgs.br/prosoft/bdi4jade/?page_id=46</otherURI>
        <rdfs:comment xml:lang="en">A physical entity which is capable of action derived of its intentions themselves derived from its beliefs, such as robots, animals, human.
Link below presents the reference used.</rdfs:comment>
        <author xml:lang="en">creation PROTEUS Consortium - 
modified Bruno Patin - 16/09/2014
- introduction of one link to BDI agent
- addition on the comment</author>
    </owl:Class>
    


    <!-- http://europe.bourges.univ-orleans.fr/sites/default/files/download/Ontology/Core/kernel.owl#Animal -->

    <owl:Class rdf:about="http://europe.bourges.univ-orleans.fr/sites/default/files/download/Ontology/Core/kernel.owl#Animal">
        <rdfs:subClassOf rdf:resource="http://europe.bourges.univ-orleans.fr/sites/default/files/download/Ontology/Core/kernel.owl#AtomicSystem"/>
        <wikipediaURI rdf:datatype="&xsd;anyURI">http://en.wikipedia.org/wiki/Animal</wikipediaURI>
        <wiktionaryURI rdf:datatype="&xsd;anyURI">http://en.wiktionary.org/wiki/animal</wiktionaryURI>
        <openCycURI rdf:datatype="&xsd;anyURI">http://sw.opencyc.org/concept/Mx4rvViwMZwpEbGdrcN5Y29ycA</openCycURI>
        <rdfs:comment xml:lang="en">Animal are typically motile, living, whole organisms. Humans ARE animals.</rdfs:comment>
        <author xml:lang="en">Bruno Patin - 16/09/2014
- animal is introduced due to the fact you mobile with intentions and randomised actions that are not artefact</author>
    </owl:Class>
    


    <!-- http://europe.bourges.univ-orleans.fr/sites/default/files/download/Ontology/Core/kernel.owl#Application -->

    <owl:Class rdf:about="http://europe.bourges.univ-orleans.fr/sites/default/files/download/Ontology/Core/kernel.owl#Application">
        <rdfs:subClassOf rdf:resource="http://europe.bourges.univ-orleans.fr/sites/default/files/download/Ontology/Core/kernel.owl#Software"/>
        <owl:disjointWith rdf:resource="http://europe.bourges.univ-orleans.fr/sites/default/files/download/Ontology/Core/kernel.owl#SoftwareModule"/>
        <rdfs:comment xml:lang="en">It is a computing entity able to work upon a hardware that provides computing capcabilities.
It is a computing entity capable of providing life to another software. At the bottom level, it is the OS of the computer.</rdfs:comment>
    </owl:Class>
    


    <!-- http://europe.bourges.univ-orleans.fr/sites/default/files/download/Ontology/Core/kernel.owl#ApplicationInteraction -->

    <owl:Class rdf:about="http://europe.bourges.univ-orleans.fr/sites/default/files/download/Ontology/Core/kernel.owl#ApplicationInteraction">
        <rdfs:subClassOf rdf:resource="http://europe.bourges.univ-orleans.fr/sites/default/files/download/Ontology/Core/kernel.owl#Interaction"/>
        <rdfs:subClassOf>
            <owl:Restriction>
                <owl:onProperty rdf:resource="http://europe.bourges.univ-orleans.fr/sites/default/files/download/Ontology/Core/kernel.owl#impacts"/>
                <owl:allValuesFrom rdf:resource="http://europe.bourges.univ-orleans.fr/sites/default/files/download/Ontology/Core/kernel.owl#Software"/>
            </owl:Restriction>
        </rdfs:subClassOf>
        <owl:disjointWith rdf:resource="http://europe.bourges.univ-orleans.fr/sites/default/files/download/Ontology/Core/kernel.owl#DriverToHardwareInteraction"/>
        <owl:disjointWith rdf:resource="http://europe.bourges.univ-orleans.fr/sites/default/files/download/Ontology/Core/kernel.owl#HardwareToDriverInteraction"/>
        <owl:disjointWith rdf:resource="http://europe.bourges.univ-orleans.fr/sites/default/files/download/Ontology/Core/kernel.owl#PhysicalInteraction"/>
        <rdfs:comment xml:lang="en">Interaction between two software that are parts of an application. They could be interactions between frameworks, applications, libraries, drivers, processes, or other logical units of Application. In order to avoid redendancy the name does not quote two times the Aplication word</rdfs:comment>
    </owl:Class>
    


    <!-- http://europe.bourges.univ-orleans.fr/sites/default/files/download/Ontology/Core/kernel.owl#AtomicModel -->

    <owl:Class rdf:about="http://europe.bourges.univ-orleans.fr/sites/default/files/download/Ontology/Core/kernel.owl#AtomicModel">
        <rdfs:subClassOf rdf:resource="http://europe.bourges.univ-orleans.fr/sites/default/files/download/Ontology/Core/kernel.owl#AtomicSystem"/>
        <rdfs:subClassOf rdf:resource="http://europe.bourges.univ-orleans.fr/sites/default/files/download/Ontology/Core/kernel.owl#Model"/>
        <owl:disjointWith rdf:resource="http://europe.bourges.univ-orleans.fr/sites/default/files/download/Ontology/Core/kernel.owl#CompositeModel"/>
        <rdfs:comment xml:lang="en">This concept groups the different theory that can be used to model one or more system. It is often linnked to a mathematical theory. It also defines the &quot;external&quot; model concept meaning that the model exist, is provided but is only known through its interface.
An atomic system can models more than one system. It explains whay the properties models has cardinality more than one.
An atomic model beiing an atomic system is thus disjoint from a composite model as it is a composite system.</rdfs:comment>
    </owl:Class>
    


    <!-- http://europe.bourges.univ-orleans.fr/sites/default/files/download/Ontology/Core/kernel.owl#AtomicSystem -->

    <owl:Class rdf:about="http://europe.bourges.univ-orleans.fr/sites/default/files/download/Ontology/Core/kernel.owl#AtomicSystem">
        <rdfs:subClassOf rdf:resource="http://europe.bourges.univ-orleans.fr/sites/default/files/download/Ontology/Core/kernel.owl#System"/>
        <rdfs:subClassOf>
            <owl:Restriction>
                <owl:onProperty rdf:resource="http://europe.bourges.univ-orleans.fr/sites/default/files/download/Ontology/Core/kernel.owl#isAtomic"/>
                <owl:hasValue rdf:datatype="&xsd;boolean">true</owl:hasValue>
            </owl:Restriction>
        </rdfs:subClassOf>
        <owl:disjointWith rdf:resource="http://europe.bourges.univ-orleans.fr/sites/default/files/download/Ontology/Core/kernel.owl#CompositeSystem"/>
        <rdfs:comment xml:lang="en">An atomic system can&apos;t be split into parts.</rdfs:comment>
    </owl:Class>
    


    <!-- http://europe.bourges.univ-orleans.fr/sites/default/files/download/Ontology/Core/kernel.owl#AutomataEndState -->

    <owl:Class rdf:about="http://europe.bourges.univ-orleans.fr/sites/default/files/download/Ontology/Core/kernel.owl#AutomataEndState">
        <rdfs:subClassOf rdf:resource="http://europe.bourges.univ-orleans.fr/sites/default/files/download/Ontology/Core/kernel.owl#AutomataState"/>
        <owl:disjointWith rdf:resource="http://europe.bourges.univ-orleans.fr/sites/default/files/download/Ontology/Core/kernel.owl#AutomataInitialState"/>
        <rdfs:comment xml:lang="en">End state of a Finite State Machine</rdfs:comment>
    </owl:Class>
    


    <!-- http://europe.bourges.univ-orleans.fr/sites/default/files/download/Ontology/Core/kernel.owl#AutomataInitialState -->

    <owl:Class rdf:about="http://europe.bourges.univ-orleans.fr/sites/default/files/download/Ontology/Core/kernel.owl#AutomataInitialState">
        <rdfs:subClassOf rdf:resource="http://europe.bourges.univ-orleans.fr/sites/default/files/download/Ontology/Core/kernel.owl#AutomataState"/>
        <rdfs:comment xml:lang="en">Initial state of a Finite State Machine</rdfs:comment>
    </owl:Class>
    


    <!-- http://europe.bourges.univ-orleans.fr/sites/default/files/download/Ontology/Core/kernel.owl#AutomataState -->

    <owl:Class rdf:about="http://europe.bourges.univ-orleans.fr/sites/default/files/download/Ontology/Core/kernel.owl#AutomataState">
        <rdfs:subClassOf rdf:resource="http://europe.bourges.univ-orleans.fr/sites/default/files/download/Ontology/Core/kernel.owl#State"/>
        <rdfs:comment xml:lang="en">The states of a Finite State Machine are a particular case of state</rdfs:comment>
    </owl:Class>
    


    <!-- http://europe.bourges.univ-orleans.fr/sites/default/files/download/Ontology/Core/kernel.owl#Build -->

    <owl:Class rdf:about="http://europe.bourges.univ-orleans.fr/sites/default/files/download/Ontology/Core/kernel.owl#Build">
        <rdfs:subClassOf rdf:resource="http://europe.bourges.univ-orleans.fr/sites/default/files/download/Ontology/Core/kernel.owl#Action"/>
        <rdfs:subClassOf>
            <owl:Restriction>
                <owl:onProperty rdf:resource="http://europe.bourges.univ-orleans.fr/sites/default/files/download/Ontology/Core/kernel.owl#impacts"/>
                <owl:allValuesFrom rdf:resource="http://europe.bourges.univ-orleans.fr/sites/default/files/download/Ontology/Core/kernel.owl#Hardware"/>
            </owl:Restriction>
        </rdfs:subClassOf>
        <author xml:lang="en">creation Bruno Patin - 09/10/2013
- this action allows to explain the specificity of Hardware concept to be built by Humans</author>
    </owl:Class>
    


    <!-- http://europe.bourges.univ-orleans.fr/sites/default/files/download/Ontology/Core/kernel.owl#ChangeEvent -->

    <owl:Class rdf:about="http://europe.bourges.univ-orleans.fr/sites/default/files/download/Ontology/Core/kernel.owl#ChangeEvent">
        <rdfs:subClassOf rdf:resource="http://europe.bourges.univ-orleans.fr/sites/default/files/download/Ontology/Core/kernel.owl#Event"/>
        <owl:disjointWith rdf:resource="http://europe.bourges.univ-orleans.fr/sites/default/files/download/Ontology/Core/kernel.owl#Interaction"/>
        <rdfs:comment xml:lang="en">A condition becomes true.</rdfs:comment>
    </owl:Class>
    


    <!-- http://europe.bourges.univ-orleans.fr/sites/default/files/download/Ontology/Core/kernel.owl#Clock -->

    <owl:Class rdf:about="http://europe.bourges.univ-orleans.fr/sites/default/files/download/Ontology/Core/kernel.owl#Clock">
        <rdfs:subClassOf rdf:resource="http://europe.bourges.univ-orleans.fr/sites/default/files/download/Ontology/Core/kernel.owl#Hardware"/>
        <rdfs:comment xml:lang="en">The timeframe of the world needs to be translated in something usable by other hardware. This the role of the clock concept.</rdfs:comment>
    </owl:Class>
    


    <!-- http://europe.bourges.univ-orleans.fr/sites/default/files/download/Ontology/Core/kernel.owl#CompositeModel -->

    <owl:Class rdf:about="http://europe.bourges.univ-orleans.fr/sites/default/files/download/Ontology/Core/kernel.owl#CompositeModel">
        <rdfs:subClassOf rdf:resource="http://europe.bourges.univ-orleans.fr/sites/default/files/download/Ontology/Core/kernel.owl#CompositeSystem"/>
        <rdfs:subClassOf rdf:resource="http://europe.bourges.univ-orleans.fr/sites/default/files/download/Ontology/Core/kernel.owl#Model"/>
        <owl:disjointWith rdf:resource="http://europe.bourges.univ-orleans.fr/sites/default/files/download/Ontology/Core/kernel.owl#Environment"/>
        <rdfs:comment xml:lang="en">This concept groups the different theory that can be used to model two or more system. It is often linked to a mathematical theory. In the composite model case it is also often linked to architecture representation of this same system. E.g. the environment, reality of it, can be represented as the aggregation of terrain and buildings or it can be represented by the surface where only one system represent terrain AND buildings. As for any model (as is this ontology), the way to represent depends of its usage.
An atomic model being an atomic system is thus disjoint from a composite model as it is a composite system.</rdfs:comment>
    </owl:Class>
    


    <!-- http://europe.bourges.univ-orleans.fr/sites/default/files/download/Ontology/Core/kernel.owl#CompositeSystem -->

    <owl:Class rdf:about="http://europe.bourges.univ-orleans.fr/sites/default/files/download/Ontology/Core/kernel.owl#CompositeSystem">
        <rdfs:subClassOf rdf:resource="http://europe.bourges.univ-orleans.fr/sites/default/files/download/Ontology/Core/kernel.owl#System"/>
        <rdfs:subClassOf>
            <owl:Restriction>
                <owl:onProperty rdf:resource="http://europe.bourges.univ-orleans.fr/sites/default/files/download/Ontology/Core/kernel.owl#aggregates"/>
                <owl:onClass rdf:resource="http://europe.bourges.univ-orleans.fr/sites/default/files/download/Ontology/Core/kernel.owl#System"/>
                <owl:minQualifiedCardinality rdf:datatype="&xsd;nonNegativeInteger">2</owl:minQualifiedCardinality>
            </owl:Restriction>
        </rdfs:subClassOf>
        <rdfs:subClassOf>
            <owl:Restriction>
                <owl:onProperty rdf:resource="http://europe.bourges.univ-orleans.fr/sites/default/files/download/Ontology/Core/kernel.owl#isAtomic"/>
                <owl:hasValue rdf:datatype="&xsd;boolean">false</owl:hasValue>
            </owl:Restriction>
        </rdfs:subClassOf>
        <rdfs:comment xml:lang="en">A composite system is an aggregate of systems. 

It is needed to use the Composite system approach if you work with two systems at least. If one system is concerned then you need in fact to use the underlying atomic system.

In DEVS it is possible to create a system enclosing only one system. It is of no use if something else is not done in between (such as enclosing a differential modelled system into a DEVS block). When discussing composition here we are speaking of the intrinsic property of composition. These aspects of adapting one system to another interface will be of help when discussing the models exhibiting these composition properties in a computer for simulation purpose.</rdfs:comment>
        <author xml:lang="en">creation PROTEUS consortium - 
modified Bruno Patin - 09/09/2013
- min value is changed from 2 to 1
modified Bruno Patin - 14/09/2013
- min value goes back to two because there was a misconception considering Robotic systems
- explanations added in the comment
- addition of OpenCyc link</author>
    </owl:Class>
    


    <!-- http://europe.bourges.univ-orleans.fr/sites/default/files/download/Ontology/Core/kernel.owl#Connector -->

    <owl:Class rdf:about="http://europe.bourges.univ-orleans.fr/sites/default/files/download/Ontology/Core/kernel.owl#Connector">
        <owl:disjointWith rdf:resource="http://europe.bourges.univ-orleans.fr/sites/default/files/download/Ontology/Core/kernel.owl#Event"/>
        <owl:disjointWith rdf:resource="http://europe.bourges.univ-orleans.fr/sites/default/files/download/Ontology/Core/kernel.owl#Evolution"/>
        <owl:disjointWith rdf:resource="http://europe.bourges.univ-orleans.fr/sites/default/files/download/Ontology/Core/kernel.owl#Frame"/>
        <owl:disjointWith rdf:resource="http://europe.bourges.univ-orleans.fr/sites/default/files/download/Ontology/Core/kernel.owl#Information"/>
        <owl:disjointWith rdf:resource="http://europe.bourges.univ-orleans.fr/sites/default/files/download/Ontology/Core/kernel.owl#Interaction"/>
        <owl:disjointWith rdf:resource="http://europe.bourges.univ-orleans.fr/sites/default/files/download/Ontology/Core/kernel.owl#Port"/>
        <owl:disjointWith rdf:resource="http://europe.bourges.univ-orleans.fr/sites/default/files/download/Ontology/Core/kernel.owl#Probe"/>
        <owl:disjointWith rdf:resource="http://europe.bourges.univ-orleans.fr/sites/default/files/download/Ontology/Core/kernel.owl#Protocol"/>
        <owl:disjointWith rdf:resource="http://europe.bourges.univ-orleans.fr/sites/default/files/download/Ontology/Core/kernel.owl#System"/>
        <owl:disjointWith rdf:resource="http://europe.bourges.univ-orleans.fr/sites/default/files/download/Ontology/Core/kernel.owl#Time"/>
        <owl:disjointWith rdf:resource="http://europe.bourges.univ-orleans.fr/sites/default/files/download/Ontology/Core/kernel.owl#Transition"/>
        <rdfs:comment xml:lang="en">A connector is the link that can exist between ports of systems. It  has a unique upstream port and a unique downstream port. There are no interaction possible between two systems if no connector relies them.

This concept is closely linked to system concept.</rdfs:comment>
    </owl:Class>
    


    <!-- http://europe.bourges.univ-orleans.fr/sites/default/files/download/Ontology/Core/kernel.owl#Data -->

    <owl:Class rdf:about="http://europe.bourges.univ-orleans.fr/sites/default/files/download/Ontology/Core/kernel.owl#Data">
        <rdfs:subClassOf rdf:resource="http://europe.bourges.univ-orleans.fr/sites/default/files/download/Ontology/Core/kernel.owl#Information"/>
        <openCycURI rdf:datatype="&xsd;anyURI">http://sw.opencyc.org/concept/Mx4rF8Vc5VFnEdaCtgACs0uXdw</openCycURI>
        <rdfs:comment xml:lang="en">This type of information is directly interpretable by a machine, for example boolean, bits, etc.</rdfs:comment>
        <author xml:lang="en">creation PROTEUS consortium - 
modified Bruno Patin - 13/10/2013
- introduction of openCyc reference</author>
    </owl:Class>
    


    <!-- http://europe.bourges.univ-orleans.fr/sites/default/files/download/Ontology/Core/kernel.owl#DeterministicEvolution -->

    <owl:Class rdf:about="http://europe.bourges.univ-orleans.fr/sites/default/files/download/Ontology/Core/kernel.owl#DeterministicEvolution">
        <rdfs:subClassOf rdf:resource="http://europe.bourges.univ-orleans.fr/sites/default/files/download/Ontology/Core/kernel.owl#Evolution"/>
        <owl:disjointWith rdf:resource="http://europe.bourges.univ-orleans.fr/sites/default/files/download/Ontology/Core/kernel.owl#StochasticEvolution"/>
        <rdfs:comment xml:lang="en">intrinsic property of any object to evolve through time without random phenomenon intervention which would affect the course of the evolution.</rdfs:comment>
    </owl:Class>
    


    <!-- http://europe.bourges.univ-orleans.fr/sites/default/files/download/Ontology/Core/kernel.owl#Driver -->

    <owl:Class rdf:about="http://europe.bourges.univ-orleans.fr/sites/default/files/download/Ontology/Core/kernel.owl#Driver">
        <rdfs:subClassOf rdf:resource="http://europe.bourges.univ-orleans.fr/sites/default/files/download/Ontology/Core/kernel.owl#Application"/>
        <rdfs:subClassOf>
            <owl:Restriction>
                <owl:onProperty rdf:resource="http://europe.bourges.univ-orleans.fr/sites/default/files/download/Ontology/Core/kernel.owl#triggers"/>
                <owl:allValuesFrom>
                    <owl:Class>
                        <owl:unionOf rdf:parseType="Collection">
                            <rdf:Description rdf:about="http://europe.bourges.univ-orleans.fr/sites/default/files/download/Ontology/Core/kernel.owl#ApplicationInteraction"/>
                            <rdf:Description rdf:about="http://europe.bourges.univ-orleans.fr/sites/default/files/download/Ontology/Core/kernel.owl#DriverToHardwareInteraction"/>
                        </owl:unionOf>
                    </owl:Class>
                </owl:allValuesFrom>
            </owl:Restriction>
        </rdfs:subClassOf>
        <owl:disjointWith rdf:resource="http://europe.bourges.univ-orleans.fr/sites/default/files/download/Ontology/Core/kernel.owl#FileSystem"/>
        <owl:disjointWith rdf:resource="http://europe.bourges.univ-orleans.fr/sites/default/files/download/Ontology/Core/kernel.owl#OperatingSystem"/>
        <owl:disjointWith rdf:resource="http://europe.bourges.univ-orleans.fr/sites/default/files/download/Ontology/Core/kernel.owl#SoftwareProbe"/>
        <rdfs:comment xml:lang="en">It is an application which controls the corresponding hardware. The DeviceSystem of a platform like a RoboticSystem, will be composed of theHardware components and the corresponding software driver components. The hardware considered must have some computing abilities in order to allow the driver to execute.</rdfs:comment>
    </owl:Class>
    


    <!-- http://europe.bourges.univ-orleans.fr/sites/default/files/download/Ontology/Core/kernel.owl#DriverToHardwareInteraction -->

    <owl:Class rdf:about="http://europe.bourges.univ-orleans.fr/sites/default/files/download/Ontology/Core/kernel.owl#DriverToHardwareInteraction">
        <rdfs:subClassOf rdf:resource="http://europe.bourges.univ-orleans.fr/sites/default/files/download/Ontology/Core/kernel.owl#Interaction"/>
        <rdfs:subClassOf>
            <owl:Restriction>
                <owl:onProperty rdf:resource="http://europe.bourges.univ-orleans.fr/sites/default/files/download/Ontology/Core/kernel.owl#impacts"/>
                <owl:allValuesFrom rdf:resource="http://europe.bourges.univ-orleans.fr/sites/default/files/download/Ontology/Core/kernel.owl#Hardware"/>
            </owl:Restriction>
        </rdfs:subClassOf>
        <owl:disjointWith rdf:resource="http://europe.bourges.univ-orleans.fr/sites/default/files/download/Ontology/Core/kernel.owl#HardwareToDriverInteraction"/>
        <owl:disjointWith rdf:resource="http://europe.bourges.univ-orleans.fr/sites/default/files/download/Ontology/Core/kernel.owl#PhysicalInteraction"/>
        <rdfs:comment xml:lang="en">Interaction from Drivers (ActuatorDriver, CommunicationDriver, PowerDriver, SensorDriver) to their corresponding hardware(ActuatorHardware, CommunicationHardware, PowerHardware, SensorHardware).</rdfs:comment>
    </owl:Class>
    


    <!-- http://europe.bourges.univ-orleans.fr/sites/default/files/download/Ontology/Core/kernel.owl#Environment -->

    <owl:Class rdf:about="http://europe.bourges.univ-orleans.fr/sites/default/files/download/Ontology/Core/kernel.owl#Environment">
        <rdfs:subClassOf rdf:resource="http://europe.bourges.univ-orleans.fr/sites/default/files/download/Ontology/Core/kernel.owl#CompositeSystem"/>
        <rdfs:subClassOf rdf:resource="http://europe.bourges.univ-orleans.fr/sites/default/files/download/Ontology/Core/kernel.owl#PhysicalObject"/>
        <rdfs:subClassOf>
            <owl:Restriction>
                <owl:onProperty rdf:resource="http://europe.bourges.univ-orleans.fr/sites/default/files/download/Ontology/Core/kernel.owl#hasPort"/>
                <owl:maxCardinality rdf:datatype="&xsd;nonNegativeInteger">0</owl:maxCardinality>
            </owl:Restriction>
        </rdfs:subClassOf>
        <rdfs:subClassOf>
            <owl:Restriction>
                <owl:onProperty rdf:resource="http://europe.bourges.univ-orleans.fr/sites/default/files/download/Ontology/Core/kernel.owl#triggers"/>
                <owl:allValuesFrom rdf:resource="http://europe.bourges.univ-orleans.fr/sites/default/files/download/Ontology/Core/kernel.owl#PhysicalInteraction"/>
            </owl:Restriction>
        </rdfs:subClassOf>
        <owl:disjointWith rdf:resource="http://europe.bourges.univ-orleans.fr/sites/default/files/download/Ontology/Core/kernel.owl#Hardware"/>
        <rdfs:comment xml:lang="en">This environment groups everything that exist. Nothing is outside and everything lives in it. An alias for environment could be Universe or World in an ontologic meaning. This is the highest possible &quot;container&quot; for the physical objects to exist.
Considering the scenario to be represented using this concept it expresses also the boundary we imagine for the problem. As an example, for a mobile on ground robot there is no need to represent anything concerning water.

The difference between physical objects and THE environment is that the PhysicalInteraction are part only of the latter and propagated into it.

There is a difference between the meaning of OpenCyc concept to the one of the ontology due to the fact there is nothing enclosing RobotML Environment concept when OpenCyc does not state anything on this point.</rdfs:comment>
    </owl:Class>
    <owl:Axiom>
        <rdfs:comment xml:lang="en">this property expresses the fact that the environment is not associated to any software running in it.</rdfs:comment>
        <owl:annotatedSource rdf:resource="http://europe.bourges.univ-orleans.fr/sites/default/files/download/Ontology/Core/kernel.owl#Environment"/>
        <owl:annotatedProperty rdf:resource="&rdfs;subClassOf"/>
        <owl:annotatedTarget>
            <owl:Restriction>
                <owl:onProperty rdf:resource="http://europe.bourges.univ-orleans.fr/sites/default/files/download/Ontology/Core/kernel.owl#triggers"/>
                <owl:allValuesFrom rdf:resource="http://europe.bourges.univ-orleans.fr/sites/default/files/download/Ontology/Core/kernel.owl#PhysicalInteraction"/>
            </owl:Restriction>
        </owl:annotatedTarget>
    </owl:Axiom>
    <owl:Axiom>
        <rdfs:comment xml:lang="en">this property constrains the environment not to have any port. Thus no interactions can occur between environment and another anything.</rdfs:comment>
        <owl:annotatedSource rdf:resource="http://europe.bourges.univ-orleans.fr/sites/default/files/download/Ontology/Core/kernel.owl#Environment"/>
        <owl:annotatedProperty rdf:resource="&rdfs;subClassOf"/>
        <owl:annotatedTarget>
            <owl:Restriction>
                <owl:onProperty rdf:resource="http://europe.bourges.univ-orleans.fr/sites/default/files/download/Ontology/Core/kernel.owl#hasPort"/>
                <owl:maxCardinality rdf:datatype="&xsd;nonNegativeInteger">0</owl:maxCardinality>
            </owl:Restriction>
        </owl:annotatedTarget>
    </owl:Axiom>
    


    <!-- http://europe.bourges.univ-orleans.fr/sites/default/files/download/Ontology/Core/kernel.owl#Event -->

    <owl:Class rdf:about="http://europe.bourges.univ-orleans.fr/sites/default/files/download/Ontology/Core/kernel.owl#Event">
        <owl:disjointWith rdf:resource="http://europe.bourges.univ-orleans.fr/sites/default/files/download/Ontology/Core/kernel.owl#Evolution"/>
        <owl:disjointWith rdf:resource="http://europe.bourges.univ-orleans.fr/sites/default/files/download/Ontology/Core/kernel.owl#Frame"/>
        <owl:disjointWith rdf:resource="http://europe.bourges.univ-orleans.fr/sites/default/files/download/Ontology/Core/kernel.owl#Information"/>
        <owl:disjointWith rdf:resource="http://europe.bourges.univ-orleans.fr/sites/default/files/download/Ontology/Core/kernel.owl#Port"/>
        <owl:disjointWith rdf:resource="http://europe.bourges.univ-orleans.fr/sites/default/files/download/Ontology/Core/kernel.owl#Probe"/>
        <owl:disjointWith rdf:resource="http://europe.bourges.univ-orleans.fr/sites/default/files/download/Ontology/Core/kernel.owl#Protocol"/>
        <owl:disjointWith rdf:resource="http://europe.bourges.univ-orleans.fr/sites/default/files/download/Ontology/Core/kernel.owl#System"/>
        <owl:disjointWith rdf:resource="http://europe.bourges.univ-orleans.fr/sites/default/files/download/Ontology/Core/kernel.owl#Time"/>
        <owl:disjointWith rdf:resource="http://europe.bourges.univ-orleans.fr/sites/default/files/download/Ontology/Core/kernel.owl#Transition"/>
        <otherURI rdf:datatype="&xsd;anyURI">Stanford encyclopedia of philosophy
http://plato.stanford.edu/entries/events/</otherURI>
        <wikipediaURI rdf:datatype="&xsd;anyURI">http://en.wikipedia.org/wiki/Event_%28philosophy%29</wikipediaURI>
        <openCycURI rdf:datatype="&xsd;anyURI">http://sw.opencyc.org/concept/Mx4rvViADZwpEbGdrcN5Y29ycA</openCycURI>
        <rdfs:comment xml:lang="en">In philosophy, events are objects in time or instantiations of properties in objects. Here events are closely linked to system concept as they are the modalities that make them change their states.</rdfs:comment>
    </owl:Class>
    


    <!-- http://europe.bourges.univ-orleans.fr/sites/default/files/download/Ontology/Core/kernel.owl#Evolution -->

    <owl:Class rdf:about="http://europe.bourges.univ-orleans.fr/sites/default/files/download/Ontology/Core/kernel.owl#Evolution">
        <rdfs:subClassOf rdf:resource="&owl;Thing"/>
        <rdfs:subClassOf>
            <owl:Restriction>
                <owl:onProperty rdf:resource="http://europe.bourges.univ-orleans.fr/sites/default/files/download/Ontology/Core/kernel.owl#isAFunctionOfTime"/>
                <owl:maxCardinality rdf:datatype="&xsd;nonNegativeInteger">1</owl:maxCardinality>
            </owl:Restriction>
        </rdfs:subClassOf>
        <owl:disjointWith rdf:resource="http://europe.bourges.univ-orleans.fr/sites/default/files/download/Ontology/Core/kernel.owl#Frame"/>
        <owl:disjointWith rdf:resource="http://europe.bourges.univ-orleans.fr/sites/default/files/download/Ontology/Core/kernel.owl#Information"/>
        <owl:disjointWith rdf:resource="http://europe.bourges.univ-orleans.fr/sites/default/files/download/Ontology/Core/kernel.owl#Interaction"/>
        <owl:disjointWith rdf:resource="http://europe.bourges.univ-orleans.fr/sites/default/files/download/Ontology/Core/kernel.owl#Port"/>
        <owl:disjointWith rdf:resource="http://europe.bourges.univ-orleans.fr/sites/default/files/download/Ontology/Core/kernel.owl#Probe"/>
        <owl:disjointWith rdf:resource="http://europe.bourges.univ-orleans.fr/sites/default/files/download/Ontology/Core/kernel.owl#Protocol"/>
        <owl:disjointWith rdf:resource="http://europe.bourges.univ-orleans.fr/sites/default/files/download/Ontology/Core/kernel.owl#System"/>
        <owl:disjointWith rdf:resource="http://europe.bourges.univ-orleans.fr/sites/default/files/download/Ontology/Core/kernel.owl#Time"/>
        <owl:disjointWith rdf:resource="http://europe.bourges.univ-orleans.fr/sites/default/files/download/Ontology/Core/kernel.owl#Transition"/>
        <wikipediaURI rdf:datatype="&xsd;anyURI">http://en.wikipedia.org/wiki/Time_evolution</wikipediaURI>
        <openCycURI rdf:datatype="&xsd;anyURI">http://sw.opencyc.org/concept/Mx4rvoZDlZwpEbGdrcN5Y29ycA</openCycURI>
        <TODO xml:lang="en">2. EvolutionModel should not have inputState or the like, it should have system associated with time value. It means that if a system is associated to time then an evolution model is able to make it change changing the value of time.</TODO>
        <rdfs:comment xml:lang="en">Evolution is what allows systems to live through a state trajectory either in a discrete or in a continuous form depending on the type of law used. Here evolution means the intrinsic property of any object to evolve through time.

Considering the wikipedia link, the closest wording to be considered is &quot;time evolution&quot; that introduces explicitely the internal state dynamic and in fact the system concept.

Considering openCyc link it refers to darwin evolution theory. This is very close to this definition that refers to anything in the universe and not only biological entities.</rdfs:comment>
    </owl:Class>
    


    <!-- http://europe.bourges.univ-orleans.fr/sites/default/files/download/Ontology/Core/kernel.owl#FileSystem -->

    <owl:Class rdf:about="http://europe.bourges.univ-orleans.fr/sites/default/files/download/Ontology/Core/kernel.owl#FileSystem">
        <rdfs:subClassOf rdf:resource="http://europe.bourges.univ-orleans.fr/sites/default/files/download/Ontology/Core/kernel.owl#Application"/>
        <rdfs:subClassOf>
            <owl:Restriction>
                <owl:onProperty rdf:resource="http://europe.bourges.univ-orleans.fr/sites/default/files/download/Ontology/Core/kernel.owl#triggers"/>
                <owl:allValuesFrom rdf:resource="http://europe.bourges.univ-orleans.fr/sites/default/files/download/Ontology/Core/kernel.owl#ApplicationInteraction"/>
            </owl:Restriction>
        </rdfs:subClassOf>
        <owl:disjointWith rdf:resource="http://europe.bourges.univ-orleans.fr/sites/default/files/download/Ontology/Core/kernel.owl#OperatingSystem"/>
        <owl:disjointWith rdf:resource="http://europe.bourges.univ-orleans.fr/sites/default/files/download/Ontology/Core/kernel.owl#SoftwareProbe"/>
        <owl:disjointWith rdf:resource="http://europe.bourges.univ-orleans.fr/sites/default/files/download/Ontology/Core/kernel.owl#Wrapper"/>
        <openCycURI rdf:datatype="&xsd;anyURI">http://sw.opencyc.org/concept/Mx4rv98a6JwpEbGdrcN5Y29ycA</openCycURI>
        <rdfs:comment xml:lang="en">A file system is an application that organizes data expected to be retained after a program terminates by providing procedures to store, retrieve and update data, as well as manage the available space on the device(s) which contain it. A file system organizes data in an efficient manner and is tuned to the specific characteristics of the device. There is usually a tight coupling between the operating system and the file system.</rdfs:comment>
        <author xml:lang="en">creation PROTEUS consortium - 
modified Bruno Patin - 30/09/2013
- FileSystem IS an application using the OperatingSystem to manage interaction with stored data
- addition of openCyc reference</author>
    </owl:Class>
    


    <!-- http://europe.bourges.univ-orleans.fr/sites/default/files/download/Ontology/Core/kernel.owl#Frame -->

    <owl:Class rdf:about="http://europe.bourges.univ-orleans.fr/sites/default/files/download/Ontology/Core/kernel.owl#Frame">
        <owl:disjointWith rdf:resource="http://europe.bourges.univ-orleans.fr/sites/default/files/download/Ontology/Core/kernel.owl#Information"/>
        <owl:disjointWith rdf:resource="http://europe.bourges.univ-orleans.fr/sites/default/files/download/Ontology/Core/kernel.owl#Interaction"/>
        <owl:disjointWith rdf:resource="http://europe.bourges.univ-orleans.fr/sites/default/files/download/Ontology/Core/kernel.owl#Port"/>
        <owl:disjointWith rdf:resource="http://europe.bourges.univ-orleans.fr/sites/default/files/download/Ontology/Core/kernel.owl#Probe"/>
        <owl:disjointWith rdf:resource="http://europe.bourges.univ-orleans.fr/sites/default/files/download/Ontology/Core/kernel.owl#Protocol"/>
        <owl:disjointWith rdf:resource="http://europe.bourges.univ-orleans.fr/sites/default/files/download/Ontology/Core/kernel.owl#System"/>
        <owl:disjointWith rdf:resource="http://europe.bourges.univ-orleans.fr/sites/default/files/download/Ontology/Core/kernel.owl#Time"/>
        <owl:disjointWith rdf:resource="http://europe.bourges.univ-orleans.fr/sites/default/files/download/Ontology/Core/kernel.owl#Transition"/>
        <wikipediaURI rdf:datatype="&xsd;anyURI">http://en.wikipedia.org/wiki/Frame_of_reference</wikipediaURI>
        <openCycURI rdf:datatype="&xsd;anyURI">http://sw.opencyc.org/concept/Mx4rvVjUoJwpEbGdrcN5Y29ycA</openCycURI>
        <rdfs:comment xml:lang="en">This class instantiates the capability to link points in space. Space can be any dimension needed. This property can be constrained when the class is linked to others. As an example, physical object will use 3D coordinate systems using euclidean representation or 4D if using an einsteinen representation.

It is through this class that space will have an associated metric.

Attention must be focused on the fact there is an essential difference between the frame that expresses the fundamental property of object to be referenced and reference system that are the capability to manipulate referential (cartesian, circular, spherical, whatever). It means that there is only one referential associated to the environment and each of the physical objects it includes and there are many ways to manipulate them through reference systems.

The openCyc definition refers to a more generic concept. The capability that a frame has to provide a context in which objects can be referenced. Not only positionned.</rdfs:comment>
    </owl:Class>
    


    <!-- http://europe.bourges.univ-orleans.fr/sites/default/files/download/Ontology/Core/kernel.owl#Hardware -->

    <owl:Class rdf:about="http://europe.bourges.univ-orleans.fr/sites/default/files/download/Ontology/Core/kernel.owl#Hardware">
        <rdfs:subClassOf rdf:resource="http://europe.bourges.univ-orleans.fr/sites/default/files/download/Ontology/Core/kernel.owl#PhysicalObject"/>
        <author rdf:datatype="&xsd;anyURI">creation PROTEUS consortium - 
modified Bruno Patin - 30/09/2013
- addition of opencyc reference</author>
        <openCycURI rdf:datatype="&xsd;anyURI">http://sw.opencyc.org/concept/Mx4rvVkH_ZwpEbGdrcN5Y29ycA</openCycURI>
        <rdfs:comment xml:lang="en">The hardware characteristics is to be man made. It means that when built, from human perspective, it had a goal. Can be changed because of its use. Such a hardware is supposed to have computing abilities if it is associated to some software.

It is closer to &quot;Artifact&quot; opencyc definition than from the hardware part that is itself closer to &quot;marketable&quot; parts.</rdfs:comment>
    </owl:Class>
    


    <!-- http://europe.bourges.univ-orleans.fr/sites/default/files/download/Ontology/Core/kernel.owl#HardwareToDriverInteraction -->

    <owl:Class rdf:about="http://europe.bourges.univ-orleans.fr/sites/default/files/download/Ontology/Core/kernel.owl#HardwareToDriverInteraction">
        <rdfs:subClassOf rdf:resource="http://europe.bourges.univ-orleans.fr/sites/default/files/download/Ontology/Core/kernel.owl#Interaction"/>
        <rdfs:subClassOf>
            <owl:Restriction>
                <owl:onProperty rdf:resource="http://europe.bourges.univ-orleans.fr/sites/default/files/download/Ontology/Core/kernel.owl#impacts"/>
                <owl:allValuesFrom rdf:resource="http://europe.bourges.univ-orleans.fr/sites/default/files/download/Ontology/Core/kernel.owl#Driver"/>
            </owl:Restriction>
        </rdfs:subClassOf>
        <owl:disjointWith rdf:resource="http://europe.bourges.univ-orleans.fr/sites/default/files/download/Ontology/Core/kernel.owl#PhysicalInteraction"/>
        <rdfs:comment xml:lang="en">Interaction from Hardware (ActuatorHardware, CommunicationHardware, PowerHardware, SensorHardware) to their corresponding Drivers (ActuatorDriver, CommunicationDriver, PowerDriver, SensorDriver)). For instance, return of information coming from the sensor hardware to be managed by the software part of the platform.</rdfs:comment>
    </owl:Class>
    


    <!-- http://europe.bourges.univ-orleans.fr/sites/default/files/download/Ontology/Core/kernel.owl#Human -->

    <owl:Class rdf:about="http://europe.bourges.univ-orleans.fr/sites/default/files/download/Ontology/Core/kernel.owl#Human">
        <rdfs:subClassOf rdf:resource="http://europe.bourges.univ-orleans.fr/sites/default/files/download/Ontology/Core/kernel.owl#Animal"/>
        <rdfs:isDefinedBy rdf:datatype="&xsd;anyURI">http://sw.opencyc.org/concept/Mx4rIcwFloGUQdeMlsOWYLFB2w</rdfs:isDefinedBy>
        <rdfs:seeAlso rdf:datatype="&xsd;string">openCyc: HomoSapiens</rdfs:seeAlso>
        <rdfs:comment xml:lang="en">A human moves in waterbodies, over ground and over water surface (swiming). He or she pilots robots.</rdfs:comment>
    </owl:Class>
    


    <!-- http://europe.bourges.univ-orleans.fr/sites/default/files/download/Ontology/Core/kernel.owl#Information -->

    <owl:Class rdf:about="http://europe.bourges.univ-orleans.fr/sites/default/files/download/Ontology/Core/kernel.owl#Information">
        <owl:disjointWith rdf:resource="http://europe.bourges.univ-orleans.fr/sites/default/files/download/Ontology/Core/kernel.owl#Interaction"/>
        <owl:disjointWith rdf:resource="http://europe.bourges.univ-orleans.fr/sites/default/files/download/Ontology/Core/kernel.owl#Port"/>
        <owl:disjointWith rdf:resource="http://europe.bourges.univ-orleans.fr/sites/default/files/download/Ontology/Core/kernel.owl#Probe"/>
        <owl:disjointWith rdf:resource="http://europe.bourges.univ-orleans.fr/sites/default/files/download/Ontology/Core/kernel.owl#Protocol"/>
        <owl:disjointWith rdf:resource="http://europe.bourges.univ-orleans.fr/sites/default/files/download/Ontology/Core/kernel.owl#System"/>
        <owl:disjointWith rdf:resource="http://europe.bourges.univ-orleans.fr/sites/default/files/download/Ontology/Core/kernel.owl#Time"/>
        <owl:disjointWith rdf:resource="http://europe.bourges.univ-orleans.fr/sites/default/files/download/Ontology/Core/kernel.owl#Transition"/>
        <wikipediaURI rdf:datatype="&xsd;anyURI">http://en.wikipedia.org/wiki/Information</wikipediaURI>
        <openCycURI rdf:datatype="&xsd;anyURI">http://sw.opencyc.org/concept/Mx4rwQGTzJwpEbGdrcN5Y29ycA</openCycURI>
        <TODO xml:lang="en">Data is linked completely to Computers. Abstraction is linked to nothing. We do not have a concept linked to human beings or other sentient objects of the Universe (thus agent minus robots, more or less).

It is not in kernel that data and abstraction should be defined. In kernel we speak of what it is and not how it is represented. This point is to be discussed.</TODO>
        <rdfs:comment xml:lang="en">Information concept is the concept dealing with meaning. It is the way &quot;things&quot; can be described. This concept is decomposed in the abstraction concept (meaning disembodied information whatever it can means - OpenCyc uses the word intangible - and data - meaning embodied information.</rdfs:comment>
    </owl:Class>
    


    <!-- http://europe.bourges.univ-orleans.fr/sites/default/files/download/Ontology/Core/kernel.owl#InterAgentCommunication -->

    <owl:Class rdf:about="http://europe.bourges.univ-orleans.fr/sites/default/files/download/Ontology/Core/kernel.owl#InterAgentCommunication">
        <rdfs:subClassOf rdf:resource="http://europe.bourges.univ-orleans.fr/sites/default/files/download/Ontology/Core/kernel.owl#Action"/>
        <rdfs:comment xml:lang="en">For multi-robot and human-robot systems agents have to communicate in order to fulfill the mission.</rdfs:comment>
        <author xml:lang="en">creation PROTEUS consortium - 
modified Bruno Patin - 04/10/2013
- communication is a type of action as it concerns only interaction between agents, it is thus moved to Action</author>
    </owl:Class>
    


    <!-- http://europe.bourges.univ-orleans.fr/sites/default/files/download/Ontology/Core/kernel.owl#Interaction -->

    <owl:Class rdf:about="http://europe.bourges.univ-orleans.fr/sites/default/files/download/Ontology/Core/kernel.owl#Interaction">
        <owl:disjointWith rdf:resource="http://europe.bourges.univ-orleans.fr/sites/default/files/download/Ontology/Core/kernel.owl#Port"/>
        <owl:disjointWith rdf:resource="http://europe.bourges.univ-orleans.fr/sites/default/files/download/Ontology/Core/kernel.owl#Probe"/>
        <owl:disjointWith rdf:resource="http://europe.bourges.univ-orleans.fr/sites/default/files/download/Ontology/Core/kernel.owl#Protocol"/>
        <owl:disjointWith rdf:resource="http://europe.bourges.univ-orleans.fr/sites/default/files/download/Ontology/Core/kernel.owl#System"/>
        <owl:disjointWith rdf:resource="http://europe.bourges.univ-orleans.fr/sites/default/files/download/Ontology/Core/kernel.owl#Time"/>
        <owl:disjointWith rdf:resource="http://europe.bourges.univ-orleans.fr/sites/default/files/download/Ontology/Core/kernel.owl#TimeEvent"/>
        <owl:disjointWith rdf:resource="http://europe.bourges.univ-orleans.fr/sites/default/files/download/Ontology/Core/kernel.owl#Transition"/>
        <wikipediaURI rdf:datatype="&xsd;anyURI">http://en.wikipedia.org/wiki/Interaction</wikipediaURI>
        <openCycURI rdf:datatype="&xsd;anyURI">http://sw.opencyc.org/concept/Mx4rvVioQZwpEbGdrcN5Y29ycA</openCycURI>
        <rdfs:comment xml:lang="en">Interaction occurs when two or more Objects/Systems have an effect upon one another. This concept is closely linked to the system concept in this ontology. 

Interaction is in fact close to Action OpenCyc concept. It is more abstract because it is not a tangible thing that is concerned but two systems (tangible thing = Physical Object and Physical object is a system).</rdfs:comment>
        <rdfs:comment xml:lang="en">creation PROTEUS consortium - 
modified Bruno Patin - 04/10/2013
- comment edition</rdfs:comment>
    </owl:Class>
    


    <!-- http://europe.bourges.univ-orleans.fr/sites/default/files/download/Ontology/Core/kernel.owl#Model -->

    <owl:Class rdf:about="http://europe.bourges.univ-orleans.fr/sites/default/files/download/Ontology/Core/kernel.owl#Model">
        <rdfs:subClassOf rdf:resource="http://europe.bourges.univ-orleans.fr/sites/default/files/download/Ontology/Core/kernel.owl#System"/>
        <rdfs:subClassOf>
            <owl:Restriction>
                <owl:onProperty rdf:resource="http://europe.bourges.univ-orleans.fr/sites/default/files/download/Ontology/Core/kernel.owl#models"/>
                <owl:onClass>
                    <owl:Class>
                        <owl:unionOf rdf:parseType="Collection">
                            <rdf:Description rdf:about="http://europe.bourges.univ-orleans.fr/sites/default/files/download/Ontology/Core/kernel.owl#Evolution"/>
                            <rdf:Description rdf:about="http://europe.bourges.univ-orleans.fr/sites/default/files/download/Ontology/Core/kernel.owl#System"/>
                        </owl:unionOf>
                    </owl:Class>
                </owl:onClass>
                <owl:minQualifiedCardinality rdf:datatype="&xsd;nonNegativeInteger">1</owl:minQualifiedCardinality>
            </owl:Restriction>
        </rdfs:subClassOf>
        <openCycURI rdf:datatype="&xsd;anyURI">OpenCyc Model concept is linked to artefact build by human to model other things tangible or not. This concept is more specialised.
http://sw.opencyc.org/concept/Mx4rvgEO8ZwpEbGdrcN5Y29ycA</openCycURI>
        <wikipediaURI rdf:datatype="&xsd;anyURI">this is more generic as almost anything can model almost anything. OpenCyc is not based upon system concept as the basis of the world.
http://en.wikipedia.org/wiki/Conceptual_model</wikipediaURI>
        <rdfs:comment xml:lang="en">Concept introduced in order to recognise when system is reality and when it is a model of this reality. It groups the Atomic and Composite Models.</rdfs:comment>
    </owl:Class>
    


    <!-- http://europe.bourges.univ-orleans.fr/sites/default/files/download/Ontology/Core/kernel.owl#OperatingSystem -->

    <owl:Class rdf:about="http://europe.bourges.univ-orleans.fr/sites/default/files/download/Ontology/Core/kernel.owl#OperatingSystem">
        <rdfs:subClassOf rdf:resource="http://europe.bourges.univ-orleans.fr/sites/default/files/download/Ontology/Core/kernel.owl#Application"/>
        <rdfs:subClassOf>
            <owl:Restriction>
                <owl:onProperty rdf:resource="http://europe.bourges.univ-orleans.fr/sites/default/files/download/Ontology/Core/kernel.owl#triggers"/>
                <owl:allValuesFrom rdf:resource="http://europe.bourges.univ-orleans.fr/sites/default/files/download/Ontology/Core/kernel.owl#ApplicationInteraction"/>
            </owl:Restriction>
        </rdfs:subClassOf>
        <owl:disjointWith rdf:resource="http://europe.bourges.univ-orleans.fr/sites/default/files/download/Ontology/Core/kernel.owl#SoftwareProbe"/>
        <owl:disjointWith rdf:resource="http://europe.bourges.univ-orleans.fr/sites/default/files/download/Ontology/Core/kernel.owl#Wrapper"/>
        <rdfs:comment xml:lang="en">An operating system (OS) is a set of programs that manages computer hardware resources, and provides common services for application software and file management. The operating system is the most important type of system software in a computer system. Without an operating system, a user cannot run an application program on their computer, unless the application program is self booting.</rdfs:comment>
        <openCycURI xml:lang="en">http://sw.opencyc.org/concept/Mx4rvViws5wpEbGdrcN5Y29ycA</openCycURI>
    </owl:Class>
    


    <!-- http://europe.bourges.univ-orleans.fr/sites/default/files/download/Ontology/Core/kernel.owl#PhysicalInteraction -->

    <owl:Class rdf:about="http://europe.bourges.univ-orleans.fr/sites/default/files/download/Ontology/Core/kernel.owl#PhysicalInteraction">
        <rdfs:subClassOf rdf:resource="http://europe.bourges.univ-orleans.fr/sites/default/files/download/Ontology/Core/kernel.owl#Interaction"/>
        <rdfs:subClassOf>
            <owl:Restriction>
                <owl:onProperty rdf:resource="http://europe.bourges.univ-orleans.fr/sites/default/files/download/Ontology/Core/kernel.owl#impacts"/>
                <owl:allValuesFrom rdf:resource="http://europe.bourges.univ-orleans.fr/sites/default/files/download/Ontology/Core/kernel.owl#PhysicalObject"/>
            </owl:Restriction>
        </rdfs:subClassOf>
        <rdfs:comment>It is the same type of object as DriverTo Hardware and HardwareToDriver but at a more abstract level because it is an interaction between two Physical objects.</rdfs:comment>
    </owl:Class>
    


    <!-- http://europe.bourges.univ-orleans.fr/sites/default/files/download/Ontology/Core/kernel.owl#PhysicalObject -->

    <owl:Class rdf:about="http://europe.bourges.univ-orleans.fr/sites/default/files/download/Ontology/Core/kernel.owl#PhysicalObject">
        <rdfs:subClassOf rdf:resource="http://europe.bourges.univ-orleans.fr/sites/default/files/download/Ontology/Core/kernel.owl#System"/>
        <rdfs:subClassOf>
            <owl:Restriction>
                <owl:onProperty rdf:resource="http://europe.bourges.univ-orleans.fr/sites/default/files/download/Ontology/Core/kernel.owl#triggers"/>
                <owl:someValuesFrom>
                    <owl:Class>
                        <owl:unionOf rdf:parseType="Collection">
                            <rdf:Description rdf:about="http://europe.bourges.univ-orleans.fr/sites/default/files/download/Ontology/Core/kernel.owl#HardwareToDriverInteraction"/>
                            <rdf:Description rdf:about="http://europe.bourges.univ-orleans.fr/sites/default/files/download/Ontology/Core/kernel.owl#PhysicalInteraction"/>
                        </owl:unionOf>
                    </owl:Class>
                </owl:someValuesFrom>
            </owl:Restriction>
        </rdfs:subClassOf>
        <owl:disjointWith rdf:resource="http://europe.bourges.univ-orleans.fr/sites/default/files/download/Ontology/Core/kernel.owl#Software"/>
        <openCycURI rdf:datatype="&xsd;anyURI">http://sw.opencyc.org/concept/Mx4rvVj27ZwpEbGdrcN5Y29ycA</openCycURI>
        <rdfs:comment xml:lang="en">The Physical object is something that can be characterised through a border and considered as a whole with respect to the problem considered. As an example, a robot is an object when considering the mobile robotic problem. 
It exist in itself in the environment and is submitted to laws (called here Physical interactions) that govern every aspects of its life in the environment. As an exemple the dynamic law of movement.
A physical object, defining a border, can contain many other physical objects or no object. The decomposition is useful when the user needs to represent a frame supporting inside or at its surface other objects or when a robot is a multi part thing (articulated robot).</rdfs:comment>
    </owl:Class>
    


    <!-- http://europe.bourges.univ-orleans.fr/sites/default/files/download/Ontology/Core/kernel.owl#Port -->

    <owl:Class rdf:about="http://europe.bourges.univ-orleans.fr/sites/default/files/download/Ontology/Core/kernel.owl#Port">
        <rdfs:subClassOf rdf:resource="&owl;Thing"/>
        <rdfs:subClassOf>
            <owl:Restriction>
                <owl:onProperty rdf:resource="http://europe.bourges.univ-orleans.fr/sites/default/files/download/Ontology/Core/kernel.owl#isIn_Out"/>
                <owl:maxCardinality rdf:datatype="&xsd;nonNegativeInteger">1</owl:maxCardinality>
            </owl:Restriction>
        </rdfs:subClassOf>
        <owl:disjointWith rdf:resource="http://europe.bourges.univ-orleans.fr/sites/default/files/download/Ontology/Core/kernel.owl#Probe"/>
        <owl:disjointWith rdf:resource="http://europe.bourges.univ-orleans.fr/sites/default/files/download/Ontology/Core/kernel.owl#Protocol"/>
        <owl:disjointWith rdf:resource="http://europe.bourges.univ-orleans.fr/sites/default/files/download/Ontology/Core/kernel.owl#System"/>
        <owl:disjointWith rdf:resource="http://europe.bourges.univ-orleans.fr/sites/default/files/download/Ontology/Core/kernel.owl#Time"/>
        <owl:disjointWith rdf:resource="http://europe.bourges.univ-orleans.fr/sites/default/files/download/Ontology/Core/kernel.owl#Transition"/>
        <openCycURI rdf:datatype="&xsd;anyURI">There is no equivalent of port concept in OpenCyc. There are three examples of port:
Computer port: http://sw.opencyc.org/concept/Mx4rvVkGw5wpEbGdrcN5Y29ycA
infrastructure, transport port: http://sw.opencyc.org/concept/Mx4r09gVMi_gEdyAAAACs6hRXg
Naval, port facility: http://sw.opencyc.org/concept/Mx4rwRjaEpwpEbGdrcN5Y29ycA</openCycURI>
        <rdfs:comment xml:lang="en">&quot;in&quot; and/or &quot;out&quot; point of a component (here component means system), where data, events and so on pass through.

This definition is closely linked to the definition of systems as they are the entry/output point through which interactions can occur.</rdfs:comment>
        <rdfs:comment xml:lang="fr">point d&apos;entrée et/ou de sortie d&apos;un composant, par où peuvent transiter des données, des événements, etc.</rdfs:comment>
    </owl:Class>
    


    <!-- http://europe.bourges.univ-orleans.fr/sites/default/files/download/Ontology/Core/kernel.owl#Probe -->

    <owl:Class rdf:about="http://europe.bourges.univ-orleans.fr/sites/default/files/download/Ontology/Core/kernel.owl#Probe">
        <owl:disjointWith rdf:resource="http://europe.bourges.univ-orleans.fr/sites/default/files/download/Ontology/Core/kernel.owl#Protocol"/>
        <owl:disjointWith rdf:resource="http://europe.bourges.univ-orleans.fr/sites/default/files/download/Ontology/Core/kernel.owl#Time"/>
        <owl:disjointWith rdf:resource="http://europe.bourges.univ-orleans.fr/sites/default/files/download/Ontology/Core/kernel.owl#Transition"/>
        <wiktionaryURI rdf:datatype="&xsd;anyURI">2nd and 3rd definitions are close to the definition provided here.
http://en.wiktionary.org/wiki/probe</wiktionaryURI>
        <rdfs:comment xml:lang="en">Probe is the concept that provides the capability to create information from the observation of states and thus of a system due to the fact systems have states.</rdfs:comment>
        <TODO xml:lang="en">Sensors can be viewed as type of probes. This is to be verified as it would probably simplify the ontology.</TODO>
    </owl:Class>
    


    <!-- http://europe.bourges.univ-orleans.fr/sites/default/files/download/Ontology/Core/kernel.owl#Protocol -->

    <owl:Class rdf:about="http://europe.bourges.univ-orleans.fr/sites/default/files/download/Ontology/Core/kernel.owl#Protocol">
        <owl:disjointWith rdf:resource="http://europe.bourges.univ-orleans.fr/sites/default/files/download/Ontology/Core/kernel.owl#System"/>
        <owl:disjointWith rdf:resource="http://europe.bourges.univ-orleans.fr/sites/default/files/download/Ontology/Core/kernel.owl#Time"/>
        <owl:disjointWith rdf:resource="http://europe.bourges.univ-orleans.fr/sites/default/files/download/Ontology/Core/kernel.owl#Transition"/>
        <openCycURI rdf:datatype="&xsd;anyURI">In this ontology the protocol concept is larger than this concept as it applies only to agent.
http://sw.opencyc.org/concept/Mx4rxo_VAPHDEdaO6gABAkLVdg</openCycURI>
        <wikipediaURI rdf:datatype="&xsd;anyURI">Protocols in communication field is slightly expanded in this ontology
http://en.wikipedia.org/wiki/Communications_protocol</wikipediaURI>
        <rdfs:comment xml:lang="en">A protocol is a convention on the way systems interact. It then constrains the information exchanges which implements an interaction.</rdfs:comment>
        <TODO xml:lang="en">If a protocol is constraining information exchanges, it means that there are information exchange between physical objects due to interaction but there are no information specialisation for these type of objects in the information context.

Considering the meaning of protocol, it cannot be considered as a kernel concept as it is not applying to the core port / Interaction but to what occurs when there is a communication between two objects thus this is something specialised that should be introduced at the system level (when there is the introduction of the communication system).

Moreover, it is stated that it is the Port / Interaction concept that are impacted. It is not true it is how dynamically things are done and the contents of the exchange but not the nature of these two concepts.</TODO>
        <author xml:lang="en">creation PROTEUS consortium -
modified Bruno Patin - 19/10/2013
- TODO has been upgraded</author>
    </owl:Class>
    


    <!-- http://europe.bourges.univ-orleans.fr/sites/default/files/download/Ontology/Core/kernel.owl#RequestEvent -->

    <owl:Class rdf:about="http://europe.bourges.univ-orleans.fr/sites/default/files/download/Ontology/Core/kernel.owl#RequestEvent">
        <rdfs:subClassOf rdf:resource="http://europe.bourges.univ-orleans.fr/sites/default/files/download/Ontology/Core/kernel.owl#Event"/>
        <rdfs:subClassOf rdf:resource="http://europe.bourges.univ-orleans.fr/sites/default/files/download/Ontology/Core/kernel.owl#Interaction"/>
        <rdfs:comment xml:lang="en">Receipt of a call for an operation.</rdfs:comment>
        <TODO xml:lang="en">clarify concept</TODO>
    </owl:Class>
    


    <!-- http://europe.bourges.univ-orleans.fr/sites/default/files/download/Ontology/Core/kernel.owl#SignalEvent -->

    <owl:Class rdf:about="http://europe.bourges.univ-orleans.fr/sites/default/files/download/Ontology/Core/kernel.owl#SignalEvent">
        <rdfs:subClassOf rdf:resource="http://europe.bourges.univ-orleans.fr/sites/default/files/download/Ontology/Core/kernel.owl#Event"/>
        <rdfs:subClassOf rdf:resource="http://europe.bourges.univ-orleans.fr/sites/default/files/download/Ontology/Core/kernel.owl#Interaction"/>
        <TODO xml:lang="en">Clarify concept</TODO>
        <rdfs:comment xml:lang="en">Receipt of an explicit realtime signal.</rdfs:comment>
    </owl:Class>
    


    <!-- http://europe.bourges.univ-orleans.fr/sites/default/files/download/Ontology/Core/kernel.owl#Software -->

    <owl:Class rdf:about="http://europe.bourges.univ-orleans.fr/sites/default/files/download/Ontology/Core/kernel.owl#Software">
        <rdfs:subClassOf rdf:resource="http://europe.bourges.univ-orleans.fr/sites/default/files/download/Ontology/Core/kernel.owl#System"/>
        <rdfs:subClassOf>
            <owl:Restriction>
                <owl:onProperty rdf:resource="http://europe.bourges.univ-orleans.fr/sites/default/files/download/Ontology/Core/kernel.owl#executesOn"/>
                <owl:onClass rdf:resource="http://europe.bourges.univ-orleans.fr/sites/default/files/download/Ontology/Core/system.owl#ComputationalHardware"/>
                <owl:minQualifiedCardinality rdf:datatype="&xsd;nonNegativeInteger">1</owl:minQualifiedCardinality>
            </owl:Restriction>
        </rdfs:subClassOf>
        <rdfs:subClassOf>
            <owl:Restriction>
                <owl:onProperty rdf:resource="http://europe.bourges.univ-orleans.fr/sites/default/files/download/Ontology/Core/kernel.owl#triggers"/>
                <owl:allValuesFrom>
                    <owl:Class>
                        <owl:unionOf rdf:parseType="Collection">
                            <rdf:Description rdf:about="http://europe.bourges.univ-orleans.fr/sites/default/files/download/Ontology/Core/kernel.owl#ApplicationInteraction"/>
                            <rdf:Description rdf:about="http://europe.bourges.univ-orleans.fr/sites/default/files/download/Ontology/Core/kernel.owl#DriverToHardwareInteraction"/>
                        </owl:unionOf>
                    </owl:Class>
                </owl:allValuesFrom>
            </owl:Restriction>
        </rdfs:subClassOf>
        <rdfs:subClassOf>
            <owl:Restriction>
                <owl:onProperty rdf:resource="http://europe.bourges.univ-orleans.fr/sites/default/files/download/Ontology/Core/kernel.owl#aggregates"/>
                <owl:allValuesFrom>
                    <owl:Class>
                        <owl:unionOf rdf:parseType="Collection">
                            <rdf:Description rdf:about="http://europe.bourges.univ-orleans.fr/sites/default/files/download/Ontology/Core/kernel.owl#Application"/>
                            <rdf:Description rdf:about="http://europe.bourges.univ-orleans.fr/sites/default/files/download/Ontology/Core/kernel.owl#SoftwareModule"/>
                        </owl:unionOf>
                    </owl:Class>
                </owl:allValuesFrom>
            </owl:Restriction>
        </rdfs:subClassOf>
        <openCycURI rdf:datatype="&xsd;anyURI">http://sw.opencyc.org/concept/Mx4rvcUMxZwpEbGdrcN5Y29ycA</openCycURI>
        <rdfs:comment xml:lang="en">This type of system represents Software, it can be an application, a framework, a library or an object  file....To actually execute it must be associated to some hardware but it does not need transformation done by an agent in order to be able to run on this hardware.

Considering what is software, it is in fact a state of the hardware supporting it. It is at some point the combination of electrical charges of some piece of semi-conductor. To distinghish it from the hardware is simply a way to categorise it and work with it.</rdfs:comment>
        <author xml:lang="en">creation PROTEUS Consortium - 
modification Bruno Patin - 13/10/2013
- update of associated comment</author>
    </owl:Class>
    


    <!-- http://europe.bourges.univ-orleans.fr/sites/default/files/download/Ontology/Core/kernel.owl#SoftwareModule -->

    <owl:Class rdf:about="http://europe.bourges.univ-orleans.fr/sites/default/files/download/Ontology/Core/kernel.owl#SoftwareModule">
        <rdfs:subClassOf rdf:resource="http://europe.bourges.univ-orleans.fr/sites/default/files/download/Ontology/Core/kernel.owl#Software"/>
        <rdfs:comment xml:lang="en">It is an application that is not executable by itself but can be composed through tooling such as RobotML platform.</rdfs:comment>
        <author xml:lang="en">creation PROTEUS consortium - 
modified Bruno Patin - 05/10/2013
- AlgorithmicModule renamed SoftwareModule. It is due to the fact that ApplicationInteraction name does not corresponds too well to its usage as FDriver, being also an application renders ambiguous usage of (DriverToHardware|HardwareToDriver)Interaction disjonction with AplicationInteractino.</author>
    </owl:Class>
    


    <!-- http://europe.bourges.univ-orleans.fr/sites/default/files/download/Ontology/Core/kernel.owl#SoftwareProbe -->

    <owl:Class rdf:about="http://europe.bourges.univ-orleans.fr/sites/default/files/download/Ontology/Core/kernel.owl#SoftwareProbe">
        <rdfs:subClassOf rdf:resource="http://europe.bourges.univ-orleans.fr/sites/default/files/download/Ontology/Core/kernel.owl#Application"/>
        <rdfs:subClassOf rdf:resource="http://europe.bourges.univ-orleans.fr/sites/default/files/download/Ontology/Core/kernel.owl#Probe"/>
        <rdfs:subClassOf>
            <owl:Restriction>
                <owl:onProperty rdf:resource="http://europe.bourges.univ-orleans.fr/sites/default/files/download/Ontology/Core/kernel.owl#observes"/>
                <owl:allValuesFrom rdf:resource="http://europe.bourges.univ-orleans.fr/sites/default/files/download/Ontology/Core/kernel.owl#AutomataState"/>
            </owl:Restriction>
        </rdfs:subClassOf>
        <rdfs:subClassOf>
            <owl:Restriction>
                <owl:onProperty rdf:resource="http://europe.bourges.univ-orleans.fr/sites/default/files/download/Ontology/Core/kernel.owl#produces"/>
                <owl:allValuesFrom rdf:resource="http://europe.bourges.univ-orleans.fr/sites/default/files/download/Ontology/Core/kernel.owl#Data"/>
            </owl:Restriction>
        </rdfs:subClassOf>
        <owl:disjointWith rdf:resource="http://europe.bourges.univ-orleans.fr/sites/default/files/download/Ontology/Core/kernel.owl#Wrapper"/>
        <rdfs:comment xml:lang="en">The software probe is able to provide data and not only information on the specific object states</rdfs:comment>
    </owl:Class>
    


    <!-- http://europe.bourges.univ-orleans.fr/sites/default/files/download/Ontology/Core/kernel.owl#State -->

    <owl:Class rdf:about="http://europe.bourges.univ-orleans.fr/sites/default/files/download/Ontology/Core/kernel.owl#State">
        <rdfs:subClassOf rdf:resource="http://europe.bourges.univ-orleans.fr/sites/default/files/download/Ontology/Core/kernel.owl#Abstraction"/>
        <rdfs:subClassOf>
            <owl:Restriction>
                <owl:onProperty rdf:resource="http://europe.bourges.univ-orleans.fr/sites/default/files/download/Ontology/Core/kernel.owl#hasStateVariables"/>
                <owl:minCardinality rdf:datatype="&xsd;nonNegativeInteger">1</owl:minCardinality>
            </owl:Restriction>
        </rdfs:subClassOf>
        <rdfs:comment xml:lang="en">The state expresses the fact that at some point in time (discrete or continuous expression of it), we will tag an object (interaction as well as component) and identify that it was as observed at this point. The fact that we need to &quot;measure&quot; values to identify the state of the object is of no concern here.</rdfs:comment>
        <author xml:lang="en">creation PROTEUS Consortium - 
modified Bruno Patin - 13/07/2014
- adaptation of comment in order to prepare Actual State definition</author>
    </owl:Class>
    


    <!-- http://europe.bourges.univ-orleans.fr/sites/default/files/download/Ontology/Core/kernel.owl#StateMachine -->

    <owl:Class rdf:about="http://europe.bourges.univ-orleans.fr/sites/default/files/download/Ontology/Core/kernel.owl#StateMachine">
        <rdfs:subClassOf rdf:resource="http://europe.bourges.univ-orleans.fr/sites/default/files/download/Ontology/Core/kernel.owl#Evolution"/>
        <rdfs:comment xml:lang="en">A discrete type of a evolution model is a finite state machine (FSM). A FSM has a finite set of states, a finite set of transitions between these states, an initial state and an end state. Activities can be associated to states.</rdfs:comment>
    </owl:Class>
    


    <!-- http://europe.bourges.univ-orleans.fr/sites/default/files/download/Ontology/Core/kernel.owl#StochasticEvolution -->

    <owl:Class rdf:about="http://europe.bourges.univ-orleans.fr/sites/default/files/download/Ontology/Core/kernel.owl#StochasticEvolution">
        <rdfs:subClassOf rdf:resource="http://europe.bourges.univ-orleans.fr/sites/default/files/download/Ontology/Core/kernel.owl#Evolution"/>
        <rdfs:comment xml:lang="en">Considering that evolution is stochastic is a philosophical point of view that considers that randomness is part of the fabric of the universe and if there is only one past, there could be many future due to that. So it is an Intrinsic property of any object to evolve through time with some random phenomenon intervention which would affect the course of the evolution. Thus 

To model Noise as a stochasticphenomenom is not the similar as considering a stochastic evolution world. It means that when modeling evolution as stochastic there will be a need to run many simulations to know the futy-ure trends and at this point The Noise Model and Biais Model would be considered as these random phenomenon that will be taken as inputs to determine many transitions for one previous state.</rdfs:comment>
        <author xml:lang="en">created PROTEUS Consortium - 
modified Bruno Patin - 21/06/2014
- renamed from StochasticEvolutionModel to StochasticEvolution
- adaptation of comment</author>
    </owl:Class>
    


    <!-- http://europe.bourges.univ-orleans.fr/sites/default/files/download/Ontology/Core/kernel.owl#System -->

    <owl:Class rdf:about="http://europe.bourges.univ-orleans.fr/sites/default/files/download/Ontology/Core/kernel.owl#System">
        <rdfs:subClassOf rdf:resource="&owl;Thing"/>
        <rdfs:subClassOf>
            <owl:Restriction>
                <owl:onProperty rdf:resource="http://europe.bourges.univ-orleans.fr/sites/default/files/download/Ontology/Core/kernel.owl#isAtomic"/>
                <owl:cardinality rdf:datatype="&xsd;nonNegativeInteger">1</owl:cardinality>
            </owl:Restriction>
        </rdfs:subClassOf>
        <owl:disjointWith rdf:resource="http://europe.bourges.univ-orleans.fr/sites/default/files/download/Ontology/Core/kernel.owl#Time"/>
        <owl:disjointWith rdf:resource="http://europe.bourges.univ-orleans.fr/sites/default/files/download/Ontology/Core/kernel.owl#Transition"/>
        <wikipediaURI rdf:datatype="&xsd;anyURI">http://en.wikipedia.org/wiki/System</wikipediaURI>
        <openCycURI rdf:datatype="&xsd;anyURI">http://sw.opencyc.org/concept/Mx4rv9Xu1ZwpEbGdrcN5Y29ycA</openCycURI>
        <author xml:lang="en">creation PROTEUS consortium - 
modified Bruno Patin - 30/09/2013
- modification of description to stick to what is a System in this ontology
modified Bruno Patin - 13/09/2013
- modification of description to describe what is this system description with respect to time...
</author>
        <rdfs:comment xml:lang="en">system IS object of the world but that there could be schematic (an actual concrete information) that could represent it (describe it thus). The world IS a system in our ontology. A system that models another means a concrete and actual &quot;in the world&quot; system (such as a simulator that is a software application) providing similar behaviour that another one (such as an aircraft).

The description done here is &quot;anhistoric&quot;. This means that what is described of the system is what is not depending of its life and thus of time. It is time and evolution that allows to have a system situated in the world. As an example, if we consider a robot, we will know it can have dimension, be created, walk or swim or whatever. We will not know that it is The robot built by hoover and nowadays used by Ms Smith that it&apos;s on and putting forks on the table at this very moment. These last elements need a specification of space and time to be available. and to know what it will do several minutes after, we will need to know its evolution...</rdfs:comment>
    </owl:Class>
    


    <!-- http://europe.bourges.univ-orleans.fr/sites/default/files/download/Ontology/Core/kernel.owl#Time -->

    <owl:Class rdf:about="http://europe.bourges.univ-orleans.fr/sites/default/files/download/Ontology/Core/kernel.owl#Time">
        <owl:disjointWith rdf:resource="http://europe.bourges.univ-orleans.fr/sites/default/files/download/Ontology/Core/kernel.owl#Transition"/>
        <openCycURI rdf:datatype="&xsd;anyURI">here we are speaking of duration... Is it time?
http://sw.opencyc.org/concept/Mx4rvViApZwpEbGdrcN5Y29ycA</openCycURI>
        <wikipediaURI rdf:datatype="&xsd;anyURI">http://en.wikipedia.org/wiki/Time</wikipediaURI>
        <rdfs:comment xml:lang="en">**Time** here is the concept that allows **Evolution** to occur. It is not said how it is represented but that it exists. It allows evolution to have a meaning.</rdfs:comment>
        <author xml:lang="en">creation PROTEUS Consortium - </author>
    </owl:Class>
    


    <!-- http://europe.bourges.univ-orleans.fr/sites/default/files/download/Ontology/Core/kernel.owl#TimeEvent -->

    <owl:Class rdf:about="http://europe.bourges.univ-orleans.fr/sites/default/files/download/Ontology/Core/kernel.owl#TimeEvent">
        <rdfs:subClassOf rdf:resource="http://europe.bourges.univ-orleans.fr/sites/default/files/download/Ontology/Core/kernel.owl#Event"/>
        <rdfs:comment xml:lang="en">Passage of a designated period of time from some time point. This kind of event occurs a duration after another event.</rdfs:comment>
    </owl:Class>
    


    <!-- http://europe.bourges.univ-orleans.fr/sites/default/files/download/Ontology/Core/kernel.owl#Transition -->

    <owl:Class rdf:about="http://europe.bourges.univ-orleans.fr/sites/default/files/download/Ontology/Core/kernel.owl#Transition">
        <TODO rdf:datatype="&xsd;anyURI">This description should be expanded to the generic system modelling we have here in this ontology. FSM is a way to model evolution model</TODO>
        <wiktionaryURI rdf:datatype="&xsd;anyURI">see 1st definition
http://en.wiktionary.org/wiki/transition</wiktionaryURI>
        <rdfs:comment xml:lang="en">The transition concept is closely linked to to the dynamic part of the ontology. It describes the period in which there is a change in the system. It is triggered by an event (internal or external to the system). Before the system is in its original state and then it has another one, its destination state. Transition can take time (duration) but the change is instantaneous at the end of the transition between origin and destination states.</rdfs:comment>
    </owl:Class>
    


    <!-- http://europe.bourges.univ-orleans.fr/sites/default/files/download/Ontology/Core/kernel.owl#Wrapper -->

    <owl:Class rdf:about="http://europe.bourges.univ-orleans.fr/sites/default/files/download/Ontology/Core/kernel.owl#Wrapper">
        <rdfs:subClassOf rdf:resource="http://europe.bourges.univ-orleans.fr/sites/default/files/download/Ontology/Core/kernel.owl#SoftwareModule"/>
        <rdfs:subClassOf>
            <owl:Restriction>
                <owl:onProperty rdf:resource="http://europe.bourges.univ-orleans.fr/sites/default/files/download/Ontology/Core/kernel.owl#triggers"/>
                <owl:allValuesFrom rdf:resource="http://europe.bourges.univ-orleans.fr/sites/default/files/download/Ontology/Core/kernel.owl#ApplicationInteraction"/>
            </owl:Restriction>
        </rdfs:subClassOf>
        <rdfs:comment xml:lang="en">It is an “application” that allows another “application” to use  “External algorithmic modules”. Part of its ports are linked to the application using the module and part of them are link to the module used. The goal of this application is thus to translate the dataflow from one application to the other</rdfs:comment>
    </owl:Class>
    


    <!-- http://europe.bourges.univ-orleans.fr/sites/default/files/download/Ontology/Core/system.owl#ComputationalHardware -->

    <owl:Class rdf:about="http://europe.bourges.univ-orleans.fr/sites/default/files/download/Ontology/Core/system.owl#ComputationalHardware">
        <rdfs:subClassOf rdf:resource="http://europe.bourges.univ-orleans.fr/sites/default/files/download/Ontology/Core/kernel.owl#Hardware"/>
    </owl:Class>
    


    <!-- http://www.w3.org/2002/07/owl#Thing -->

    <rdf:Description rdf:about="&owl;Thing">
        <rdfs:comment xml:lang="en">root of the whole PROTEUS ontology</rdfs:comment>
    </rdf:Description>
    


    <!-- 
    ///////////////////////////////////////////////////////////////////////////////////////
    //
    // Individuals
    //
    ///////////////////////////////////////////////////////////////////////////////////////
     -->

    


    <!-- http://europe.bourges.univ-orleans.fr/sites/default/files/download/Ontology/Core/kernel.owl#Earth -->

    <owl:NamedIndividual rdf:about="http://europe.bourges.univ-orleans.fr/sites/default/files/download/Ontology/Core/kernel.owl#Earth">
        <rdf:type rdf:resource="http://europe.bourges.univ-orleans.fr/sites/default/files/download/Ontology/Core/kernel.owl#PhysicalObject"/>
    </owl:NamedIndividual>
    


    <!-- http://europe.bourges.univ-orleans.fr/sites/default/files/download/Ontology/Core/kernel.owl#Gravity -->

    <owl:NamedIndividual rdf:about="http://europe.bourges.univ-orleans.fr/sites/default/files/download/Ontology/Core/kernel.owl#Gravity">
        <rdf:type rdf:resource="http://europe.bourges.univ-orleans.fr/sites/default/files/download/Ontology/Core/kernel.owl#PhysicalInteraction"/>
    </owl:NamedIndividual>
    


    <!-- http://europe.bourges.univ-orleans.fr/sites/default/files/download/Ontology/Core/kernel.owl#Me -->

    <owl:NamedIndividual rdf:about="http://europe.bourges.univ-orleans.fr/sites/default/files/download/Ontology/Core/kernel.owl#Me">
        <rdf:type rdf:resource="http://europe.bourges.univ-orleans.fr/sites/default/files/download/Ontology/Core/kernel.owl#Human"/>
    </owl:NamedIndividual>
    


    <!-- http://europe.bourges.univ-orleans.fr/sites/default/files/download/Ontology/Core/kernel.owl#Moon -->

    <owl:NamedIndividual rdf:about="http://europe.bourges.univ-orleans.fr/sites/default/files/download/Ontology/Core/kernel.owl#Moon">
        <rdf:type rdf:resource="http://europe.bourges.univ-orleans.fr/sites/default/files/download/Ontology/Core/kernel.owl#PhysicalObject"/>
    </owl:NamedIndividual>
    


    <!-- http://europe.bourges.univ-orleans.fr/sites/default/files/download/Ontology/Core/kernel.owl#Sun -->

    <owl:NamedIndividual rdf:about="http://europe.bourges.univ-orleans.fr/sites/default/files/download/Ontology/Core/kernel.owl#Sun">
        <rdf:type rdf:resource="http://europe.bourges.univ-orleans.fr/sites/default/files/download/Ontology/Core/kernel.owl#PhysicalObject"/>
    </owl:NamedIndividual>
    


    <!-- http://europe.bourges.univ-orleans.fr/sites/default/files/download/Ontology/Core/kernel.owl#Universe -->

    <owl:NamedIndividual rdf:about="http://europe.bourges.univ-orleans.fr/sites/default/files/download/Ontology/Core/kernel.owl#Universe">
        <rdf:type rdf:resource="http://europe.bourges.univ-orleans.fr/sites/default/files/download/Ontology/Core/kernel.owl#Environment"/>
        <isAtomic rdf:datatype="&xsd;boolean">false</isAtomic>
        <author xml:lang="en">Creation PROTEUS Consortium - 
modified Bruno Patin - 13/09/2014
- completion of the individual characteristics</author>
        <aggregates rdf:resource="http://europe.bourges.univ-orleans.fr/sites/default/files/download/Ontology/Core/kernel.owl#Earth"/>
        <aggregates rdf:resource="http://europe.bourges.univ-orleans.fr/sites/default/files/download/Ontology/Core/kernel.owl#Me"/>
        <aggregates rdf:resource="http://europe.bourges.univ-orleans.fr/sites/default/files/download/Ontology/Core/kernel.owl#Moon"/>
        <aggregates rdf:resource="http://europe.bourges.univ-orleans.fr/sites/default/files/download/Ontology/Core/kernel.owl#Sun"/>
    </owl:NamedIndividual>
    


    <!-- 
    ///////////////////////////////////////////////////////////////////////////////////////
    //
    // General axioms
    //
    ///////////////////////////////////////////////////////////////////////////////////////
     -->

    <rdf:Description>
        <rdf:type rdf:resource="&owl;AllDifferent"/>
        <owl:distinctMembers rdf:parseType="Collection">
            <rdf:Description rdf:about="http://europe.bourges.univ-orleans.fr/sites/default/files/download/Ontology/Core/kernel.owl#Earth"/>
            <rdf:Description rdf:about="http://europe.bourges.univ-orleans.fr/sites/default/files/download/Ontology/Core/kernel.owl#Me"/>
            <rdf:Description rdf:about="http://europe.bourges.univ-orleans.fr/sites/default/files/download/Ontology/Core/kernel.owl#Moon"/>
            <rdf:Description rdf:about="http://europe.bourges.univ-orleans.fr/sites/default/files/download/Ontology/Core/kernel.owl#Sun"/>
            <rdf:Description rdf:about="http://europe.bourges.univ-orleans.fr/sites/default/files/download/Ontology/Core/kernel.owl#Universe"/>
        </owl:distinctMembers>
    </rdf:Description>
    


    <!-- 
    ///////////////////////////////////////////////////////////////////////////////////////
    //
    // Rules
    //
    ///////////////////////////////////////////////////////////////////////////////////////
     -->

    <rdf:Description rdf:about="urn:swrl#x">
        <rdf:type rdf:resource="&swrl;Variable"/>
    </rdf:Description>
    <rdf:Description rdf:about="urn:swrl#z">
        <rdf:type rdf:resource="&swrl;Variable"/>
    </rdf:Description>
    <rdf:Description rdf:about="urn:swrl#y">
        <rdf:type rdf:resource="&swrl;Variable"/>
    </rdf:Description>
    <rdf:Description rdf:about="urn:swrl#a">
        <rdf:type rdf:resource="&swrl;Variable"/>
    </rdf:Description>
    <rdf:Description rdf:about="urn:swrl#b">
        <rdf:type rdf:resource="&swrl;Variable"/>
    </rdf:Description>
    <rdf:Description>
        <rdf:type rdf:resource="&swrl;Imp"/>
        <rdfs:comment xml:lang="en">if two physical objects are linked through a physical interaction then their associated frames are dependent one from the other.</rdfs:comment>
        <swrl:head>
            <rdf:Description>
                <rdf:type rdf:resource="&swrl;AtomList"/>
                <rdf:rest>
                    <rdf:Description>
                        <rdf:type rdf:resource="&swrl;AtomList"/>
                        <rdf:rest rdf:resource="&rdf;nil"/>
                        <rdf:first>
                            <rdf:Description>
                                <rdf:type rdf:resource="&swrl;IndividualPropertyAtom"/>
                                <swrl:propertyPredicate rdf:resource="http://europe.bourges.univ-orleans.fr/sites/default/files/download/Ontology/Core/kernel.owl#constrainsFrame"/>
                                <swrl:argument2 rdf:resource="urn:swrl#a"/>
                                <swrl:argument1 rdf:resource="urn:swrl#b"/>
                            </rdf:Description>
                        </rdf:first>
                    </rdf:Description>
                </rdf:rest>
                <rdf:first>
                    <rdf:Description>
                        <rdf:type rdf:resource="&swrl;IndividualPropertyAtom"/>
                        <swrl:propertyPredicate rdf:resource="http://europe.bourges.univ-orleans.fr/sites/default/files/download/Ontology/Core/kernel.owl#constrainsFrame"/>
                        <swrl:argument1 rdf:resource="urn:swrl#a"/>
                        <swrl:argument2 rdf:resource="urn:swrl#b"/>
                    </rdf:Description>
                </rdf:first>
            </rdf:Description>
        </swrl:head>
        <swrl:body>
            <rdf:Description>
                <rdf:type rdf:resource="&swrl;AtomList"/>
                <rdf:rest>
                    <rdf:Description>
                        <rdf:type rdf:resource="&swrl;AtomList"/>
                        <rdf:rest>
                            <rdf:Description>
                                <rdf:type rdf:resource="&swrl;AtomList"/>
                                <rdf:first>
                                    <rdf:Description>
                                        <rdf:type rdf:resource="&swrl;ClassAtom"/>
                                        <swrl:classPredicate rdf:resource="http://europe.bourges.univ-orleans.fr/sites/default/files/download/Ontology/Core/kernel.owl#PhysicalInteraction"/>
                                        <swrl:argument1 rdf:resource="urn:swrl#z"/>
                                    </rdf:Description>
                                </rdf:first>
                                <rdf:rest>
                                    <rdf:Description>
                                        <rdf:type rdf:resource="&swrl;AtomList"/>
                                        <rdf:rest>
                                            <rdf:Description>
                                                <rdf:type rdf:resource="&swrl;AtomList"/>
                                                <rdf:first>
                                                    <rdf:Description>
                                                        <rdf:type rdf:resource="&swrl;ClassAtom"/>
                                                        <swrl:classPredicate rdf:resource="http://europe.bourges.univ-orleans.fr/sites/default/files/download/Ontology/Core/kernel.owl#PhysicalObject"/>
                                                        <swrl:argument1 rdf:resource="urn:swrl#y"/>
                                                    </rdf:Description>
                                                </rdf:first>
                                                <rdf:rest>
                                                    <rdf:Description>
                                                        <rdf:type rdf:resource="&swrl;AtomList"/>
                                                        <rdf:rest>
                                                            <rdf:Description>
                                                                <rdf:type rdf:resource="&swrl;AtomList"/>
                                                                <rdf:rest>
                                                                    <rdf:Description>
                                                                        <rdf:type rdf:resource="&swrl;AtomList"/>
                                                                        <rdf:rest>
                                                                            <rdf:Description>
                                                                                <rdf:type rdf:resource="&swrl;AtomList"/>
                                                                                <rdf:rest rdf:resource="&rdf;nil"/>
                                                                                <rdf:first>
                                                                                    <rdf:Description>
                                                                                        <rdf:type rdf:resource="&swrl;IndividualPropertyAtom"/>
                                                                                        <swrl:propertyPredicate rdf:resource="http://europe.bourges.univ-orleans.fr/sites/default/files/download/Ontology/Core/kernel.owl#triggers"/>
                                                                                        <swrl:argument1 rdf:resource="urn:swrl#x"/>
                                                                                        <swrl:argument2 rdf:resource="urn:swrl#z"/>
                                                                                    </rdf:Description>
                                                                                </rdf:first>
                                                                            </rdf:Description>
                                                                        </rdf:rest>
                                                                        <rdf:first>
                                                                            <rdf:Description>
                                                                                <rdf:type rdf:resource="&swrl;IndividualPropertyAtom"/>
                                                                                <swrl:propertyPredicate rdf:resource="http://europe.bourges.univ-orleans.fr/sites/default/files/download/Ontology/Core/kernel.owl#impacts"/>
                                                                                <swrl:argument2 rdf:resource="urn:swrl#y"/>
                                                                                <swrl:argument1 rdf:resource="urn:swrl#z"/>
                                                                            </rdf:Description>
                                                                        </rdf:first>
                                                                    </rdf:Description>
                                                                </rdf:rest>
                                                                <rdf:first>
                                                                    <rdf:Description>
                                                                        <rdf:type rdf:resource="&swrl;IndividualPropertyAtom"/>
                                                                        <swrl:propertyPredicate rdf:resource="http://europe.bourges.univ-orleans.fr/sites/default/files/download/Ontology/Core/kernel.owl#definesAFrame"/>
                                                                        <swrl:argument2 rdf:resource="urn:swrl#b"/>
                                                                        <swrl:argument1 rdf:resource="urn:swrl#y"/>
                                                                    </rdf:Description>
                                                                </rdf:first>
                                                            </rdf:Description>
                                                        </rdf:rest>
                                                        <rdf:first>
                                                            <rdf:Description>
                                                                <rdf:type rdf:resource="&swrl;IndividualPropertyAtom"/>
                                                                <swrl:propertyPredicate rdf:resource="http://europe.bourges.univ-orleans.fr/sites/default/files/download/Ontology/Core/kernel.owl#definesAFrame"/>
                                                                <swrl:argument2 rdf:resource="urn:swrl#a"/>
                                                                <swrl:argument1 rdf:resource="urn:swrl#x"/>
                                                            </rdf:Description>
                                                        </rdf:first>
                                                    </rdf:Description>
                                                </rdf:rest>
                                            </rdf:Description>
                                        </rdf:rest>
                                        <rdf:first>
                                            <rdf:Description>
                                                <rdf:type rdf:resource="&swrl;ClassAtom"/>
                                                <swrl:classPredicate rdf:resource="http://europe.bourges.univ-orleans.fr/sites/default/files/download/Ontology/Core/kernel.owl#PhysicalObject"/>
                                                <swrl:argument1 rdf:resource="urn:swrl#x"/>
                                            </rdf:Description>
                                        </rdf:first>
                                    </rdf:Description>
                                </rdf:rest>
                            </rdf:Description>
                        </rdf:rest>
                        <rdf:first>
                            <rdf:Description>
                                <rdf:type rdf:resource="&swrl;ClassAtom"/>
                                <swrl:classPredicate rdf:resource="http://europe.bourges.univ-orleans.fr/sites/default/files/download/Ontology/Core/kernel.owl#Frame"/>
                                <swrl:argument1 rdf:resource="urn:swrl#b"/>
                            </rdf:Description>
                        </rdf:first>
                    </rdf:Description>
                </rdf:rest>
                <rdf:first>
                    <rdf:Description>
                        <rdf:type rdf:resource="&swrl;ClassAtom"/>
                        <swrl:classPredicate rdf:resource="http://europe.bourges.univ-orleans.fr/sites/default/files/download/Ontology/Core/kernel.owl#Frame"/>
                        <swrl:argument1 rdf:resource="urn:swrl#a"/>
                    </rdf:Description>
                </rdf:first>
            </rdf:Description>
        </swrl:body>
    </rdf:Description>
    <rdf:Description>
        <rdf:type rdf:resource="&swrl;Imp"/>
        <rdfs:comment xml:lang="en">this rule enforces the fact that if a physical object triggers an  action then it is an agent.</rdfs:comment>
        <swrl:head>
            <rdf:Description>
                <rdf:type rdf:resource="&swrl;AtomList"/>
                <rdf:rest rdf:resource="&rdf;nil"/>
                <rdf:first>
                    <rdf:Description>
                        <rdf:type rdf:resource="&swrl;ClassAtom"/>
                        <swrl:classPredicate rdf:resource="http://europe.bourges.univ-orleans.fr/sites/default/files/download/Ontology/Core/kernel.owl#Agent"/>
                        <swrl:argument1 rdf:resource="urn:swrl#x"/>
                    </rdf:Description>
                </rdf:first>
            </rdf:Description>
        </swrl:head>
        <swrl:body>
            <rdf:Description>
                <rdf:type rdf:resource="&swrl;AtomList"/>
                <rdf:rest>
                    <rdf:Description>
                        <rdf:type rdf:resource="&swrl;AtomList"/>
                        <rdf:rest>
                            <rdf:Description>
                                <rdf:type rdf:resource="&swrl;AtomList"/>
                                <rdf:rest rdf:resource="&rdf;nil"/>
                                <rdf:first>
                                    <rdf:Description>
                                        <rdf:type rdf:resource="&swrl;IndividualPropertyAtom"/>
                                        <swrl:propertyPredicate rdf:resource="http://europe.bourges.univ-orleans.fr/sites/default/files/download/Ontology/Core/kernel.owl#triggers"/>
                                        <swrl:argument1 rdf:resource="urn:swrl#x"/>
                                        <swrl:argument2 rdf:resource="urn:swrl#y"/>
                                    </rdf:Description>
                                </rdf:first>
                            </rdf:Description>
                        </rdf:rest>
                        <rdf:first>
                            <rdf:Description>
                                <rdf:type rdf:resource="&swrl;ClassAtom"/>
                                <swrl:classPredicate rdf:resource="http://europe.bourges.univ-orleans.fr/sites/default/files/download/Ontology/Core/kernel.owl#PhysicalObject"/>
                                <swrl:argument1 rdf:resource="urn:swrl#x"/>
                            </rdf:Description>
                        </rdf:first>
                    </rdf:Description>
                </rdf:rest>
                <rdf:first>
                    <rdf:Description>
                        <rdf:type rdf:resource="&swrl;ClassAtom"/>
                        <swrl:classPredicate rdf:resource="http://europe.bourges.univ-orleans.fr/sites/default/files/download/Ontology/Core/kernel.owl#Action"/>
                        <swrl:argument1 rdf:resource="urn:swrl#y"/>
                    </rdf:Description>
                </rdf:first>
            </rdf:Description>
        </swrl:body>
    </rdf:Description>
    <rdf:Description>
        <rdf:type rdf:resource="&swrl;Imp"/>
        <rdfs:comment xml:lang="en">If the port of a system emits an interaction then this interaction is triggered by the system.</rdfs:comment>
        <swrl:body>
            <rdf:Description>
                <rdf:type rdf:resource="&swrl;AtomList"/>
                <rdf:first>
                    <rdf:Description>
                        <rdf:type rdf:resource="&swrl;ClassAtom"/>
                        <swrl:classPredicate rdf:resource="http://europe.bourges.univ-orleans.fr/sites/default/files/download/Ontology/Core/kernel.owl#Interaction"/>
                        <swrl:argument1 rdf:resource="urn:swrl#y"/>
                    </rdf:Description>
                </rdf:first>
                <rdf:rest>
                    <rdf:Description>
                        <rdf:type rdf:resource="&swrl;AtomList"/>
                        <rdf:first>
                            <rdf:Description>
                                <rdf:type rdf:resource="&swrl;ClassAtom"/>
                                <swrl:classPredicate rdf:resource="http://europe.bourges.univ-orleans.fr/sites/default/files/download/Ontology/Core/kernel.owl#Port"/>
                                <swrl:argument1 rdf:resource="urn:swrl#z"/>
                            </rdf:Description>
                        </rdf:first>
                        <rdf:rest>
                            <rdf:Description>
                                <rdf:type rdf:resource="&swrl;AtomList"/>
                                <rdf:first>
                                    <rdf:Description>
                                        <rdf:type rdf:resource="&swrl;ClassAtom"/>
                                        <swrl:classPredicate rdf:resource="http://europe.bourges.univ-orleans.fr/sites/default/files/download/Ontology/Core/kernel.owl#System"/>
                                        <swrl:argument1 rdf:resource="urn:swrl#x"/>
                                    </rdf:Description>
                                </rdf:first>
                                <rdf:rest>
                                    <rdf:Description>
                                        <rdf:type rdf:resource="&swrl;AtomList"/>
                                        <rdf:first>
                                            <rdf:Description>
                                                <rdf:type rdf:resource="&swrl;IndividualPropertyAtom"/>
                                                <swrl:propertyPredicate rdf:resource="http://europe.bourges.univ-orleans.fr/sites/default/files/download/Ontology/Core/kernel.owl#emits"/>
                                                <swrl:argument2 rdf:resource="urn:swrl#y"/>
                                                <swrl:argument1 rdf:resource="urn:swrl#z"/>
                                            </rdf:Description>
                                        </rdf:first>
                                        <rdf:rest>
                                            <rdf:Description>
                                                <rdf:type rdf:resource="&swrl;AtomList"/>
                                                <rdf:rest rdf:resource="&rdf;nil"/>
                                                <rdf:first>
                                                    <rdf:Description>
                                                        <rdf:type rdf:resource="&swrl;IndividualPropertyAtom"/>
                                                        <swrl:propertyPredicate rdf:resource="http://europe.bourges.univ-orleans.fr/sites/default/files/download/Ontology/Core/kernel.owl#hasPort"/>
                                                        <swrl:argument1 rdf:resource="urn:swrl#x"/>
                                                        <swrl:argument2 rdf:resource="urn:swrl#z"/>
                                                    </rdf:Description>
                                                </rdf:first>
                                            </rdf:Description>
                                        </rdf:rest>
                                    </rdf:Description>
                                </rdf:rest>
                            </rdf:Description>
                        </rdf:rest>
                    </rdf:Description>
                </rdf:rest>
            </rdf:Description>
        </swrl:body>
        <swrl:head>
            <rdf:Description>
                <rdf:type rdf:resource="&swrl;AtomList"/>
                <rdf:rest rdf:resource="&rdf;nil"/>
                <rdf:first>
                    <rdf:Description>
                        <rdf:type rdf:resource="&swrl;IndividualPropertyAtom"/>
                        <swrl:propertyPredicate rdf:resource="http://europe.bourges.univ-orleans.fr/sites/default/files/download/Ontology/Core/kernel.owl#triggers"/>
                        <swrl:argument1 rdf:resource="urn:swrl#x"/>
                        <swrl:argument2 rdf:resource="urn:swrl#y"/>
                    </rdf:Description>
                </rdf:first>
            </rdf:Description>
        </swrl:head>
    </rdf:Description>
    <rdf:Description>
        <rdf:type rdf:resource="&swrl;Imp"/>
        <rdfs:comment xml:lang="en">a frame is defined by a physical system. Another frame positioned in this defined frame has to be different as dependent on it</rdfs:comment>
        <swrl:body>
            <rdf:Description>
                <rdf:type rdf:resource="&swrl;AtomList"/>
                <rdf:rest>
                    <rdf:Description>
                        <rdf:type rdf:resource="&swrl;AtomList"/>
                        <rdf:rest rdf:resource="&rdf;nil"/>
                        <rdf:first>
                            <rdf:Description>
                                <rdf:type rdf:resource="&swrl;IndividualPropertyAtom"/>
                                <swrl:propertyPredicate rdf:resource="http://europe.bourges.univ-orleans.fr/sites/default/files/download/Ontology/Core/kernel.owl#isPositionedIn"/>
                                <swrl:argument1 rdf:resource="urn:swrl#x"/>
                                <swrl:argument2 rdf:resource="urn:swrl#y"/>
                            </rdf:Description>
                        </rdf:first>
                    </rdf:Description>
                </rdf:rest>
                <rdf:first>
                    <rdf:Description>
                        <rdf:type rdf:resource="&swrl;IndividualPropertyAtom"/>
                        <swrl:propertyPredicate rdf:resource="http://europe.bourges.univ-orleans.fr/sites/default/files/download/Ontology/Core/kernel.owl#definesAFrame"/>
                        <swrl:argument1 rdf:resource="urn:swrl#x"/>
                        <swrl:argument2 rdf:resource="urn:swrl#z"/>
                    </rdf:Description>
                </rdf:first>
            </rdf:Description>
        </swrl:body>
        <swrl:head>
            <rdf:Description>
                <rdf:type rdf:resource="&swrl;AtomList"/>
                <rdf:rest rdf:resource="&rdf;nil"/>
                <rdf:first>
                    <rdf:Description>
                        <rdf:type rdf:resource="&swrl;DifferentIndividualsAtom"/>
                        <swrl:argument1 rdf:resource="urn:swrl#y"/>
                        <swrl:argument2 rdf:resource="urn:swrl#z"/>
                    </rdf:Description>
                </rdf:first>
            </rdf:Description>
        </swrl:head>
    </rdf:Description>
    <rdf:Description>
        <rdf:type rdf:resource="&swrl;Imp"/>
        <rdfs:comment xml:lang="en">if a system is the result of the aggregation of one system or more then it is a composite system and this is tagged by the isAtmic proprty set to false.</rdfs:comment>
        <swrl:body>
            <rdf:Description>
                <rdf:type rdf:resource="&swrl;AtomList"/>
                <rdf:first>
                    <rdf:Description>
                        <rdf:type rdf:resource="&swrl;ClassAtom"/>
                        <swrl:classPredicate rdf:resource="http://europe.bourges.univ-orleans.fr/sites/default/files/download/Ontology/Core/kernel.owl#System"/>
                        <swrl:argument1 rdf:resource="urn:swrl#x"/>
                    </rdf:Description>
                </rdf:first>
                <rdf:rest>
                    <rdf:Description>
                        <rdf:type rdf:resource="&swrl;AtomList"/>
                        <rdf:rest>
                            <rdf:Description>
                                <rdf:type rdf:resource="&swrl;AtomList"/>
                                <rdf:rest rdf:resource="&rdf;nil"/>
                                <rdf:first>
                                    <rdf:Description>
                                        <rdf:type rdf:resource="&swrl;IndividualPropertyAtom"/>
                                        <swrl:propertyPredicate rdf:resource="http://europe.bourges.univ-orleans.fr/sites/default/files/download/Ontology/Core/kernel.owl#aggregates"/>
                                        <swrl:argument1 rdf:resource="urn:swrl#x"/>
                                        <swrl:argument2 rdf:resource="urn:swrl#y"/>
                                    </rdf:Description>
                                </rdf:first>
                            </rdf:Description>
                        </rdf:rest>
                        <rdf:first>
                            <rdf:Description>
                                <rdf:type rdf:resource="&swrl;ClassAtom"/>
                                <swrl:classPredicate rdf:resource="http://europe.bourges.univ-orleans.fr/sites/default/files/download/Ontology/Core/kernel.owl#System"/>
                                <swrl:argument1 rdf:resource="urn:swrl#y"/>
                            </rdf:Description>
                        </rdf:first>
                    </rdf:Description>
                </rdf:rest>
            </rdf:Description>
        </swrl:body>
        <swrl:head>
            <rdf:Description>
                <rdf:type rdf:resource="&swrl;AtomList"/>
                <rdf:rest rdf:resource="&rdf;nil"/>
                <rdf:first>
                    <rdf:Description>
                        <rdf:type rdf:resource="&swrl;DatavaluedPropertyAtom"/>
                        <swrl:argument2 rdf:datatype="&xsd;boolean">false</swrl:argument2>
                        <swrl:propertyPredicate rdf:resource="http://europe.bourges.univ-orleans.fr/sites/default/files/download/Ontology/Core/kernel.owl#isAtomic"/>
                        <swrl:argument1 rdf:resource="urn:swrl#x"/>
                    </rdf:Description>
                </rdf:first>
            </rdf:Description>
        </swrl:head>
    </rdf:Description>
    <rdf:Description>
        <rdf:type rdf:resource="&swrl;Imp"/>
        <rdfs:comment xml:lang="en">a physical object able to build some hardware implies the physical object to be a human</rdfs:comment>
        <swrl:body>
            <rdf:Description>
                <rdf:type rdf:resource="&swrl;AtomList"/>
                <rdf:rest>
                    <rdf:Description>
                        <rdf:type rdf:resource="&swrl;AtomList"/>
                        <rdf:first>
                            <rdf:Description>
                                <rdf:type rdf:resource="&swrl;ClassAtom"/>
                                <swrl:classPredicate rdf:resource="http://europe.bourges.univ-orleans.fr/sites/default/files/download/Ontology/Core/kernel.owl#PhysicalObject"/>
                                <swrl:argument1 rdf:resource="urn:swrl#x"/>
                            </rdf:Description>
                        </rdf:first>
                        <rdf:rest>
                            <rdf:Description>
                                <rdf:type rdf:resource="&swrl;AtomList"/>
                                <rdf:rest rdf:resource="&rdf;nil"/>
                                <rdf:first>
                                    <rdf:Description>
                                        <rdf:type rdf:resource="&swrl;IndividualPropertyAtom"/>
                                        <swrl:propertyPredicate rdf:resource="http://europe.bourges.univ-orleans.fr/sites/default/files/download/Ontology/Core/kernel.owl#triggers"/>
                                        <swrl:argument1 rdf:resource="urn:swrl#x"/>
                                        <swrl:argument2 rdf:resource="urn:swrl#y"/>
                                    </rdf:Description>
                                </rdf:first>
                            </rdf:Description>
                        </rdf:rest>
                    </rdf:Description>
                </rdf:rest>
                <rdf:first>
                    <rdf:Description>
                        <rdf:type rdf:resource="&swrl;ClassAtom"/>
                        <swrl:classPredicate rdf:resource="http://europe.bourges.univ-orleans.fr/sites/default/files/download/Ontology/Core/kernel.owl#Build"/>
                        <swrl:argument1 rdf:resource="urn:swrl#y"/>
                    </rdf:Description>
                </rdf:first>
            </rdf:Description>
        </swrl:body>
        <swrl:head>
            <rdf:Description>
                <rdf:type rdf:resource="&swrl;AtomList"/>
                <rdf:rest rdf:resource="&rdf;nil"/>
                <rdf:first>
                    <rdf:Description>
                        <rdf:type rdf:resource="&swrl;ClassAtom"/>
                        <swrl:classPredicate rdf:resource="http://europe.bourges.univ-orleans.fr/sites/default/files/download/Ontology/Core/kernel.owl#Human"/>
                        <swrl:argument1 rdf:resource="urn:swrl#x"/>
                    </rdf:Description>
                </rdf:first>
            </rdf:Description>
        </swrl:head>
    </rdf:Description>
</rdf:RDF>



<!-- Generated by the OWL API (version 3.5.1) http://owlapi.sourceforge.net -->

