<?xml version="1.0"?>


<!DOCTYPE rdf:RDF [
    <!ENTITY owl "http://www.w3.org/2002/07/owl#" >
    <!ENTITY swrl "http://www.w3.org/2003/11/swrl#" >
    <!ENTITY swrlb "http://www.w3.org/2003/11/swrlb#" >
    <!ENTITY xsd "http://www.w3.org/2001/XMLSchema#" >
    <!ENTITY rdfs "http://www.w3.org/2000/01/rdf-schema#" >
    <!ENTITY rdf "http://www.w3.org/1999/02/22-rdf-syntax-ns#" >
    <!ENTITY protege "http://protege.stanford.edu/plugins/owl/protege#" >
    <!ENTITY xsp "http://www.owl-ontologies.com/2005/08/07/xsp.owl#" >
    <!ENTITY swrla "http://swrl.stanford.edu/ontologies/3.3/swrla.owl#" >
    <!ENTITY sqwrl "http://sqwrl.stanford.edu/ontologies/built-ins/3.4/sqwrl.owl#" >
    <!ENTITY robo "http://europe.bourges.univ-orleans.fr/sites/default/files/download/Ontology/Core/robot.owl#" >
    <!ENTITY syst "http://europe.bourges.univ-orleans.fr/sites/default/files/download/Ontology/Core/system.owl#" >
    <!ENTITY kern "http://europe.bourges.univ-orleans.fr/sites/default/files/download/Ontology/Core/kernel.owl#" >
    <!ENTITY info "http://europe.bourges.univ-orleans.fr/sites/default/files/download/Ontology/Core/information.owl#" >
    <!ENTITY envi "http://europe.bourges.univ-orleans.fr/sites/default/files/download/Ontology/Core/environment.owl#" >
]>


<rdf:RDF xmlns="http://europe.bourges.univ-orleans.fr/sites/default/files/download/Ontology/Core/robot.owl#"
     xml:base="http://europe.bourges.univ-orleans.fr/sites/default/files/download/Ontology/Core/robot.owl"
     xmlns:protege="http://protege.stanford.edu/plugins/owl/protege#"
     xmlns:xsp="http://www.owl-ontologies.com/2005/08/07/xsp.owl#"
     xmlns:robo="http://europe.bourges.univ-orleans.fr/sites/default/files/download/Ontology/Core/robot.owl#"
     xmlns:kern="http://europe.bourges.univ-orleans.fr/sites/default/files/download/Ontology/Core/kernel.owl#"
     xmlns:info="http://europe.bourges.univ-orleans.fr/sites/default/files/download/Ontology/Core/information.owl#"
     xmlns:sqwrl="http://sqwrl.stanford.edu/ontologies/built-ins/3.4/sqwrl.owl#"
     xmlns:rdfs="http://www.w3.org/2000/01/rdf-schema#"
     xmlns:swrl="http://www.w3.org/2003/11/swrl#"
     xmlns:envi="http://europe.bourges.univ-orleans.fr/sites/default/files/download/Ontology/Core/environment.owl#"
     xmlns:syst="http://europe.bourges.univ-orleans.fr/sites/default/files/download/Ontology/Core/system.owl#"
     xmlns:xsd="http://www.w3.org/2001/XMLSchema#"
     xmlns:owl="http://www.w3.org/2002/07/owl#"
     xmlns:swrlb="http://www.w3.org/2003/11/swrlb#"
     xmlns:rdf="http://www.w3.org/1999/02/22-rdf-syntax-ns#"
     xmlns:swrla="http://swrl.stanford.edu/ontologies/3.3/swrla.owl#">
    <owl:Ontology rdf:about="http://europe.bourges.univ-orleans.fr/sites/default/files/download/Ontology/Core/robot.owl">
        <owl:versionInfo rdf:datatype="&xsd;string">version delivered 1.0</owl:versionInfo>
        <rdfs:comment xml:lang="en">FaCT++ does not work with this ontology. HermiT shall be used for reasoning.</rdfs:comment>
        <rdfs:comment xml:lang="en">This ontology describes the robot field providing their classification</rdfs:comment>
        <rdfs:comment xml:lang="en">This work is based upon a previous one funded by the French Research agency ANR (Agence Nationale de la Recherche) through thePROTEUS project (see http://www.anr-project.fr). It is the property of its authors and is governed by the CECILL B V1 licence (see http://www.cecill.info for information and the associated Licence_CeCILL-B_V1-en.txt or Licence_CeCILL-B_V1-fr.txt files).</rdfs:comment>
        <rdfs:comment xml:lang="en">Version for Protégé 4.x flavors.</rdfs:comment>
        <owl:imports rdf:resource="http://europe.bourges.univ-orleans.fr/sites/default/files/download/Ontology/Core/environment.owl"/>
        <owl:imports rdf:resource="http://europe.bourges.univ-orleans.fr/sites/default/files/download/Ontology/Core/kernel.owl"/>
        <owl:imports rdf:resource="http://europe.bourges.univ-orleans.fr/sites/default/files/download/Ontology/Core/system.owl"/>
        <owl:imports rdf:resource="http://sqwrl.stanford.edu/ontologies/built-ins/3.4/sqwrl.owl"/>
        <owl:imports rdf:resource="http://swrl.stanford.edu/ontologies/3.3/swrla.owl"/>
    </owl:Ontology>
    


    <!-- 
    ///////////////////////////////////////////////////////////////////////////////////////
    //
    // Object Properties
    //
    ///////////////////////////////////////////////////////////////////////////////////////
     -->

    


    <!-- http://europe.bourges.univ-orleans.fr/sites/default/files/download/Ontology/Core/robot.owl#movesIn -->

    <owl:ObjectProperty rdf:about="&robo;movesIn">
        <rdfs:comment xml:lang="en">The movesIn property expresses the fact that *PhysicalObject*s may have &quot;engines&quot; that moves them from their own volition (they will be *Agent*) or supervised externally (they will be *MobileRobots* such as an aircraft or a car or whatever)</rdfs:comment>
        <kern:author xml:lang="en">creation PROTEUS Consortium - 
modified Bruno Patin - 04/08/2014
- comment modified as it was strictly speaking of robots</kern:author>
        <rdfs:subPropertyOf rdf:resource="&envi;evolvesIn"/>
        <rdfs:range rdf:resource="&kern;PhysicalObject"/>
        <rdfs:domain>
            <owl:Class>
                <owl:unionOf rdf:parseType="Collection">
                    <rdf:Description rdf:about="&kern;Human"/>
                    <rdf:Description rdf:about="&robo;MobileRobot"/>
                </owl:unionOf>
            </owl:Class>
        </rdfs:domain>
    </owl:ObjectProperty>
    


    <!-- http://europe.bourges.univ-orleans.fr/sites/default/files/download/Ontology/Core/robot.owl#movesInAtmosphere -->

    <owl:ObjectProperty rdf:about="&robo;movesInAtmosphere">
        <rdfs:comment xml:lang="en">UAV move in atmosphere.</rdfs:comment>
        <rdfs:range rdf:resource="&envi;Atmosphere"/>
        <rdfs:subPropertyOf rdf:resource="&robo;movesIn"/>
        <rdfs:domain>
            <owl:Class>
                <owl:unionOf rdf:parseType="Collection">
                    <rdf:Description rdf:about="&robo;AirRobot"/>
                    <rdf:Description rdf:about="&robo;HybridRobot"/>
                </owl:unionOf>
            </owl:Class>
        </rdfs:domain>
    </owl:ObjectProperty>
    


    <!-- http://europe.bourges.univ-orleans.fr/sites/default/files/download/Ontology/Core/robot.owl#movesInWaterbody -->

    <owl:ObjectProperty rdf:about="&robo;movesInWaterbody">
        <rdfs:comment xml:lang="en">UUV and diving humans move in waterbodies.</rdfs:comment>
        <rdfs:range rdf:resource="&envi;Waterbody"/>
        <rdfs:subPropertyOf rdf:resource="&robo;movesIn"/>
        <rdfs:domain>
            <owl:Class>
                <owl:unionOf rdf:parseType="Collection">
                    <rdf:Description rdf:about="&kern;Human"/>
                    <rdf:Description rdf:about="&robo;HybridRobot"/>
                    <rdf:Description rdf:about="&robo;UnderwaterRobot"/>
                </owl:unionOf>
            </owl:Class>
        </rdfs:domain>
    </owl:ObjectProperty>
    


    <!-- http://europe.bourges.univ-orleans.fr/sites/default/files/download/Ontology/Core/robot.owl#movesOver -->

    <owl:ObjectProperty rdf:about="&robo;movesOver">
        <rdfs:comment xml:lang="en">Some robots moves over a ground surface or a surface of a waterbody</rdfs:comment>
        <rdfs:range rdf:resource="&envi;Surface"/>
        <rdfs:subPropertyOf rdf:resource="&envi;evolvesIn"/>
        <rdfs:domain>
            <owl:Class>
                <owl:unionOf rdf:parseType="Collection">
                    <rdf:Description rdf:about="&kern;Human"/>
                    <rdf:Description rdf:about="&robo;MobileRobot"/>
                </owl:unionOf>
            </owl:Class>
        </rdfs:domain>
    </owl:ObjectProperty>
    


    <!-- http://europe.bourges.univ-orleans.fr/sites/default/files/download/Ontology/Core/robot.owl#movesOverGround -->

    <owl:ObjectProperty rdf:about="&robo;movesOverGround">
        <rdfs:comment xml:lang="en">UGV and humans move over stairs, floor and land surface.</rdfs:comment>
        <rdfs:subPropertyOf rdf:resource="&robo;movesOver"/>
        <rdfs:domain>
            <owl:Class>
                <owl:unionOf rdf:parseType="Collection">
                    <rdf:Description rdf:about="&kern;Human"/>
                    <rdf:Description rdf:about="&robo;GroundRobot"/>
                    <rdf:Description rdf:about="&robo;HybridRobot"/>
                </owl:unionOf>
            </owl:Class>
        </rdfs:domain>
        <rdfs:range>
            <owl:Class>
                <owl:unionOf rdf:parseType="Collection">
                    <rdf:Description rdf:about="&envi;Floor"/>
                    <rdf:Description rdf:about="&envi;LandSurface"/>
                    <rdf:Description rdf:about="&envi;Stairs"/>
                </owl:unionOf>
            </owl:Class>
        </rdfs:range>
    </owl:ObjectProperty>
    


    <!-- http://europe.bourges.univ-orleans.fr/sites/default/files/download/Ontology/Core/robot.owl#movesOverWatersurface -->

    <owl:ObjectProperty rdf:about="&robo;movesOverWatersurface">
        <rdfs:comment xml:lang="en">USV and swiming humans move over watersurface</rdfs:comment>
        <rdfs:range rdf:resource="&envi;WaterSurface"/>
        <rdfs:subPropertyOf rdf:resource="&robo;movesOver"/>
        <rdfs:domain>
            <owl:Class>
                <owl:unionOf rdf:parseType="Collection">
                    <rdf:Description rdf:about="&kern;Human"/>
                    <rdf:Description rdf:about="&robo;HybridRobot"/>
                    <rdf:Description rdf:about="&robo;SurfaceRobot"/>
                </owl:unionOf>
            </owl:Class>
        </rdfs:domain>
    </owl:ObjectProperty>
    


    <!-- http://europe.bourges.univ-orleans.fr/sites/default/files/download/Ontology/Core/robot.owl#pilots -->

    <owl:ObjectProperty rdf:about="&robo;pilots">
        <rdfs:comment xml:lang="en">A human agent can drive a robotic Vehicle (AV, GV, SV, UV), this action will be achieved on these piloted systems.</rdfs:comment>
        <rdfs:domain rdf:resource="&kern;Human"/>
        <rdfs:range rdf:resource="&robo;PilotedSystem"/>
    </owl:ObjectProperty>
    


    <!-- http://europe.bourges.univ-orleans.fr/sites/default/files/download/Ontology/Core/robot.owl#uses -->

    <owl:ObjectProperty rdf:about="&robo;uses">
        <rdfs:comment xml:lang="en">A robot needs on or multiple robotic middleware to makes all the application of its robotic systems works.</rdfs:comment>
        <rdfs:domain rdf:resource="&robo;Robot"/>
        <rdfs:range rdf:resource="&syst;RoboticMiddleware"/>
    </owl:ObjectProperty>
    


    <!-- 
    ///////////////////////////////////////////////////////////////////////////////////////
    //
    // Classes
    //
    ///////////////////////////////////////////////////////////////////////////////////////
     -->

    


    <!-- http://europe.bourges.univ-orleans.fr/sites/default/files/download/Ontology/Core/kernel.owl#Environment -->

    <rdf:Description rdf:about="&kern;Environment">
        <owl:disjointWith rdf:resource="&robo;GlobalPlatform"/>
        <owl:disjointWith rdf:resource="&robo;Robot"/>
    </rdf:Description>
    


    <!-- http://europe.bourges.univ-orleans.fr/sites/default/files/download/Ontology/Core/kernel.owl#Human -->

    <rdf:Description rdf:about="&kern;Human">
        <owl:disjointWith rdf:resource="&robo;Robot"/>
    </rdf:Description>
    


    <!-- http://europe.bourges.univ-orleans.fr/sites/default/files/download/Ontology/Core/robot.owl#AirRobot -->

    <owl:Class rdf:about="&robo;AirRobot">
        <rdfs:subClassOf rdf:resource="&robo;MobileRobot"/>
        <rdfs:subClassOf>
            <owl:Restriction>
                <owl:onProperty rdf:resource="&robo;movesIn"/>
                <owl:someValuesFrom rdf:resource="&envi;Atmosphere"/>
            </owl:Restriction>
        </rdfs:subClassOf>
        <owl:disjointWith rdf:resource="&robo;GroundRobot"/>
        <owl:disjointWith rdf:resource="&robo;HybridRobot"/>
        <owl:disjointWith rdf:resource="&robo;SurfaceRobot"/>
        <owl:disjointWith rdf:resource="&robo;UnderwaterRobot"/>
        <kern:author xml:lang="en">20/06/2014 - Bruno Patin
- renamed from AirVehicle to AirRobot</kern:author>
        <rdfs:comment xml:lang="en">Air robots are those able to move in air.
Only aircraft with either fixed (like planes) either rotary (like helicopters) wings are considered in this definition.</rdfs:comment>
        <kern:TODO xml:lang="en">there must be linked somewhat like a chassis but there is a specific aeronautical wording.</kern:TODO>
    </owl:Class>
    


    <!-- http://europe.bourges.univ-orleans.fr/sites/default/files/download/Ontology/Core/robot.owl#AutonomousRobot -->

    <owl:Class rdf:about="&robo;AutonomousRobot">
        <rdfs:subClassOf rdf:resource="&kern;Agent"/>
        <rdfs:subClassOf rdf:resource="&robo;Robot"/>
        <kern:openCycURI rdf:datatype="&xsd;anyURI">http://sw.opencyc.org/concept/Mx4rwQr1pJwpEbGdrcN5Y29ycA</kern:openCycURI>
        <rdfs:comment xml:lang="en">An autonomous robot computes its course of actions with a certain level of autonomy meaning there are decisions that the robot can implement for itself and not totally monitored by other agents.</rdfs:comment>
        <kern:author xml:lang="en">creation Bruno Patin / Jean-Loup Farges - 13/07/2014</kern:author>
    </owl:Class>
    


    <!-- http://europe.bourges.univ-orleans.fr/sites/default/files/download/Ontology/Core/robot.owl#Car-likeRobot -->

    <owl:Class rdf:about="&robo;Car-likeRobot">
        <rdfs:subClassOf rdf:resource="&robo;GroundRobot"/>
        <rdfs:subClassOf>
            <owl:Restriction>
                <owl:onProperty rdf:resource="&kern;has"/>
                <owl:onClass rdf:resource="&syst;Chassis"/>
                <owl:minQualifiedCardinality rdf:datatype="&xsd;nonNegativeInteger">1</owl:minQualifiedCardinality>
            </owl:Restriction>
        </rdfs:subClassOf>
        <rdfs:subClassOf>
            <owl:Restriction>
                <owl:onProperty rdf:resource="&kern;aggregates"/>
                <owl:onClass rdf:resource="&syst;SteeredWheelSystem"/>
                <owl:minQualifiedCardinality rdf:datatype="&xsd;nonNegativeInteger">1</owl:minQualifiedCardinality>
            </owl:Restriction>
        </rdfs:subClassOf>
        <rdfs:subClassOf>
            <owl:Restriction>
                <owl:onProperty rdf:resource="&kern;aggregates"/>
                <owl:onClass rdf:resource="&syst;EngineSystem"/>
                <owl:minQualifiedCardinality rdf:datatype="&xsd;nonNegativeInteger">1</owl:minQualifiedCardinality>
            </owl:Restriction>
        </rdfs:subClassOf>
        <owl:disjointWith rdf:resource="&robo;DifferentialRobot"/>
        <rdfs:comment xml:lang="en">Wheeled robot with a driven mechanism based in axes of wheels (Front-wheel Driven, Rear-wheel Driven or Four-wheel Driven). Normally composed of 4 wheels. It requires an additional steering motion mechanism to turn the vehicle.</rdfs:comment>
    </owl:Class>
    


    <!-- http://europe.bourges.univ-orleans.fr/sites/default/files/download/Ontology/Core/robot.owl#DifferentialRobot -->

    <owl:Class rdf:about="&robo;DifferentialRobot">
        <rdfs:subClassOf rdf:resource="&robo;GroundRobot"/>
        <rdfs:subClassOf>
            <owl:Restriction>
                <owl:onProperty rdf:resource="&kern;aggregates"/>
                <owl:onClass rdf:resource="&syst;EngineSystem"/>
                <owl:minQualifiedCardinality rdf:datatype="&xsd;nonNegativeInteger">2</owl:minQualifiedCardinality>
            </owl:Restriction>
        </rdfs:subClassOf>
        <rdfs:subClassOf>
            <owl:Restriction>
                <owl:onProperty rdf:resource="&kern;has"/>
                <owl:onClass rdf:resource="&syst;Chassis"/>
                <owl:minQualifiedCardinality rdf:datatype="&xsd;nonNegativeInteger">1</owl:minQualifiedCardinality>
            </owl:Restriction>
        </rdfs:subClassOf>
        <rdfs:comment xml:lang="en">A differential vehicle is a mobile robot whose movement is based on two separately driven velocities of the rotational mechanism of both sides of the robot body. It can thus change its direction by varying the relative rate of rotation and hence does not require an additional steering motion. We can find wheeled differential vehicles or caterpillar vehicles.</rdfs:comment>
    </owl:Class>
    


    <!-- http://europe.bourges.univ-orleans.fr/sites/default/files/download/Ontology/Core/robot.owl#GlobalPlatform -->

    <owl:Class rdf:about="&robo;GlobalPlatform">
        <rdfs:subClassOf rdf:resource="&kern;CompositeSystem"/>
        <rdfs:subClassOf>
            <owl:Class>
                <owl:intersectionOf rdf:parseType="Collection">
                    <owl:Restriction>
                        <owl:onProperty rdf:resource="&kern;aggregates"/>
                        <owl:someValuesFrom rdf:resource="&kern;Human"/>
                    </owl:Restriction>
                    <owl:Restriction>
                        <owl:onProperty rdf:resource="&kern;aggregates"/>
                        <owl:someValuesFrom rdf:resource="&robo;Robot"/>
                    </owl:Restriction>
                    <owl:Restriction>
                        <owl:onProperty rdf:resource="&kern;aggregates"/>
                        <owl:someValuesFrom rdf:resource="&syst;ControlStationSystem"/>
                    </owl:Restriction>
                </owl:intersectionOf>
            </owl:Class>
        </rdfs:subClassOf>
        <owl:disjointWith rdf:resource="&robo;Robot"/>
        <owl:disjointWith rdf:resource="&syst;DriverDeviceSystem"/>
        <rdfs:comment xml:lang="en">This composite system groups at least three other ones:
- one robot
- one control station
- one human agent

Its definition is:
System of systems is a collection of task-oriented or dedicated systems that pool their resources and capabilities together to obtain a new, more complex, &apos;meta-system&apos; which offers more functionality and performance than simply the sum of the constituent systems. Currently, systems of systems is a critical research discipline for which frames of reference, thought processes, quantitative analysis, tools, and design methods are incomplete. The methodology for defining, abstracting, modelling, and analysing system of systems problems is typically referred to as system of systems engineering. 
A “robotic system of systems” is a specialised system of systems where there is at least one “robot”, one “control station” and one “human agent”.</rdfs:comment>
    </owl:Class>
    


    <!-- http://europe.bourges.univ-orleans.fr/sites/default/files/download/Ontology/Core/robot.owl#GroundRobot -->

    <owl:Class rdf:about="&robo;GroundRobot">
        <rdfs:subClassOf rdf:resource="&robo;MobileRobot"/>
        <rdfs:subClassOf>
            <owl:Restriction>
                <owl:onProperty rdf:resource="&robo;movesOver"/>
                <owl:someValuesFrom rdf:resource="&envi;Surface"/>
            </owl:Restriction>
        </rdfs:subClassOf>
        <owl:disjointWith rdf:resource="&robo;HybridRobot"/>
        <owl:disjointWith rdf:resource="&robo;SurfaceRobot"/>
        <owl:disjointWith rdf:resource="&robo;UnderwaterRobot"/>
        <rdfs:comment xml:lang="en">Ground Vehicle. Only the wheeled and caterpillar robotic vehicles will be considered.</rdfs:comment>
    </owl:Class>
    


    <!-- http://europe.bourges.univ-orleans.fr/sites/default/files/download/Ontology/Core/robot.owl#HybridRobot -->

    <owl:Class rdf:about="&robo;HybridRobot">
        <rdfs:subClassOf rdf:resource="&robo;MobileRobot"/>
        <owl:disjointWith rdf:resource="&robo;SurfaceRobot"/>
        <owl:disjointWith rdf:resource="&robo;UnderwaterRobot"/>
        <rdfs:comment xml:lang="en">Type of vehicle which can move in different environments. Like the Amphibious vehicles.</rdfs:comment>
    </owl:Class>
    


    <!-- http://europe.bourges.univ-orleans.fr/sites/default/files/download/Ontology/Core/robot.owl#LeggedRobot -->

    <owl:Class rdf:about="&robo;LeggedRobot">
        <rdfs:subClassOf rdf:resource="&robo;GroundRobot"/>
        <rdfs:subClassOf>
            <owl:Restriction>
                <owl:onProperty rdf:resource="&kern;has"/>
                <owl:onClass rdf:resource="&syst;Chassis"/>
                <owl:minQualifiedCardinality rdf:datatype="&xsd;nonNegativeInteger">1</owl:minQualifiedCardinality>
            </owl:Restriction>
        </rdfs:subClassOf>
        <rdfs:subClassOf>
            <owl:Restriction>
                <owl:onProperty rdf:resource="&kern;has"/>
                <owl:onClass rdf:resource="&syst;LegSystem"/>
                <owl:minQualifiedCardinality rdf:datatype="&xsd;nonNegativeInteger">1</owl:minQualifiedCardinality>
            </owl:Restriction>
        </rdfs:subClassOf>
        <rdfs:comment xml:lang="en">For these robots locomotion is assured thanks to articulated bodies (legs for human).</rdfs:comment>
    </owl:Class>
    


    <!-- http://europe.bourges.univ-orleans.fr/sites/default/files/download/Ontology/Core/robot.owl#ManipulatorRobot -->

    <owl:Class rdf:about="&robo;ManipulatorRobot">
        <rdfs:subClassOf rdf:resource="&robo;Robot"/>
        <rdfs:comment xml:lang="en">This is a robot that have at least one grasping system.</rdfs:comment>
    </owl:Class>
    


    <!-- http://europe.bourges.univ-orleans.fr/sites/default/files/download/Ontology/Core/robot.owl#MobileRobot -->

    <owl:Class rdf:about="&robo;MobileRobot">
        <rdfs:subClassOf rdf:resource="&robo;Robot"/>
    </owl:Class>
    


    <!-- http://europe.bourges.univ-orleans.fr/sites/default/files/download/Ontology/Core/robot.owl#PilotedSystem -->

    <owl:Class rdf:about="&robo;PilotedSystem">
        <rdfs:subClassOf rdf:resource="&robo;Robot"/>
        <owl:disjointWith rdf:resource="&robo;UnmannedSystem"/>
        <rdfs:comment xml:lang="en">To represent the piloted robots category and specificities. A car, A piloted aircraft are robots.</rdfs:comment>
    </owl:Class>
    


    <!-- http://europe.bourges.univ-orleans.fr/sites/default/files/download/Ontology/Core/robot.owl#Robot -->

    <owl:Class rdf:about="&robo;Robot">
        <rdfs:subClassOf rdf:resource="&kern;CompositeSystem"/>
        <rdfs:subClassOf>
            <owl:Restriction>
                <owl:onProperty rdf:resource="&kern;aggregates"/>
                <owl:allValuesFrom rdf:resource="&syst;CyberPhysicalSystem"/>
            </owl:Restriction>
        </rdfs:subClassOf>
        <rdfs:subClassOf>
            <owl:Restriction>
                <owl:onProperty rdf:resource="&kern;hasProbe"/>
                <owl:minCardinality rdf:datatype="&xsd;nonNegativeInteger">1</owl:minCardinality>
            </owl:Restriction>
        </rdfs:subClassOf>
        <rdfs:subClassOf>
            <owl:Restriction>
                <owl:onProperty rdf:resource="&kern;hasProbe"/>
                <owl:allValuesFrom rdf:resource="&syst;SensorSystem"/>
            </owl:Restriction>
        </rdfs:subClassOf>
        <owl:disjointWith rdf:resource="&syst;DriverDeviceSystem"/>
        <rdfs:comment xml:lang="en">A robot is a physical object that is designed by a human agent in order to provide a service by acting on the physical world that are eventually monitored by another agent (be it human or another system).
A robot is a composite system but it aggregates only Cyber Physical systems.
This system is also used as a classifier for the different types of robots.</rdfs:comment>
        <kern:author xml:lang="en">creation PROTEUS consortium - 
modified Bruno Patin - 30/09/2013
- comment has changed due to revision of what is the concept
- alignment done to opencyc
modified Bruno Patin - 13/07/2014
- alignment to opencyc deemed incorrect. In order to take into account pure reactive robots (e.g. exo skeleton) it was necessary to introduce a new concept, autonomous robot.</kern:author>
    </owl:Class>
    


    <!-- http://europe.bourges.univ-orleans.fr/sites/default/files/download/Ontology/Core/robot.owl#SurfaceRobot -->

    <owl:Class rdf:about="&robo;SurfaceRobot">
        <rdfs:subClassOf rdf:resource="&robo;MobileRobot"/>
        <rdfs:subClassOf>
            <owl:Restriction>
                <owl:onProperty rdf:resource="&robo;movesOver"/>
                <owl:someValuesFrom rdf:resource="&envi;WaterSurface"/>
            </owl:Restriction>
        </rdfs:subClassOf>
        <owl:disjointWith rdf:resource="&robo;UnderwaterRobot"/>
        <rdfs:comment xml:lang="en">Water Vehicle that remains in the surface of the water (boats or ships-like vehicles).</rdfs:comment>
    </owl:Class>
    


    <!-- http://europe.bourges.univ-orleans.fr/sites/default/files/download/Ontology/Core/robot.owl#UnderwaterRobot -->

    <owl:Class rdf:about="&robo;UnderwaterRobot">
        <rdfs:subClassOf rdf:resource="&robo;MobileRobot"/>
        <rdfs:subClassOf>
            <owl:Restriction>
                <owl:onProperty rdf:resource="&robo;movesIn"/>
                <owl:someValuesFrom rdf:resource="&envi;Waterbody"/>
            </owl:Restriction>
        </rdfs:subClassOf>
        <rdfs:comment xml:lang="en">Vehicles that can move under the water, fish-like or submarine-like vehicles.</rdfs:comment>
    </owl:Class>
    


    <!-- http://europe.bourges.univ-orleans.fr/sites/default/files/download/Ontology/Core/robot.owl#UnmannedSystem -->

    <owl:Class rdf:about="&robo;UnmannedSystem">
        <rdfs:subClassOf rdf:resource="&robo;Robot"/>
        <rdfs:comment xml:lang="en">To represent the unmanned robots category and specificities. Unmanned only means nobody control the robot from inside (no &quot;pilot&quot; onboard).</rdfs:comment>
    </owl:Class>
    


    <!-- http://europe.bourges.univ-orleans.fr/sites/default/files/download/Ontology/Core/system.owl#DriverDeviceSystem -->

    <rdf:Description rdf:about="&syst;DriverDeviceSystem"/>
</rdf:RDF>



<!-- Generated by the OWL API (version 3.4.2) http://owlapi.sourceforge.net -->

