<?xml version="1.0"?>


<!DOCTYPE rdf:RDF [
    <!ENTITY owl "http://www.w3.org/2002/07/owl#" >
    <!ENTITY swrl "http://www.w3.org/2003/11/swrl#" >
    <!ENTITY swrlb "http://www.w3.org/2003/11/swrlb#" >
    <!ENTITY xsd "http://www.w3.org/2001/XMLSchema#" >
    <!ENTITY rdfs "http://www.w3.org/2000/01/rdf-schema#" >
    <!ENTITY rdf "http://www.w3.org/1999/02/22-rdf-syntax-ns#" >
    <!ENTITY protege "http://protege.stanford.edu/plugins/owl/protege#" >
    <!ENTITY xsp "http://www.owl-ontologies.com/2005/08/07/xsp.owl#" >
    <!ENTITY swrla "http://swrl.stanford.edu/ontologies/3.3/swrla.owl#" >
    <!ENTITY sqwrl "http://sqwrl.stanford.edu/ontologies/built-ins/3.4/sqwrl.owl#" >
    <!ENTITY kern "http://europe.bourges.univ-orleans.fr/sites/default/files/download/Ontology/Core/kernel.owl#" >
    <!ENTITY envi "http://europe.bourges.univ-orleans.fr/sites/default/files/download/Ontology/Core/environment.owl#" >
]>


<rdf:RDF xmlns="http://europe.bourges.univ-orleans.fr/sites/default/files/download/Ontology/Core/environment.owl#"
     xml:base="http://europe.bourges.univ-orleans.fr/sites/default/files/download/Ontology/Core/environment.owl"
     xmlns:protege="http://protege.stanford.edu/plugins/owl/protege#"
     xmlns:xsp="http://www.owl-ontologies.com/2005/08/07/xsp.owl#"
     xmlns:kern="http://europe.bourges.univ-orleans.fr/sites/default/files/download/Ontology/Core/kernel.owl#"
     xmlns:sqwrl="http://sqwrl.stanford.edu/ontologies/built-ins/3.4/sqwrl.owl#"
     xmlns:rdfs="http://www.w3.org/2000/01/rdf-schema#"
     xmlns:swrl="http://www.w3.org/2003/11/swrl#"
     xmlns:envi="http://europe.bourges.univ-orleans.fr/sites/default/files/download/Ontology/Core/environment.owl#"
     xmlns:owl="http://www.w3.org/2002/07/owl#"
     xmlns:xsd="http://www.w3.org/2001/XMLSchema#"
     xmlns:swrlb="http://www.w3.org/2003/11/swrlb#"
     xmlns:rdf="http://www.w3.org/1999/02/22-rdf-syntax-ns#"
     xmlns:swrla="http://swrl.stanford.edu/ontologies/3.3/swrla.owl#">
    <owl:Ontology rdf:about="http://europe.bourges.univ-orleans.fr/sites/default/files/download/Ontology/Core/environment.owl">
        <rdfs:comment xml:lang="en">This work is based upon a previous one funded by the French Research agency ANR (Agence Nationale de la Recherche) through thePROTEUS project (see http://www.anr-project.fr). It is the property of its authors and is governed by the CECILL B V1 licence (see http://www.cecill.info for information and the associated Licence_CeCILL-B_V1-en.txt or Licence_CeCILL-B_V1-fr.txt files).</rdfs:comment>
        <owl:imports rdf:resource="http://europe.bourges.univ-orleans.fr/sites/default/files/download/Ontology/Core/information.owl"/>
        <owl:imports rdf:resource="http://europe.bourges.univ-orleans.fr/sites/default/files/download/Ontology/Core/kernel.owl"/>
        <owl:imports rdf:resource="http://sqwrl.stanford.edu/ontologies/built-ins/3.4/sqwrl.owl"/>
    </owl:Ontology>
    


    <!-- 
    ///////////////////////////////////////////////////////////////////////////////////////
    //
    // Object Properties
    //
    ///////////////////////////////////////////////////////////////////////////////////////
     -->

    


    <!-- http://europe.bourges.univ-orleans.fr/sites/default/files/download/Ontology/Core/environment.owl#accelerates -->

    <owl:ObjectProperty rdf:about="&envi;accelerates">
        <rdfs:comment xml:lang="en">force accelerates physical object</rdfs:comment>
        <rdfs:domain rdf:resource="&envi;Force"/>
        <rdfs:range rdf:resource="&kern;PhysicalObject"/>
    </owl:ObjectProperty>
    


    <!-- http://europe.bourges.univ-orleans.fr/sites/default/files/download/Ontology/Core/environment.owl#forbidsMovement -->

    <owl:ObjectProperty rdf:about="&envi;forbidsMovement">
        <rdfs:comment>This relation is linked to the fact that some physical interactions are limited in their impact wrt movement of impacted Physical Object. For instance consdiering joint object they generally forbids movement other inside a specific subgroup of the euclidean displacements group.</rdfs:comment>
        <rdfs:subPropertyOf rdf:resource="&kern;constrainsFrame"/>
    </owl:ObjectProperty>
    


    <!-- http://europe.bourges.univ-orleans.fr/sites/default/files/download/Ontology/Core/environment.owl#hasAtmosphere -->

    <owl:ObjectProperty rdf:about="&envi;hasAtmosphere">
        <rdfs:comment xml:lang="en">Some planets have atmosphere</rdfs:comment>
        <rdfs:range rdf:resource="&envi;Atmosphere"/>
        <rdfs:domain rdf:resource="&envi;Planet"/>
    </owl:ObjectProperty>
    


    <!-- http://europe.bourges.univ-orleans.fr/sites/default/files/download/Ontology/Core/environment.owl#hasBuilding -->

    <owl:ObjectProperty rdf:about="&envi;hasBuilding">
        <rdfs:comment xml:lang="en">Planets such as Earth have buildings.</rdfs:comment>
        <rdfs:range rdf:resource="&envi;Building"/>
        <rdfs:domain rdf:resource="&envi;Planet"/>
    </owl:ObjectProperty>
    


    <!-- http://europe.bourges.univ-orleans.fr/sites/default/files/download/Ontology/Core/environment.owl#hasCurrentInFluid -->

    <owl:ObjectProperty rdf:about="&envi;hasCurrentInFluid">
        <rdfs:comment xml:lang="en">Atmospheres and waterbodies may have distribution of current in them and it is one of their physical characteristics</rdfs:comment>
        <rdfs:domain rdf:resource="&envi;FluidObject"/>
        <rdfs:range rdf:resource="http://europe.bourges.univ-orleans.fr/sites/default/files/download/Ontology/Core/information.owl#Tensor"/>
    </owl:ObjectProperty>
    


    <!-- http://europe.bourges.univ-orleans.fr/sites/default/files/download/Ontology/Core/environment.owl#hasFloor -->

    <owl:ObjectProperty rdf:about="&envi;hasFloor">
        <rdfs:comment xml:lang="en">buildings have floors</rdfs:comment>
        <rdfs:domain rdf:resource="&envi;Building"/>
        <rdfs:range rdf:resource="&envi;Floor"/>
    </owl:ObjectProperty>
    


    <!-- http://europe.bourges.univ-orleans.fr/sites/default/files/download/Ontology/Core/environment.owl#hasLandSurface -->

    <owl:ObjectProperty rdf:about="&envi;hasLandSurface">
        <rdfs:comment xml:lang="en">A planet has a land surface whose vertical and horizontal dimensions characteirse the terrain.</rdfs:comment>
        <rdfs:range rdf:resource="&envi;LandSurface"/>
        <rdfs:domain rdf:resource="&envi;Planet"/>
        <rdfs:subPropertyOf rdf:resource="&envi;hasSurface"/>
    </owl:ObjectProperty>
    


    <!-- http://europe.bourges.univ-orleans.fr/sites/default/files/download/Ontology/Core/environment.owl#hasStairs -->

    <owl:ObjectProperty rdf:about="&envi;hasStairs">
        <rdfs:comment xml:lang="en">Stairs are usually in buildings, but some stairs are outdoor.</rdfs:comment>
        <rdfs:range rdf:resource="&envi;Stairs"/>
        <rdfs:domain>
            <owl:Class>
                <owl:unionOf rdf:parseType="Collection">
                    <rdf:Description rdf:about="&envi;Building"/>
                    <rdf:Description rdf:about="&envi;Planet"/>
                </owl:unionOf>
            </owl:Class>
        </rdfs:domain>
    </owl:ObjectProperty>
    


    <!-- http://europe.bourges.univ-orleans.fr/sites/default/files/download/Ontology/Core/environment.owl#hasSurface -->

    <owl:ObjectProperty rdf:about="&envi;hasSurface">
        <rdfs:comment xml:lang="en">Physical objects have surfaces that determine their boudaries.</rdfs:comment>
        <rdfs:range rdf:resource="&envi;Surface"/>
        <owl:inverseOf rdf:resource="&envi;isSurfaceOf"/>
        <rdfs:domain rdf:resource="&kern;PhysicalObject"/>
    </owl:ObjectProperty>
    


    <!-- http://europe.bourges.univ-orleans.fr/sites/default/files/download/Ontology/Core/environment.owl#hasWaterbody -->

    <owl:ObjectProperty rdf:about="&envi;hasWaterbody">
        <rdfs:comment xml:lang="en">Planets have waterbodies such as oceans, seas...</rdfs:comment>
        <rdfs:domain rdf:resource="&envi;Planet"/>
        <rdfs:range rdf:resource="&envi;Waterbody"/>
    </owl:ObjectProperty>
    


    <!-- http://europe.bourges.univ-orleans.fr/sites/default/files/download/Ontology/Core/environment.owl#isAssociatedToPO -->

    <owl:ObjectProperty rdf:about="&envi;isAssociatedToPO">
        <rdfs:domain rdf:resource="&kern;Frame"/>
        <rdfs:range rdf:resource="&kern;PhysicalObject"/>
    </owl:ObjectProperty>
    


    <!-- http://europe.bourges.univ-orleans.fr/sites/default/files/download/Ontology/Core/environment.owl#isLocatedOver -->

    <owl:ObjectProperty rdf:about="&envi;isLocatedOver">
        <rdfs:comment xml:lang="en">Buildings are located over land surface.</rdfs:comment>
        <rdfs:domain rdf:resource="&envi;Building"/>
        <rdfs:range rdf:resource="&envi;LandSurface"/>
    </owl:ObjectProperty>
    


    <!-- http://europe.bourges.univ-orleans.fr/sites/default/files/download/Ontology/Core/environment.owl#isSurfaceOf -->

    <owl:ObjectProperty rdf:about="&envi;isSurfaceOf">
        <rdfs:comment xml:lang="en">Surfaces are the borders of physical objects.</rdfs:comment>
        <rdfs:domain rdf:resource="&envi;Surface"/>
        <rdfs:range rdf:resource="&kern;PhysicalObject"/>
    </owl:ObjectProperty>
    


    <!-- http://europe.bourges.univ-orleans.fr/sites/default/files/download/Ontology/Core/environment.owl#produceGravityForce -->

    <owl:ObjectProperty rdf:about="&envi;produceGravityForce">
        <rdfs:comment xml:lang="en">this property specifies that a planet is able to locally create for any phyical object on or above its surface a gravity force.</rdfs:comment>
        <rdfs:range rdf:resource="&envi;GravityForce"/>
        <rdfs:domain rdf:resource="&envi;Planet"/>
    </owl:ObjectProperty>
    


    <!-- http://europe.bourges.univ-orleans.fr/sites/default/files/download/Ontology/Core/kernel.owl#definesAFrame -->

    <rdf:Description rdf:about="&kern;definesAFrame">
        <rdf:type rdf:resource="&owl;FunctionalProperty"/>
        <owl:inverseOf rdf:resource="&envi;isAssociatedToPO"/>
    </rdf:Description>
    


    <!-- http://europe.bourges.univ-orleans.fr/sites/default/files/download/Ontology/Core/kernel.owl#hasFSMActivity -->

    <owl:ObjectProperty rdf:about="&kern;hasFSMActivity">
        <rdfs:comment xml:lang="en">A state can be associated to Finite State Machine Activities.</rdfs:comment>
        <rdfs:domain rdf:resource="&kern;AutomataState"/>
        <rdfs:range rdf:resource="&kern;FSMActivity"/>
        <rdfs:subPropertyOf rdf:resource="&kern;has"/>
    </owl:ObjectProperty>
    


    <!-- http://europe.bourges.univ-orleans.fr/sites/default/files/download/Ontology/Core/kernel.owl#isImplementedWith -->

    <owl:ObjectProperty rdf:about="&kern;isImplementedWith">
        <rdfs:comment xml:lang="en">An FSMActivity is implemented by an algorithm</rdfs:comment>
        <rdfs:range rdf:resource="&kern;Algorithm"/>
        <rdfs:domain rdf:resource="&kern;FSMActivity"/>
    </owl:ObjectProperty>
    


    <!-- 
    ///////////////////////////////////////////////////////////////////////////////////////
    //
    // Classes
    //
    ///////////////////////////////////////////////////////////////////////////////////////
     -->

    


    <!-- http://europe.bourges.univ-orleans.fr/sites/default/files/download/Ontology/Core/environment.owl#AerodynamicForce -->

    <owl:Class rdf:about="&envi;AerodynamicForce">
        <rdfs:subClassOf rdf:resource="&envi;Force"/>
        <rdfs:subClassOf>
            <owl:Restriction>
                <owl:onProperty rdf:resource="&kern;systemSource"/>
                <owl:allValuesFrom rdf:resource="&envi;Atmosphere"/>
            </owl:Restriction>
        </rdfs:subClassOf>
        <owl:disjointWith rdf:resource="&envi;Buoyancy"/>
        <owl:disjointWith rdf:resource="&envi;GravityForce"/>
        <owl:disjointWith rdf:resource="&envi;NormalForce"/>
        <rdfs:comment xml:lang="en">Aerodynamic force is the resultant force exerted on a body by the air (or some other gas) in which the body is immersed, and is due to the relative motion between the body and the fluid.</rdfs:comment>
    </owl:Class>
    


    <!-- http://europe.bourges.univ-orleans.fr/sites/default/files/download/Ontology/Core/environment.owl#AstronomicalObject -->

    <owl:Class rdf:about="&envi;AstronomicalObject">
        <rdfs:subClassOf rdf:resource="&kern;PhysicalObject"/>
        <owl:disjointWith rdf:resource="&kern;Agent"/>
        <owl:disjointWith rdf:resource="&kern;Environment"/>
        <owl:disjointWith rdf:resource="&kern;Hardware"/>
        <kern:author xml:lang="en">creation Bruno Patin - 04/10/2013
- individuals creation process (solar system) leads to create such a class</kern:author>
        <kern:openCycURI xml:lang="en">http://sw.opencyc.org/concept/Mx4rvVjReJwpEbGdrcN5Y29ycA</kern:openCycURI>
    </owl:Class>
    


    <!-- http://europe.bourges.univ-orleans.fr/sites/default/files/download/Ontology/Core/environment.owl#Atmosphere -->

    <owl:Class rdf:about="&envi;Atmosphere">
        <rdfs:subClassOf rdf:resource="&envi;FluidObject"/>
        <owl:disjointWith rdf:resource="&envi;Waterbody"/>
        <rdfs:comment xml:lang="en">a layer of gases that may surround a planet ]and that is held in place by the gravity of the planet. It is of interest if there are influences exercising on included physical objects.</rdfs:comment>
    </owl:Class>
    


    <!-- http://europe.bourges.univ-orleans.fr/sites/default/files/download/Ontology/Core/environment.owl#AtomicSurface -->

    <owl:Class rdf:about="&envi;AtomicSurface">
        <rdfs:subClassOf rdf:resource="&envi;Surface"/>
        <rdfs:subClassOf rdf:resource="&kern;AtomicSystem"/>
        <rdfs:comment xml:lang="en">An atomic surface is a surface where properties applie to every point of this surface.</rdfs:comment>
    </owl:Class>
    


    <!-- http://europe.bourges.univ-orleans.fr/sites/default/files/download/Ontology/Core/environment.owl#Building -->

    <owl:Class rdf:about="&envi;Building">
        <rdfs:subClassOf rdf:resource="&envi;SolidObject"/>
        <owl:disjointWith rdf:resource="&envi;Planet"/>
        <owl:disjointWith rdf:resource="&envi;Surface"/>
        <owl:disjointWith rdf:resource="&kern;Agent"/>
        <owl:disjointWith rdf:resource="&kern;Hardware"/>
        <rdfs:comment xml:lang="en">human-made structure used or intended for supporting or sheltering any use or continuous occupancy</rdfs:comment>
    </owl:Class>
    


    <!-- http://europe.bourges.univ-orleans.fr/sites/default/files/download/Ontology/Core/environment.owl#Buoyancy -->

    <owl:Class rdf:about="&envi;Buoyancy">
        <rdfs:subClassOf rdf:resource="&envi;Force"/>
        <owl:disjointWith rdf:resource="&envi;GravityForce"/>
        <owl:disjointWith rdf:resource="&envi;NormalForce"/>
        <rdfs:comment xml:lang="en">Buoyancy is an upward acting force exerted by a fluid, that opposes an object&apos;s weight. This force is relevant for physical objects in waterbodies or at watersurface.</rdfs:comment>
    </owl:Class>
    


    <!-- http://europe.bourges.univ-orleans.fr/sites/default/files/download/Ontology/Core/environment.owl#Floor -->

    <owl:Class rdf:about="&envi;Floor">
        <rdfs:subClassOf rdf:resource="&envi;Surface"/>
        <owl:disjointWith rdf:resource="&envi;LandSurface"/>
        <owl:disjointWith rdf:resource="&envi;Stairs"/>
        <owl:disjointWith rdf:resource="&envi;WaterSurface"/>
        <rdfs:comment xml:lang="en">Walking surface of a room in a building.</rdfs:comment>
    </owl:Class>
    


    <!-- http://europe.bourges.univ-orleans.fr/sites/default/files/download/Ontology/Core/environment.owl#FluidObject -->

    <owl:Class rdf:about="&envi;FluidObject">
        <rdfs:subClassOf rdf:resource="&kern;PhysicalObject"/>
        <owl:disjointWith rdf:resource="&envi;SolidObject"/>
        <owl:disjointWith rdf:resource="&envi;Surface"/>
        <owl:disjointWith rdf:resource="&kern;Environment"/>
        <rdfs:isDefinedBy rdf:datatype="&xsd;anyURI">http://sw.opencyc.org/concept/Mx4rvVjR45wpEbGdrcN5Y29ycA</rdfs:isDefinedBy>
        <rdfs:seeAlso rdf:datatype="&xsd;string">openCyc: FluidTangibleThing</rdfs:seeAlso>
        <rdfs:comment xml:lang="en">Fluid objects are physical objects that are able to deform and to flow</rdfs:comment>
    </owl:Class>
    


    <!-- http://europe.bourges.univ-orleans.fr/sites/default/files/download/Ontology/Core/environment.owl#Force -->

    <owl:Class rdf:about="&envi;Force">
        <rdfs:subClassOf rdf:resource="&kern;PhysicalInteraction"/>
        <rdfs:subClassOf>
            <owl:Restriction>
                <owl:onProperty rdf:resource="&kern;impacts"/>
                <owl:allValuesFrom rdf:resource="&kern;PhysicalObject"/>
            </owl:Restriction>
        </rdfs:subClassOf>
        <rdfs:subClassOf>
            <owl:Restriction>
                <owl:onProperty rdf:resource="&kern;systemSource"/>
                <owl:allValuesFrom rdf:resource="&kern;PhysicalObject"/>
            </owl:Restriction>
        </rdfs:subClassOf>
        <owl:disjointWith rdf:resource="&envi;Torque"/>
        <rdfs:comment xml:lang="en">A force is any influence that causes a free body to undergo a change in speed, a change in direction, or a change in shape. It is an interaction as it can be caused either by another body or as a synthesis of the environment influence (the two of them are systems).</rdfs:comment>
    </owl:Class>
    


    <!-- http://europe.bourges.univ-orleans.fr/sites/default/files/download/Ontology/Core/environment.owl#GravityForce -->

    <owl:Class rdf:about="&envi;GravityForce">
        <rdfs:subClassOf rdf:resource="&envi;Force"/>
        <owl:disjointWith rdf:resource="&envi;NormalForce"/>
        <rdfs:comment xml:lang="en">A force that is directly proportional to the PhysicalObject mass.</rdfs:comment>
    </owl:Class>
    


    <!-- http://europe.bourges.univ-orleans.fr/sites/default/files/download/Ontology/Core/environment.owl#LandSurface -->

    <owl:Class rdf:about="&envi;LandSurface">
        <rdfs:subClassOf rdf:resource="&envi;Surface"/>
        <rdfs:subClassOf>
            <owl:Restriction>
                <owl:onProperty rdf:resource="&envi;isSurfaceOf"/>
                <owl:someValuesFrom>
                    <owl:Class>
                        <owl:intersectionOf rdf:parseType="Collection">
                            <rdf:Description rdf:about="&envi;Planet"/>
                            <rdf:Description rdf:about="&envi;SolidObject"/>
                        </owl:intersectionOf>
                    </owl:Class>
                </owl:someValuesFrom>
            </owl:Restriction>
        </rdfs:subClassOf>
        <owl:disjointWith rdf:resource="&envi;Stairs"/>
        <owl:disjointWith rdf:resource="&envi;WaterSurface"/>
        <rdfs:comment xml:lang="en">The solid surface of a planet.</rdfs:comment>
    </owl:Class>
    


    <!-- http://europe.bourges.univ-orleans.fr/sites/default/files/download/Ontology/Core/environment.owl#MachineTorque -->

    <owl:Class rdf:about="&envi;MachineTorque">
        <rdfs:subClassOf rdf:resource="&envi;Torque"/>
        <kern:openCycURI rdf:datatype="&xsd;anyURI">http://sw.opencyc.org/concept/Mx4rvVkFSJwpEbGdrcN5Y29ycA</kern:openCycURI>
        <kern:author xml:lang="en">creation Jean-Loup Farges - 10/09/2013
modified Bruno Patin - 15/09/2013
- authorship added
- comment added
- TODO added</kern:author>
        <kern:wikipediaURI>http://en.wikipedia.org/wiki/Torque#Machine_torque</kern:wikipediaURI>
    </owl:Class>
    


    <!-- http://europe.bourges.univ-orleans.fr/sites/default/files/download/Ontology/Core/environment.owl#NEDFrame -->

    <owl:Class rdf:about="&envi;NEDFrame">
        <rdfs:subClassOf rdf:resource="&kern;Frame"/>
        <kern:wikipediaURI rdf:datatype="&xsd;anyURI">http://en.wikipedia.org/wiki/North_east_down</kern:wikipediaURI>
        <rdfs:comment rdf:datatype="&xsd;anyURI">the north east down frame is a local coordinate system linked to global planet frame.</rdfs:comment>
    </owl:Class>
    


    <!-- http://europe.bourges.univ-orleans.fr/sites/default/files/download/Ontology/Core/environment.owl#NormalForce -->

    <owl:Class rdf:about="&envi;NormalForce">
        <rdfs:subClassOf rdf:resource="&envi;Force"/>
        <rdfs:comment xml:lang="en">The normal force is the repulsive force of interaction between atoms at close contact. This force is applicalble in hard surface contact of physical objects.</rdfs:comment>
    </owl:Class>
    


    <!-- http://europe.bourges.univ-orleans.fr/sites/default/files/download/Ontology/Core/environment.owl#Pedestrian -->

    <owl:Class rdf:about="&envi;Pedestrian">
        <rdfs:subClassOf rdf:resource="&kern;Human"/>
        <rdfs:comment xml:lang="en">Physical Agent in a scenario which perfoms the action of going on foot, i.e. walking.</rdfs:comment>
    </owl:Class>
    


    <!-- http://europe.bourges.univ-orleans.fr/sites/default/files/download/Ontology/Core/environment.owl#Planet -->

    <owl:Class rdf:about="&envi;Planet">
        <rdfs:subClassOf rdf:resource="&envi;AstronomicalObject"/>
        <owl:disjointWith rdf:resource="&envi;Surface"/>
        <owl:disjointWith rdf:resource="&kern;Agent"/>
        <owl:disjointWith rdf:resource="&kern;Hardware"/>
        <rdfs:comment xml:lang="en">a celestial body  that is massive enough to be rounded by its own gravity but not massive enough to initiate fusion process.</rdfs:comment>
        <kern:author xml:lang="en">creation PROTEUS consortium - 
modified Bruno Patin - 04/10/2013
- alignment to opencyc and move to new introduced class</kern:author>
    </owl:Class>
    


    <!-- http://europe.bourges.univ-orleans.fr/sites/default/files/download/Ontology/Core/environment.owl#SolidObject -->

    <owl:Class rdf:about="&envi;SolidObject">
        <rdfs:subClassOf rdf:resource="&kern;PhysicalObject"/>
        <owl:disjointWith rdf:resource="&envi;Surface"/>
        <owl:disjointWith rdf:resource="&kern;Environment"/>
        <rdfs:isDefinedBy rdf:datatype="&xsd;anyURI">http://sw.opencyc.org/concept/Mx4rvVjElJwpEbGdrcN5Y29ycA</rdfs:isDefinedBy>
        <rdfs:seeAlso rdf:datatype="&xsd;string">openCyc: SolidTangibleThing</rdfs:seeAlso>
    </owl:Class>
    


    <!-- http://europe.bourges.univ-orleans.fr/sites/default/files/download/Ontology/Core/environment.owl#Stairs -->

    <owl:Class rdf:about="&envi;Stairs">
        <rdfs:subClassOf rdf:resource="&envi;Surface"/>
        <owl:disjointWith rdf:resource="&envi;WaterSurface"/>
        <rdfs:comment xml:lang="en">a construction designed to bridge a large vertical distance by dividing it into smaller vertical distances, called steps.</rdfs:comment>
    </owl:Class>
    


    <!-- http://europe.bourges.univ-orleans.fr/sites/default/files/download/Ontology/Core/environment.owl#Star -->

    <owl:Class rdf:about="&envi;Star">
        <rdfs:subClassOf rdf:resource="&envi;AstronomicalObject"/>
        <rdfs:comment xml:lang="en">a celestial body  that is massive enough to be rounded by its own gravity and massive enough to initiate fusion process.</rdfs:comment>
        <kern:author xml:lang="en">creation PROTEUS consortium - 
modified Bruno Patin - 04/10/2013
- alignment to opencyc and move to new introduced class</kern:author>
        <kern:openCycURI xml:lang="en">http://sw.opencyc.org/concept/Mx4rvVi80ZwpEbGdrcN5Y29ycA</kern:openCycURI>
    </owl:Class>
    


    <!-- http://europe.bourges.univ-orleans.fr/sites/default/files/download/Ontology/Core/environment.owl#Surface -->

    <owl:Class rdf:about="&envi;Surface">
        <rdfs:subClassOf rdf:resource="&kern;PhysicalObject"/>
        <rdfs:subClassOf>
            <owl:Restriction>
                <owl:onProperty rdf:resource="&envi;hasSurface"/>
                <owl:onClass rdf:resource="&envi;Surface"/>
                <owl:qualifiedCardinality rdf:datatype="&xsd;nonNegativeInteger">0</owl:qualifiedCardinality>
            </owl:Restriction>
        </rdfs:subClassOf>
        <owl:disjointWith rdf:resource="&kern;Agent"/>
        <owl:disjointWith rdf:resource="&kern;Environment"/>
        <owl:disjointWith rdf:resource="&kern;Hardware"/>
        <rdfs:comment xml:lang="en">A two-dimensional topological manifold that is a boundary of a physical object</rdfs:comment>
    </owl:Class>
    


    <!-- http://europe.bourges.univ-orleans.fr/sites/default/files/download/Ontology/Core/environment.owl#Torque -->

    <owl:Class rdf:about="&envi;Torque">
        <rdfs:subClassOf rdf:resource="&kern;PhysicalInteraction"/>
        <rdfs:comment>Following wikipedia, torque, moment or moment of force, is the tendency of a force to rotate an object about an axis, fulcrum, or pivot.</rdfs:comment>
        <kern:author xml:lang="en">creation Jean-Loup Farges - 10/09/2013
modified Bruno Patin - 15/09/2013
- authorship added</kern:author>
        <kern:wikipediaURI>http://en.wikipedia.org/wiki/Torque</kern:wikipediaURI>
    </owl:Class>
    


    <!-- http://europe.bourges.univ-orleans.fr/sites/default/files/download/Ontology/Core/environment.owl#WaterSurface -->

    <owl:Class rdf:about="&envi;WaterSurface">
        <rdfs:subClassOf rdf:resource="&envi;Surface"/>
        <rdfs:subClassOf>
            <owl:Restriction>
                <owl:onProperty rdf:resource="&envi;isSurfaceOf"/>
                <owl:someValuesFrom rdf:resource="&envi;Waterbody"/>
            </owl:Restriction>
        </rdfs:subClassOf>
        <rdfs:comment xml:lang="en">Surface of an ocean, a sea, a lake or an artificial reservatory.</rdfs:comment>
    </owl:Class>
    


    <!-- http://europe.bourges.univ-orleans.fr/sites/default/files/download/Ontology/Core/environment.owl#Waterbody -->

    <owl:Class rdf:about="&envi;Waterbody">
        <rdfs:subClassOf rdf:resource="&envi;FluidObject"/>
        <rdfs:comment xml:lang="en">Significant accumulation of water. It is of interest if there are influences exercising on included physical objects.
This concept IS NOT the &quot;Waterbody concept&quot; as defined in openCyc and that groups everything that is related to our waterbody concept.</rdfs:comment>
    </owl:Class>
    


    <!-- http://europe.bourges.univ-orleans.fr/sites/default/files/download/Ontology/Core/kernel.owl#Agent -->

    <rdf:Description rdf:about="&kern;Agent">
        <rdfs:subClassOf rdf:resource="&envi;SolidObject"/>
        <rdfs:comment xml:lang="en">TODO: relationship with openCyc was not possible. TBD perhaps.</rdfs:comment>
    </rdf:Description>
    


    <!-- http://europe.bourges.univ-orleans.fr/sites/default/files/download/Ontology/Core/kernel.owl#Environment -->

    <rdf:Description rdf:about="&kern;Environment">
        <kern:wikipediaURI rdf:datatype="&xsd;anyURI">http://en.wikipedia.org/wiki/Environment_%28systems%29</kern:wikipediaURI>
        <kern:openCycURI rdf:datatype="&xsd;anyURI">http://sw.opencyc.org/concept/Mx4rwLW-jpwpEbGdrcN5Y29ycA</kern:openCycURI>
        <kern:author xml:lang="en">creation PROTEUS consortium - 
modified Bruno Patin - 15/09/2013
- OpenCyc and Wikipedia reference added
- comment explaining difference between the two concepts.</kern:author>
    </rdf:Description>
    


    <!-- http://europe.bourges.univ-orleans.fr/sites/default/files/download/Ontology/Core/kernel.owl#FSMActivity -->

    <owl:Class rdf:about="&kern;FSMActivity">
        <rdfs:subClassOf rdf:resource="&kern;Activity"/>
        <rdfs:comment xml:lang="en">A Finite State Machine Activity is an Activity linked to an AutomateState which is implemented by means of Algorithms.</rdfs:comment>
    </owl:Class>
    


    <!-- http://europe.bourges.univ-orleans.fr/sites/default/files/download/Ontology/Core/kernel.owl#Hardware -->

    <rdf:Description rdf:about="&kern;Hardware">
        <rdfs:subClassOf rdf:resource="&envi;SolidObject"/>
    </rdf:Description>
    


    <!-- 
    ///////////////////////////////////////////////////////////////////////////////////////
    //
    // Individuals
    //
    ///////////////////////////////////////////////////////////////////////////////////////
     -->

    


    <!-- http://europe.bourges.univ-orleans.fr/sites/default/files/download/Ontology/Core/kernel.owl#Earth -->

    <rdf:Description rdf:about="&kern;Earth">
        <rdf:type rdf:resource="&envi;Planet"/>
    </rdf:Description>
    


    <!-- http://europe.bourges.univ-orleans.fr/sites/default/files/download/Ontology/Core/kernel.owl#Moon -->

    <rdf:Description rdf:about="&kern;Moon">
        <rdf:type rdf:resource="&envi;Planet"/>
    </rdf:Description>
    


    <!-- http://europe.bourges.univ-orleans.fr/sites/default/files/download/Ontology/Core/kernel.owl#Sun -->

    <rdf:Description rdf:about="&kern;Sun">
        <rdf:type rdf:resource="&envi;Star"/>
    </rdf:Description>
</rdf:RDF>



<!-- Generated by the OWL API (version 3.4.2) http://owlapi.sourceforge.net -->

