<?xml version="1.0"?>


<!DOCTYPE rdf:RDF [
    <!ENTITY owl "http://www.w3.org/2002/07/owl#" >
    <!ENTITY swrl "http://www.w3.org/2003/11/swrl#" >
    <!ENTITY swrlb "http://www.w3.org/2003/11/swrlb#" >
    <!ENTITY xsd "http://www.w3.org/2001/XMLSchema#" >
    <!ENTITY owl2xml "http://www.w3.org/2006/12/owl2-xml#" >
    <!ENTITY rdfs "http://www.w3.org/2000/01/rdf-schema#" >
    <!ENTITY rdf "http://www.w3.org/1999/02/22-rdf-syntax-ns#" >
    <!ENTITY protege "http://protege.stanford.edu/plugins/owl/protege#" >
    <!ENTITY xsp "http://www.owl-ontologies.com/2005/08/07/xsp.owl#" >
    <!ENTITY swrla "http://swrl.stanford.edu/ontologies/3.3/swrla.owl#" >
    <!ENTITY sqwrl "http://sqwrl.stanford.edu/ontologies/built-ins/3.4/sqwrl.owl#" >
    <!ENTITY robo "http://www.anr-proteus.fr/sites/default/files/download/Ontology/robot.owl#" >
    <!ENTITY kern "http://www.anr-proteus.fr/sites/default/files/download/Ontology/kernel.owl#" >
    <!ENTITY miss "http://www.anr-proteus.fr/sites/default/files/download/Ontology/mission.owl#" >
    <!ENTITY simu "http://www.anr-proteus.fr/sites/default/files/download/Ontology/simulation.owl#" >
    <!ENTITY envi "http://www.anr-proteus.fr/sites/default/files/download/Ontology/environment.owl#" >
    <!ENTITY info "http://www.anr-proteus.fr/sites/default/files/download/Ontology/information.owl#" >
]>


<rdf:RDF xmlns="http://www.anr-proteus.fr/sites/default/files/download/Ontology/mission.owl#"
     xml:base="http://www.anr-proteus.fr/sites/default/files/download/Ontology/mission.owl"
     xmlns:protege="http://protege.stanford.edu/plugins/owl/protege#"
     xmlns:xsp="http://www.owl-ontologies.com/2005/08/07/xsp.owl#"
     xmlns:robo="http://www.anr-proteus.fr/sites/default/files/download/Ontology/robot.owl#"
     xmlns:simu="http://www.anr-proteus.fr/sites/default/files/download/Ontology/simulation.owl#"
     xmlns:kern="http://www.anr-proteus.fr/sites/default/files/download/Ontology/kernel.owl#"
     xmlns:info="http://www.anr-proteus.fr/sites/default/files/download/Ontology/information.owl#"
     xmlns:sqwrl="http://sqwrl.stanford.edu/ontologies/built-ins/3.4/sqwrl.owl#"
     xmlns:rdfs="http://www.w3.org/2000/01/rdf-schema#"
     xmlns:swrl="http://www.w3.org/2003/11/swrl#"
     xmlns:owl2xml="http://www.w3.org/2006/12/owl2-xml#"
     xmlns:envi="http://www.anr-proteus.fr/sites/default/files/download/Ontology/environment.owl#"
     xmlns:xsd="http://www.w3.org/2001/XMLSchema#"
     xmlns:owl="http://www.w3.org/2002/07/owl#"
     xmlns:swrlb="http://www.w3.org/2003/11/swrlb#"
     xmlns:rdf="http://www.w3.org/1999/02/22-rdf-syntax-ns#"
     xmlns:miss="http://www.anr-proteus.fr/sites/default/files/download/Ontology/mission.owl#"
     xmlns:swrla="http://swrl.stanford.edu/ontologies/3.3/swrla.owl#">
    <owl:Ontology rdf:about="http://www.anr-proteus.fr/sites/default/files/download/Ontology/mission.owl">
        <owl:versionInfo rdf:datatype="&xsd;string">version delivered 1.0</owl:versionInfo>
        <rdfs:comment xml:lang="en">FaCT++ does not work on this ontology. Reasoning shall be performed using HermiT.</rdfs:comment>
        <rdfs:comment xml:lang="en">This ontology describes the mission as seen by a system. It is mainly a part of the information ontology.It is using as its main paradigm for representing the mission, the Hierarchical Tasks Network as can be seen described in Julien Guitton Thesis - &quot;Architecture Hybride pour la planification d&apos;actions et de déplacements&quot; - ISAE 2010.</rdfs:comment>
        <rdfs:comment xml:lang="en">This work is based upon a previous one funded by the French Research agency ANR (Agence Nationale de la Recherche) through thePROTEUS project (see http://www.anr-project.fr). It is the property of its authors and is governed by the CECILL B V1 licence (see http://www.cecill.info for information and the associated Licence_CeCILL-B_V1-en.txt or Licence_CeCILL-B_V1-fr.txt files).</rdfs:comment>
        <rdfs:comment xml:lang="en">Version for Protégé 4.x flavors.</rdfs:comment>
        <owl:imports rdf:resource="http://sqwrl.stanford.edu/ontologies/built-ins/3.4/sqwrl.owl"/>
        <owl:imports rdf:resource="http://www.anr-proteus.fr/sites/default/files/download/Ontology/information.owl"/>
        <owl:imports rdf:resource="http://www.anr-proteus.fr/sites/default/files/download/Ontology/kernel.owl"/>
        <owl:imports rdf:resource="http://www.anr-proteus.fr/sites/default/files/download/Ontology/system.owl"/>
    </owl:Ontology>
    


    <!-- 
    ///////////////////////////////////////////////////////////////////////////////////////
    //
    // Object Properties
    //
    ///////////////////////////////////////////////////////////////////////////////////////
     -->

    


    <!-- http://www.anr-proteus.fr/sites/default/files/download/Ontology/mission.owl#allocatesTask -->

    <owl:ObjectProperty rdf:about="&miss;allocatesTask">
        <rdfs:comment xml:lang="en">Distributed task allocation allocates tasks</rdfs:comment>
        <rdfs:domain rdf:resource="&miss;DistributedTaskAllocation"/>
        <rdfs:range rdf:resource="&miss;Task"/>
    </owl:ObjectProperty>
    


    <!-- http://www.anr-proteus.fr/sites/default/files/download/Ontology/mission.owl#executesPlan -->

    <owl:ObjectProperty rdf:about="&miss;executesPlan">
        <rdfs:comment xml:lang="en">The executive System executes de plan generated by the planning system.</rdfs:comment>
        <rdfs:domain rdf:resource="&miss;ExecutiveSystem"/>
        <rdfs:range rdf:resource="&miss;Plan"/>
    </owl:ObjectProperty>
    


    <!-- http://www.anr-proteus.fr/sites/default/files/download/Ontology/mission.owl#hasAPlan -->

    <owl:ObjectProperty rdf:about="&miss;hasAPlan">
        <rdfs:comment xml:lang="en">The mission has a plan.</rdfs:comment>
        <rdfs:domain rdf:resource="&miss;Mission"/>
        <rdfs:range rdf:resource="&miss;Plan"/>
    </owl:ObjectProperty>
    


    <!-- http://www.anr-proteus.fr/sites/default/files/download/Ontology/mission.owl#hasConstraint -->

    <owl:ObjectProperty rdf:about="&miss;hasConstraint">
        <rdfs:comment xml:lang="en">The constraints of a mission define what is not possible or forbidden.</rdfs:comment>
        <rdfs:range rdf:resource="&info;Constraint"/>
        <rdfs:domain rdf:resource="&miss;Mission"/>
    </owl:ObjectProperty>
    


    <!-- http://www.anr-proteus.fr/sites/default/files/download/Ontology/mission.owl#hasDecomposition -->

    <owl:ObjectProperty rdf:about="&miss;hasDecomposition">
        <rdf:type rdf:resource="&owl;InverseFunctionalProperty"/>
        <rdfs:comment xml:lang="en">A task has zero to several decompositions i.e. different ways to perform the task.</rdfs:comment>
        <rdfs:range rdf:resource="&miss;Decomposition"/>
        <rdfs:domain rdf:resource="&miss;Task"/>
        <owl:inverseOf rdf:resource="&miss;isDecompositionOfTask"/>
    </owl:ObjectProperty>
    


    <!-- http://www.anr-proteus.fr/sites/default/files/download/Ontology/mission.owl#hasGoalState -->

    <owl:ObjectProperty rdf:about="&miss;hasGoalState">
        <rdfs:comment xml:lang="en">A mission objective may be specified as a state to be reached.</rdfs:comment>
        <rdfs:range rdf:resource="&kern;State"/>
        <rdfs:domain rdf:resource="&miss;MissionObjective"/>
    </owl:ObjectProperty>
    


    <!-- http://www.anr-proteus.fr/sites/default/files/download/Ontology/mission.owl#hasHighLevelTask -->

    <owl:ObjectProperty rdf:about="&miss;hasHighLevelTask">
        <rdfs:domain rdf:resource="&miss;MissionObjective"/>
        <rdfs:range rdf:resource="&miss;Task"/>
    </owl:ObjectProperty>
    


    <!-- http://www.anr-proteus.fr/sites/default/files/download/Ontology/mission.owl#hasObjective -->

    <owl:ObjectProperty rdf:about="&miss;hasObjective">
        <rdfs:comment xml:lang="en">A mission has objectives.</rdfs:comment>
        <rdfs:domain rdf:resource="&miss;Mission"/>
        <rdfs:range rdf:resource="&miss;MissionObjective"/>
    </owl:ObjectProperty>
    


    <!-- http://www.anr-proteus.fr/sites/default/files/download/Ontology/mission.owl#hasPlannedOperator -->

    <owl:ObjectProperty rdf:about="&miss;hasPlannedOperator">
        <rdfs:comment xml:lang="en">A plan always has planned operators.</rdfs:comment>
        <rdfs:range rdf:resource="&miss;Operator"/>
        <rdfs:domain rdf:resource="&miss;Plan"/>
    </owl:ObjectProperty>
    


    <!-- http://www.anr-proteus.fr/sites/default/files/download/Ontology/mission.owl#hasPostCondition -->

    <owl:ObjectProperty rdf:about="&miss;hasPostCondition">
        <rdfs:comment xml:lang="en">An oprator has post conditions indicating how the state is changed by the operator.</rdfs:comment>
        <rdfs:range rdf:resource="&kern;Condition"/>
        <rdfs:domain rdf:resource="&miss;Operator"/>
    </owl:ObjectProperty>
    


    <!-- http://www.anr-proteus.fr/sites/default/files/download/Ontology/mission.owl#hasPrecondition -->

    <owl:ObjectProperty rdf:about="&miss;hasPrecondition">
        <rdfs:comment xml:lang="en">A decompostion or an operator has a pre condition indicating that it is allowed.</rdfs:comment>
        <rdfs:range rdf:resource="&kern;Condition"/>
        <rdfs:domain>
            <owl:Class>
                <owl:unionOf rdf:parseType="Collection">
                    <rdf:Description rdf:about="&miss;Decomposition"/>
                    <rdf:Description rdf:about="&miss;Operator"/>
                </owl:unionOf>
            </owl:Class>
        </rdfs:domain>
    </owl:ObjectProperty>
    


    <!-- http://www.anr-proteus.fr/sites/default/files/download/Ontology/mission.owl#hasReductionTask -->

    <owl:ObjectProperty rdf:about="&miss;hasReductionTask">
        <rdfs:comment xml:lang="en">A decomposition has reduction tasks.</rdfs:comment>
        <rdfs:domain rdf:resource="&miss;Decomposition"/>
        <rdfs:range rdf:resource="&miss;Task"/>
    </owl:ObjectProperty>
    


    <!-- http://www.anr-proteus.fr/sites/default/files/download/Ontology/mission.owl#hasRessource -->

    <owl:ObjectProperty rdf:about="&miss;hasRessource">
        <rdfs:comment xml:lang="en">The ressources of a mission are the agents in charge of performing it.</rdfs:comment>
        <rdfs:range rdf:resource="&kern;Agent"/>
        <rdfs:domain rdf:resource="&miss;Mission"/>
    </owl:ObjectProperty>
    


    <!-- http://www.anr-proteus.fr/sites/default/files/download/Ontology/mission.owl#hasTaskAllocationProtocol -->

    <owl:ObjectProperty rdf:about="&miss;hasTaskAllocationProtocol">
        <rdfs:comment xml:lang="en">Distributed task allocation is based on a task allocation protocol.</rdfs:comment>
        <rdfs:domain rdf:resource="&miss;DistributedTaskAllocation"/>
        <rdfs:range rdf:resource="&miss;TaskAllocationProtocol"/>
    </owl:ObjectProperty>
    


    <!-- http://www.anr-proteus.fr/sites/default/files/download/Ontology/mission.owl#hasType -->

    <owl:ObjectProperty rdf:about="&miss;hasType">
        <rdfs:domain rdf:resource="&miss;Mission"/>
        <rdfs:range rdf:resource="&miss;MissionType"/>
    </owl:ObjectProperty>
    


    <!-- http://www.anr-proteus.fr/sites/default/files/download/Ontology/mission.owl#hasWorkFlow -->

    <owl:ObjectProperty rdf:about="&miss;hasWorkFlow">
        <rdfs:comment xml:lang="en">A mission has a workflow.</rdfs:comment>
        <rdfs:domain rdf:resource="&miss;Mission"/>
        <rdfs:range rdf:resource="&miss;WorkFlow"/>
    </owl:ObjectProperty>
    


    <!-- http://www.anr-proteus.fr/sites/default/files/download/Ontology/mission.owl#includesConstraint -->

    <owl:ObjectProperty rdf:about="&miss;includesConstraint">
        <rdfs:range rdf:resource="&info;Constraint"/>
        <rdfs:domain rdf:resource="&info;OperationalInformation"/>
    </owl:ObjectProperty>
    


    <!-- http://www.anr-proteus.fr/sites/default/files/download/Ontology/mission.owl#induceActivity -->

    <owl:ObjectProperty rdf:about="&miss;induceActivity">
        <rdfs:comment xml:lang="en">An operator, when executed, induces activities.</rdfs:comment>
        <rdfs:range rdf:resource="&kern;Activity"/>
        <rdfs:domain rdf:resource="&miss;Operator"/>
    </owl:ObjectProperty>
    


    <!-- http://www.anr-proteus.fr/sites/default/files/download/Ontology/mission.owl#isBuiltBy -->

    <owl:ObjectProperty rdf:about="&miss;isBuiltBy">
        <rdfs:comment xml:lang="en">A plan is build by an agent.</rdfs:comment>
        <rdfs:range rdf:resource="&kern;Agent"/>
        <rdfs:domain rdf:resource="&miss;Plan"/>
    </owl:ObjectProperty>
    


    <!-- http://www.anr-proteus.fr/sites/default/files/download/Ontology/mission.owl#isBuiltFrom -->

    <owl:ObjectProperty rdf:about="&miss;isBuiltFrom">
        <rdfs:domain rdf:resource="&miss;Plan"/>
        <rdfs:range>
            <owl:Class>
                <owl:unionOf rdf:parseType="Collection">
                    <rdf:Description rdf:about="&info;Constraint"/>
                    <rdf:Description rdf:about="&miss;MissionObjective"/>
                </owl:unionOf>
            </owl:Class>
        </rdfs:range>
    </owl:ObjectProperty>
    


    <!-- http://www.anr-proteus.fr/sites/default/files/download/Ontology/mission.owl#isDecompositionOfTask -->

    <owl:ObjectProperty rdf:about="&miss;isDecompositionOfTask">
        <rdf:type rdf:resource="&owl;FunctionalProperty"/>
        <rdfs:comment xml:lang="en">A decomposition is always the decomposition of a task.</rdfs:comment>
        <rdfs:domain rdf:resource="&miss;Decomposition"/>
        <rdfs:range rdf:resource="&miss;Task"/>
    </owl:ObjectProperty>
    


    <!-- http://www.anr-proteus.fr/sites/default/files/download/Ontology/mission.owl#isDescribedBy -->

    <owl:ObjectProperty rdf:about="&miss;isDescribedBy">
        <rdfs:comment xml:lang="en">A mission is described by its state machine, its constraints and its tasks. The workflow of the mission is described by the same state machine.</rdfs:comment>
        <rdfs:domain>
            <owl:Class>
                <owl:unionOf rdf:parseType="Collection">
                    <rdf:Description rdf:about="&miss;Mission"/>
                    <rdf:Description rdf:about="&miss;WorkFlow"/>
                </owl:unionOf>
            </owl:Class>
        </rdfs:domain>
        <rdfs:range>
            <owl:Class>
                <owl:unionOf rdf:parseType="Collection">
                    <rdf:Description rdf:about="&info;Constraint"/>
                    <rdf:Description rdf:about="&miss;MissionStateMachine"/>
                    <rdf:Description rdf:about="&miss;Task"/>
                </owl:unionOf>
            </owl:Class>
        </rdfs:range>
    </owl:ObjectProperty>
    


    <!-- http://www.anr-proteus.fr/sites/default/files/download/Ontology/mission.owl#isExpectedToChangeState -->

    <owl:ObjectProperty rdf:about="&miss;isExpectedToChangeState">
        <rdfs:comment xml:lang="en">An operator is expected to change state.</rdfs:comment>
        <rdfs:range rdf:resource="&kern;State"/>
        <rdfs:domain rdf:resource="&miss;Operator"/>
    </owl:ObjectProperty>
    


    <!-- http://www.anr-proteus.fr/sites/default/files/download/Ontology/mission.owl#manageMission -->

    <owl:ObjectProperty rdf:about="&miss;manageMission">
        <rdfs:comment xml:lang="en">The mission management system generates the plan with the planning system and executes it with the executive system.</rdfs:comment>
        <rdfs:range rdf:resource="&miss;Mission"/>
        <rdfs:domain rdf:resource="http://www.anr-proteus.fr/sites/default/files/download/Ontology/system.owl#MissionManagementSystem"/>
    </owl:ObjectProperty>
    


    <!-- http://www.anr-proteus.fr/sites/default/files/download/Ontology/mission.owl#performs -->

    <owl:ObjectProperty rdf:about="&miss;performs">
        <rdfs:comment xml:lang="en">An agent performs actions.</rdfs:comment>
        <rdfs:domain rdf:resource="&kern;Agent"/>
    </owl:ObjectProperty>
    


    <!-- http://www.anr-proteus.fr/sites/default/files/download/Ontology/mission.owl#producesPlan -->

    <owl:ObjectProperty rdf:about="&miss;producesPlan">
        <rdfs:comment xml:lang="en">The planning system generates a Plan which would be executed by the executive System.</rdfs:comment>
        <rdfs:range rdf:resource="&miss;Plan"/>
        <rdfs:domain rdf:resource="&miss;PlanningSystem"/>
    </owl:ObjectProperty>
    


    <!-- http://www.anr-proteus.fr/sites/default/files/download/Ontology/mission.owl#takesIntoAccount -->

    <owl:ObjectProperty rdf:about="&miss;takesIntoAccount">
        <rdfs:comment xml:lang="en">takesIntoAccount</rdfs:comment>
        <rdfs:domain rdf:resource="&miss;PlanningSystem"/>
        <rdfs:range>
            <owl:Class>
                <owl:unionOf rdf:parseType="Collection">
                    <rdf:Description rdf:about="&info;Constraint"/>
                    <rdf:Description rdf:about="&miss;MissionObjective"/>
                </owl:unionOf>
            </owl:Class>
        </rdfs:range>
    </owl:ObjectProperty>
    


    <!-- http://www.anr-proteus.fr/sites/default/files/download/Ontology/mission.owl#takesPlaceInto -->

    <owl:ObjectProperty rdf:about="&miss;takesPlaceInto">
        <rdfs:comment xml:lang="en">A mission takes place into an environement.</rdfs:comment>
        <rdfs:range rdf:resource="&kern;Environment"/>
        <rdfs:domain rdf:resource="&miss;Mission"/>
    </owl:ObjectProperty>
    


    <!-- 
    ///////////////////////////////////////////////////////////////////////////////////////
    //
    // Data properties
    //
    ///////////////////////////////////////////////////////////////////////////////////////
     -->

    


    <!-- http://www.anr-proteus.fr/sites/default/files/download/Ontology/mission.owl#isSequencial -->

    <owl:DatatypeProperty rdf:about="&miss;isSequencial">
        <rdfs:comment xml:lang="en">If it is not sequencial parallelism is allowed.</rdfs:comment>
        <rdfs:domain rdf:resource="&miss;Decomposition"/>
        <rdfs:range rdf:resource="&xsd;boolean"/>
    </owl:DatatypeProperty>
    


    <!-- 
    ///////////////////////////////////////////////////////////////////////////////////////
    //
    // Classes
    //
    ///////////////////////////////////////////////////////////////////////////////////////
     -->

    


    <!-- http://www.anr-proteus.fr/sites/default/files/download/Ontology/information.owl#OperationalInformation -->

    <rdf:Description rdf:about="&info;OperationalInformation">
        <kern:TODO xml:lang="en">The comment expresses two different concepts. They are not particularly congruent.</kern:TODO>
    </rdf:Description>
    


    <!-- http://www.anr-proteus.fr/sites/default/files/download/Ontology/mission.owl#CommunicationOfBeliefAboutEnvironment -->

    <owl:Class rdf:about="&miss;CommunicationOfBeliefAboutEnvironment">
        <rdfs:subClassOf rdf:resource="&miss;CommunicationOfBeliefs"/>
        <owl:disjointWith rdf:resource="&miss;CommunicationOfBeliefAboutOtherAgents"/>
        <owl:disjointWith rdf:resource="&miss;CommunicationOfSelfStateEstimation"/>
        <rdfs:comment xml:lang="en">Estimation of the state of the things such as targets and landmarks and of the agents not performing the mission.</rdfs:comment>
    </owl:Class>
    


    <!-- http://www.anr-proteus.fr/sites/default/files/download/Ontology/mission.owl#CommunicationOfBeliefAboutOtherAgents -->

    <owl:Class rdf:about="&miss;CommunicationOfBeliefAboutOtherAgents">
        <rdfs:subClassOf rdf:resource="&miss;CommunicationOfBeliefs"/>
        <owl:disjointWith rdf:resource="&miss;CommunicationOfSelfStateEstimation"/>
        <rdfs:comment xml:lang="en">The belief about others may be expressed with respect to own. For istance relative distance.</rdfs:comment>
    </owl:Class>
    


    <!-- http://www.anr-proteus.fr/sites/default/files/download/Ontology/mission.owl#CommunicationOfBeliefs -->

    <owl:Class rdf:about="&miss;CommunicationOfBeliefs">
        <rdfs:subClassOf rdf:resource="&kern;InterAgentCommunication"/>
        <owl:disjointWith rdf:resource="&miss;CommunicationOfIntents"/>
        <owl:disjointWith rdf:resource="&miss;CoordinationSignal"/>
        <owl:disjointWith rdf:resource="&miss;Negotiation"/>
        <rdfs:comment xml:lang="en">Exchange of data about belived state of ownship, of other agents and of the world.</rdfs:comment>
    </owl:Class>
    


    <!-- http://www.anr-proteus.fr/sites/default/files/download/Ontology/mission.owl#CommunicationOfIntents -->

    <owl:Class rdf:about="&miss;CommunicationOfIntents">
        <rdfs:subClassOf rdf:resource="&kern;InterAgentCommunication"/>
        <owl:disjointWith rdf:resource="&miss;CoordinationSignal"/>
        <owl:disjointWith rdf:resource="&miss;Negotiation"/>
        <rdfs:comment xml:lang="en">Communication of own plans.</rdfs:comment>
    </owl:Class>
    


    <!-- http://www.anr-proteus.fr/sites/default/files/download/Ontology/mission.owl#CommunicationOfSelfStateEstimation -->

    <owl:Class rdf:about="&miss;CommunicationOfSelfStateEstimation">
        <rdfs:subClassOf rdf:resource="&miss;CommunicationOfBeliefs"/>
        <rdfs:comment xml:lang="en">Corresponds mainly to the broadcast of bevived position and attitude.</rdfs:comment>
    </owl:Class>
    


    <!-- http://www.anr-proteus.fr/sites/default/files/download/Ontology/mission.owl#ContractNetProtocol -->

    <owl:Class rdf:about="&miss;ContractNetProtocol">
        <rdfs:subClassOf rdf:resource="&miss;TaskAllocationProtocol"/>
        <owl:disjointWith rdf:resource="&miss;FoundationForIntelligentPhysicalAgentsProtocol"/>
    </owl:Class>
    


    <!-- http://www.anr-proteus.fr/sites/default/files/download/Ontology/mission.owl#CoordinationSignal -->

    <owl:Class rdf:about="&miss;CoordinationSignal">
        <rdfs:subClassOf rdf:resource="&kern;InterAgentCommunication"/>
        <owl:disjointWith rdf:resource="&miss;Negotiation"/>
        <rdfs:comment xml:lang="en">This kind of communication allows coordination and synchronization at execution time.</rdfs:comment>
    </owl:Class>
    


    <!-- http://www.anr-proteus.fr/sites/default/files/download/Ontology/mission.owl#Decomposition -->

    <owl:Class rdf:about="&miss;Decomposition">
        <rdfs:subClassOf rdf:resource="&info;OperationalInformation"/>
        <owl:disjointWith rdf:resource="&miss;Mission"/>
        <owl:disjointWith rdf:resource="&miss;MissionObjective"/>
        <owl:disjointWith rdf:resource="&miss;MissionType"/>
        <owl:disjointWith rdf:resource="&miss;OperationalConstraint"/>
        <owl:disjointWith rdf:resource="&miss;Plan"/>
        <owl:disjointWith rdf:resource="&miss;Task"/>
        <owl:disjointWith rdf:resource="&miss;WorkFlow"/>
        <rdfs:comment xml:lang="en">Decomposition of a task.</rdfs:comment>
    </owl:Class>
    


    <!-- http://www.anr-proteus.fr/sites/default/files/download/Ontology/mission.owl#DistributedConflictSolving -->

    <owl:Class rdf:about="&miss;DistributedConflictSolving">
        <rdfs:subClassOf rdf:resource="&miss;Negotiation"/>
        <owl:disjointWith rdf:resource="&miss;DistributedTaskAllocation"/>
        <rdfs:comment xml:lang="en">Exchanges for solving conflicts.</rdfs:comment>
    </owl:Class>
    


    <!-- http://www.anr-proteus.fr/sites/default/files/download/Ontology/mission.owl#DistributedTaskAllocation -->

    <owl:Class rdf:about="&miss;DistributedTaskAllocation">
        <rdfs:subClassOf rdf:resource="&miss;Negotiation"/>
        <rdfs:comment xml:lang="en">Communication for distributed task allocation.</rdfs:comment>
    </owl:Class>
    


    <!-- http://www.anr-proteus.fr/sites/default/files/download/Ontology/mission.owl#EnvironmentalConstraint -->

    <owl:Class rdf:about="&miss;EnvironmentalConstraint">
        <rdfs:subClassOf rdf:resource="&info;Constraint"/>
        <owl:disjointWith rdf:resource="&miss;OperationalConstraint"/>
        <rdfs:comment xml:lang="en">This type of constraint describes the impacts of the environment on degrees of freedom for the agents involved in the mission.</rdfs:comment>
    </owl:Class>
    


    <!-- http://www.anr-proteus.fr/sites/default/files/download/Ontology/mission.owl#ExecutiveSystem -->

    <owl:Class rdf:about="&miss;ExecutiveSystem">
        <rdfs:subClassOf rdf:resource="http://www.anr-proteus.fr/sites/default/files/download/Ontology/system.owl#RoboticFunctionalSystem"/>
        <rdfs:subClassOf>
            <owl:Restriction>
                <owl:onProperty rdf:resource="http://www.anr-proteus.fr/sites/default/files/download/Ontology/system.owl#hasImplementingHardware"/>
                <owl:cardinality rdf:datatype="&xsd;nonNegativeInteger">0</owl:cardinality>
            </owl:Restriction>
        </rdfs:subClassOf>
        <rdfs:subClassOf>
            <owl:Restriction>
                <owl:onProperty rdf:resource="http://www.anr-proteus.fr/sites/default/files/download/Ontology/system.owl#hasImplementingSoftware"/>
                <owl:minCardinality rdf:datatype="&xsd;nonNegativeInteger">1</owl:minCardinality>
            </owl:Restriction>
        </rdfs:subClassOf>
        <owl:disjointWith rdf:resource="&miss;PlanningSystem"/>
        <owl:disjointWith rdf:resource="&miss;ReactiveSystem"/>
        <owl:disjointWith rdf:resource="http://www.anr-proteus.fr/sites/default/files/download/Ontology/system.owl#ControlSystem"/>
        <owl:disjointWith rdf:resource="http://www.anr-proteus.fr/sites/default/files/download/Ontology/system.owl#MissionManagementSystem"/>
        <owl:disjointWith rdf:resource="http://www.anr-proteus.fr/sites/default/files/download/Ontology/system.owl#MotionPlanningSystem"/>
        <owl:disjointWith rdf:resource="http://www.anr-proteus.fr/sites/default/files/download/Ontology/system.owl#PlatformManagementSystem"/>
        <owl:disjointWith rdf:resource="http://www.anr-proteus.fr/sites/default/files/download/Ontology/system.owl#SecuritySystem"/>
        <rdfs:comment xml:lang="en">This system is able to produce actions on the basis of a plan. It is part of the MissionManagementSystem.</rdfs:comment>
    </owl:Class>
    


    <!-- http://www.anr-proteus.fr/sites/default/files/download/Ontology/mission.owl#FiniteStateMachine -->

    <owl:Class rdf:about="&miss;FiniteStateMachine">
        <rdfs:subClassOf rdf:resource="&kern;StateMachine"/>
        <kern:TODO xml:lang="en">This concept should be moved. It is not linked to Mission ontology but to underlying ontology to decide.</kern:TODO>
    </owl:Class>
    


    <!-- http://www.anr-proteus.fr/sites/default/files/download/Ontology/mission.owl#FoundationForIntelligentPhysicalAgentsProtocol -->

    <owl:Class rdf:about="&miss;FoundationForIntelligentPhysicalAgentsProtocol">
        <rdfs:subClassOf rdf:resource="&miss;TaskAllocationProtocol"/>
    </owl:Class>
    


    <!-- http://www.anr-proteus.fr/sites/default/files/download/Ontology/mission.owl#Mission -->

    <owl:Class rdf:about="&miss;Mission">
        <rdfs:subClassOf rdf:resource="&info;OperationalInformation"/>
        <rdfs:subClassOf>
            <owl:Restriction>
                <owl:onProperty rdf:resource="&kern;isAnimatedByEvolution"/>
                <owl:allValuesFrom rdf:resource="&miss;MissionStateMachine"/>
            </owl:Restriction>
        </rdfs:subClassOf>
        <owl:disjointWith rdf:resource="&miss;MissionObjective"/>
        <owl:disjointWith rdf:resource="&miss;MissionType"/>
        <owl:disjointWith rdf:resource="&miss;OperationalConstraint"/>
        <owl:disjointWith rdf:resource="&miss;Plan"/>
        <owl:disjointWith rdf:resource="&miss;Task"/>
        <owl:disjointWith rdf:resource="&miss;WorkFlow"/>
        <rdfs:comment xml:lang="en">Description of an operational mission that can be used by the components performing it and that can be used for performence assessment.</rdfs:comment>
    </owl:Class>
    


    <!-- http://www.anr-proteus.fr/sites/default/files/download/Ontology/mission.owl#MissionObjective -->

    <owl:Class rdf:about="&miss;MissionObjective">
        <rdfs:subClassOf rdf:resource="&info;OperationalInformation"/>
        <rdfs:subClassOf>
            <owl:Restriction>
                <owl:onProperty rdf:resource="&kern;isCodedIn"/>
                <owl:allValuesFrom rdf:resource="&info;String"/>
            </owl:Restriction>
        </rdfs:subClassOf>
        <owl:disjointWith rdf:resource="&miss;MissionType"/>
        <owl:disjointWith rdf:resource="&miss;OperationalConstraint"/>
        <owl:disjointWith rdf:resource="&miss;Plan"/>
        <owl:disjointWith rdf:resource="&miss;Task"/>
        <owl:disjointWith rdf:resource="&miss;WorkFlow"/>
        <rdfs:comment xml:lang="en">The objective of a mission can be described either has a high level task to perform or as a state to be reached.</rdfs:comment>
    </owl:Class>
    


    <!-- http://www.anr-proteus.fr/sites/default/files/download/Ontology/mission.owl#MissionStateMachine -->

    <owl:Class rdf:about="&miss;MissionStateMachine">
        <rdfs:subClassOf rdf:resource="&miss;FiniteStateMachine"/>
        <rdfs:subClassOf>
            <owl:Restriction>
                <owl:onProperty rdf:resource="&kern;animates"/>
                <owl:someValuesFrom rdf:resource="&miss;Mission"/>
            </owl:Restriction>
        </rdfs:subClassOf>
    </owl:Class>
    


    <!-- http://www.anr-proteus.fr/sites/default/files/download/Ontology/mission.owl#MissionType -->

    <owl:Class rdf:about="&miss;MissionType">
        <rdfs:subClassOf rdf:resource="&info;OperationalInformation"/>
        <owl:disjointWith rdf:resource="&miss;OperationalConstraint"/>
        <owl:disjointWith rdf:resource="&miss;Plan"/>
        <owl:disjointWith rdf:resource="&miss;Task"/>
        <owl:disjointWith rdf:resource="&miss;WorkFlow"/>
        <rdfs:comment xml:lang="en">Textual or mathematical description of the kind of Mission for a specific Scenario.</rdfs:comment>
    </owl:Class>
    


    <!-- http://www.anr-proteus.fr/sites/default/files/download/Ontology/mission.owl#Negotiation -->

    <owl:Class rdf:about="&miss;Negotiation">
        <rdfs:subClassOf rdf:resource="&kern;InterAgentCommunication"/>
        <rdfs:comment xml:lang="en">For solving conflicts or for assigning tasks agents have to communicate.</rdfs:comment>
    </owl:Class>
    


    <!-- http://www.anr-proteus.fr/sites/default/files/download/Ontology/mission.owl#OperationalConstraint -->

    <owl:Class rdf:about="&miss;OperationalConstraint">
        <rdfs:subClassOf rdf:resource="&info;Constraint"/>
        <owl:disjointWith rdf:resource="&miss;Plan"/>
        <owl:disjointWith rdf:resource="&miss;Task"/>
        <owl:disjointWith rdf:resource="&miss;WorkFlow"/>
        <rdfs:comment xml:lang="en">This type of constraint defines requirements on the way the mission should be conducted and on minimal mission achievements.</rdfs:comment>
    </owl:Class>
    


    <!-- http://www.anr-proteus.fr/sites/default/files/download/Ontology/mission.owl#Operator -->

    <owl:Class rdf:about="&miss;Operator">
        <rdfs:subClassOf rdf:resource="&miss;Task"/>
        <rdfs:subClassOf>
            <owl:Restriction>
                <owl:onProperty rdf:resource="&miss;hasDecomposition"/>
                <owl:cardinality rdf:datatype="&xsd;nonNegativeInteger">0</owl:cardinality>
            </owl:Restriction>
        </rdfs:subClassOf>
        <rdfs:comment xml:lang="en">An operator is an atomic task i.e. a task without decomposition.</rdfs:comment>
    </owl:Class>
    


    <!-- http://www.anr-proteus.fr/sites/default/files/download/Ontology/mission.owl#Plan -->

    <owl:Class rdf:about="&miss;Plan">
        <rdfs:subClassOf rdf:resource="&info;OperationalInformation"/>
        <owl:disjointWith rdf:resource="&miss;Task"/>
        <owl:disjointWith rdf:resource="&miss;WorkFlow"/>
        <rdfs:comment xml:lang="en">A plan has planned operators and is built by agents taking into account mission constraints and objective.</rdfs:comment>
    </owl:Class>
    


    <!-- http://www.anr-proteus.fr/sites/default/files/download/Ontology/mission.owl#PlanningSystem -->

    <owl:Class rdf:about="&miss;PlanningSystem">
        <rdfs:subClassOf rdf:resource="http://www.anr-proteus.fr/sites/default/files/download/Ontology/system.owl#RoboticFunctionalSystem"/>
        <rdfs:subClassOf>
            <owl:Restriction>
                <owl:onProperty rdf:resource="http://www.anr-proteus.fr/sites/default/files/download/Ontology/system.owl#hasImplementingSoftware"/>
                <owl:minCardinality rdf:datatype="&xsd;nonNegativeInteger">1</owl:minCardinality>
            </owl:Restriction>
        </rdfs:subClassOf>
        <rdfs:subClassOf>
            <owl:Restriction>
                <owl:onProperty rdf:resource="http://www.anr-proteus.fr/sites/default/files/download/Ontology/system.owl#hasImplementingHardware"/>
                <owl:cardinality rdf:datatype="&xsd;nonNegativeInteger">0</owl:cardinality>
            </owl:Restriction>
        </rdfs:subClassOf>
        <owl:disjointWith rdf:resource="&miss;ReactiveSystem"/>
        <owl:disjointWith rdf:resource="http://www.anr-proteus.fr/sites/default/files/download/Ontology/system.owl#ControlSystem"/>
        <owl:disjointWith rdf:resource="http://www.anr-proteus.fr/sites/default/files/download/Ontology/system.owl#MissionManagementSystem"/>
        <owl:disjointWith rdf:resource="http://www.anr-proteus.fr/sites/default/files/download/Ontology/system.owl#MotionPlanningSystem"/>
        <owl:disjointWith rdf:resource="http://www.anr-proteus.fr/sites/default/files/download/Ontology/system.owl#PlatformManagementSystem"/>
        <owl:disjointWith rdf:resource="http://www.anr-proteus.fr/sites/default/files/download/Ontology/system.owl#SecuritySystem"/>
        <rdfs:comment xml:lang="en">This is a system which generates the plan of the mission that would be executed by the ExecutiveSystem. It is part ofo the MissionManagementSystem.</rdfs:comment>
    </owl:Class>
    


    <!-- http://www.anr-proteus.fr/sites/default/files/download/Ontology/mission.owl#ReactiveSystem -->

    <owl:Class rdf:about="&miss;ReactiveSystem">
        <rdfs:subClassOf rdf:resource="http://www.anr-proteus.fr/sites/default/files/download/Ontology/system.owl#RoboticFunctionalSystem"/>
        <rdfs:subClassOf>
            <owl:Restriction>
                <owl:onProperty rdf:resource="http://www.anr-proteus.fr/sites/default/files/download/Ontology/system.owl#hasImplementingSoftware"/>
                <owl:minCardinality rdf:datatype="&xsd;nonNegativeInteger">1</owl:minCardinality>
            </owl:Restriction>
        </rdfs:subClassOf>
        <rdfs:subClassOf>
            <owl:Restriction>
                <owl:onProperty rdf:resource="http://www.anr-proteus.fr/sites/default/files/download/Ontology/system.owl#hasImplementingHardware"/>
                <owl:cardinality rdf:datatype="&xsd;nonNegativeInteger">0</owl:cardinality>
            </owl:Restriction>
        </rdfs:subClassOf>
        <owl:disjointWith rdf:resource="http://www.anr-proteus.fr/sites/default/files/download/Ontology/system.owl#ControlSystem"/>
        <owl:disjointWith rdf:resource="http://www.anr-proteus.fr/sites/default/files/download/Ontology/system.owl#MissionManagementSystem"/>
        <owl:disjointWith rdf:resource="http://www.anr-proteus.fr/sites/default/files/download/Ontology/system.owl#MotionPlanningSystem"/>
        <owl:disjointWith rdf:resource="http://www.anr-proteus.fr/sites/default/files/download/Ontology/system.owl#PlatformManagementSystem"/>
        <owl:disjointWith rdf:resource="http://www.anr-proteus.fr/sites/default/files/download/Ontology/system.owl#SecuritySystem"/>
        <rdfs:comment xml:lang="en">This system is able to produce actions based on a behaviour.</rdfs:comment>
    </owl:Class>
    


    <!-- http://www.anr-proteus.fr/sites/default/files/download/Ontology/mission.owl#Task -->

    <owl:Class rdf:about="&miss;Task">
        <rdfs:subClassOf rdf:resource="&info;OperationalInformation"/>
        <owl:disjointWith rdf:resource="&miss;WorkFlow"/>
        <rdfs:comment xml:lang="en">It corresponds to a task as defined in Hierarchical Task Networks.</rdfs:comment>
    </owl:Class>
    


    <!-- http://www.anr-proteus.fr/sites/default/files/download/Ontology/mission.owl#TaskAllocationProtocol -->

    <owl:Class rdf:about="&miss;TaskAllocationProtocol">
        <rdfs:subClassOf rdf:resource="&kern;Protocol"/>
        <rdfs:comment xml:lang="en">A protocol to support inter-agent communication for distributed task allocation process.</rdfs:comment>
    </owl:Class>
    


    <!-- http://www.anr-proteus.fr/sites/default/files/download/Ontology/mission.owl#WorkFlow -->

    <owl:Class rdf:about="&miss;WorkFlow">
        <rdfs:subClassOf rdf:resource="&info;OperationalInformation"/>
        <rdfs:comment xml:lang="en">The way the mission should be executed.</rdfs:comment>
    </owl:Class>
    


    <!-- http://www.anr-proteus.fr/sites/default/files/download/Ontology/system.owl#ControlSystem -->

    <rdf:Description rdf:about="http://www.anr-proteus.fr/sites/default/files/download/Ontology/system.owl#ControlSystem">
        <owl:disjointWith rdf:resource="http://www.anr-proteus.fr/sites/default/files/download/Ontology/system.owl#MissionManagementSystem"/>
        <owl:disjointWith rdf:resource="http://www.anr-proteus.fr/sites/default/files/download/Ontology/system.owl#MotionPlanningSystem"/>
        <owl:disjointWith rdf:resource="http://www.anr-proteus.fr/sites/default/files/download/Ontology/system.owl#PlatformManagementSystem"/>
        <owl:disjointWith rdf:resource="http://www.anr-proteus.fr/sites/default/files/download/Ontology/system.owl#SecuritySystem"/>
    </rdf:Description>
    


    <!-- http://www.anr-proteus.fr/sites/default/files/download/Ontology/system.owl#MissionManagementSystem -->

    <rdf:Description rdf:about="http://www.anr-proteus.fr/sites/default/files/download/Ontology/system.owl#MissionManagementSystem">
        <rdfs:subClassOf>
            <owl:Restriction>
                <owl:onProperty rdf:resource="http://www.anr-proteus.fr/sites/default/files/download/Ontology/system.owl#hasImplementingSoftware"/>
                <owl:minCardinality rdf:datatype="&xsd;nonNegativeInteger">1</owl:minCardinality>
            </owl:Restriction>
        </rdfs:subClassOf>
        <rdfs:subClassOf>
            <owl:Restriction>
                <owl:onProperty rdf:resource="&kern;aggregates"/>
                <owl:allValuesFrom>
                    <owl:Class>
                        <owl:intersectionOf rdf:parseType="Collection">
                            <rdf:Description rdf:about="&miss;ExecutiveSystem"/>
                            <rdf:Description rdf:about="&miss;PlanningSystem"/>
                        </owl:intersectionOf>
                    </owl:Class>
                </owl:allValuesFrom>
            </owl:Restriction>
        </rdfs:subClassOf>
        <owl:disjointWith rdf:resource="http://www.anr-proteus.fr/sites/default/files/download/Ontology/system.owl#MotionPlanningSystem"/>
        <owl:disjointWith rdf:resource="http://www.anr-proteus.fr/sites/default/files/download/Ontology/system.owl#PlatformManagementSystem"/>
        <owl:disjointWith rdf:resource="http://www.anr-proteus.fr/sites/default/files/download/Ontology/system.owl#SecuritySystem"/>
        <rdfs:comment xml:lang="en">This system is in charge of the generation and execution of the plan. Thus it is composed of the planning and the executive system.</rdfs:comment>
    </rdf:Description>
    


    <!-- http://www.anr-proteus.fr/sites/default/files/download/Ontology/system.owl#MotionPlanningSystem -->

    <rdf:Description rdf:about="http://www.anr-proteus.fr/sites/default/files/download/Ontology/system.owl#MotionPlanningSystem">
        <rdfs:subClassOf>
            <owl:Restriction>
                <owl:onProperty rdf:resource="http://www.anr-proteus.fr/sites/default/files/download/Ontology/system.owl#hasImplementingSoftware"/>
                <owl:minCardinality rdf:datatype="&xsd;nonNegativeInteger">1</owl:minCardinality>
            </owl:Restriction>
        </rdfs:subClassOf>
        <owl:disjointWith rdf:resource="http://www.anr-proteus.fr/sites/default/files/download/Ontology/system.owl#PlatformManagementSystem"/>
        <owl:disjointWith rdf:resource="http://www.anr-proteus.fr/sites/default/files/download/Ontology/system.owl#SecuritySystem"/>
    </rdf:Description>
    


    <!-- http://www.anr-proteus.fr/sites/default/files/download/Ontology/system.owl#PlatformManagementSystem -->

    <rdf:Description rdf:about="http://www.anr-proteus.fr/sites/default/files/download/Ontology/system.owl#PlatformManagementSystem">
        <owl:disjointWith rdf:resource="http://www.anr-proteus.fr/sites/default/files/download/Ontology/system.owl#SecuritySystem"/>
    </rdf:Description>
    


    <!-- http://www.anr-proteus.fr/sites/default/files/download/Ontology/system.owl#SecuritySystem -->

    <rdf:Description rdf:about="http://www.anr-proteus.fr/sites/default/files/download/Ontology/system.owl#SecuritySystem"/>
</rdf:RDF>



<!-- Generated by the OWL API (version 3.4.2) http://owlapi.sourceforge.net -->

